##############################################################
# This file was generated on Mon, 05 Oct 2015 17:57:43 -0600
# Number of checked and rejected concepts   : 67
# Number of checked and accepted concepts   : 345
# Number of concepts that need checking     : 65
# Number of concepts with AAT match assigned: 291
##############################################################
@prefix skos: <http://www.w3.org/2004/02/skos/core#> .
@prefix rdf: <http://www.w3.org/1999/02/22-rdf-syntax-ns#> .
@prefix rdfs: <http://www.w3.org/2000/01/rdf-schema#> .
@prefix owl: <http://www.w3.org/2002/07/owl#> .
@prefix dct: <http://purl.org/dc/terms/> .
@prefix foaf: <http://xmlns.com/foaf/0.1/> .
@prefix aat: <http://vocab.getty.edu/aat/> .
@prefix dccd: <http://dendro.dans.knaw.nl/dccd-terms/> .
dccd:objectElementType rdf:type skos:ConceptScheme;
  dct:title "DCCD TRiDaS Object/Element Type Dictionary";
  dct:creator dccd:DCCD.
dccd:a7a199ae-6b80-11e5-aa5a-5ffcedf4cb3e rdf:type skos:Concept;
  skos:scopeNote """Use for lightly built, slender, open craft of shallow draft that are paddled and not rowed and normally double-ended; may have sails """@en;
  skos:exactMatch aat:300212688;
  skos:altLabel "canot"@fr;
  skos:altLabel "pirogue"@fr;
  skos:altLabel "kanu"@de;
  skos:altLabel "canoe"@en;
  skos:altLabel "canoë"@fr;
  skos:altLabel "kano"@nl;
  skos:narrower dccd:a7a1ba74-6b80-11e5-aa7a-7b1dc4c873b5;
  skos:inScheme dccd:objectElementType.
dccd:a7a1a4bc-6b80-11e5-aa5b-236804fe51af rdf:type skos:Concept;
  skos:scopeNote """shipsterm """@en;
  skos:exactMatch aat:300233025;
  skos:altLabel "kutter"@de;
  skos:altLabel "cutter"@en;
  skos:altLabel "cottre"@fr;
  skos:altLabel "kotter"@nl;
  skos:narrower dccd:a7a1ba74-6b80-11e5-aa7a-7b1dc4c873b5;
  skos:inScheme dccd:objectElementType.
dccd:a7a1a606-6b80-11e5-aa5c-1b177227ec3d rdf:type skos:Concept;
  skos:scopeNote """shipsterm """@en;
  skos:exactMatch aat:300232673;
  skos:altLabel "platboomd schip"@nl;
  skos:altLabel "plattbodenschiff"@de;
  skos:altLabel "flat bottomed vessel"@en;
  skos:altLabel "navire à fond plat"@fr;
  skos:altLabel "platbodem"@nl;
  skos:narrower dccd:a7a1ba74-6b80-11e5-aa7a-7b1dc4c873b5;
  skos:inScheme dccd:objectElementType.
dccd:a7a1a6c4-6b80-11e5-aa5d-3f5fa69529c9 rdf:type skos:Concept;
  skos:scopeNote """Rooms in or attached to churches where the sacred utensils and vestments are kept """@en;
  skos:exactMatch aat:300266764;
  skos:altLabel "vestry"@en;
  skos:altLabel "sacristy"@en;
  skos:altLabel "almerei"@de;
  skos:altLabel "gerbekammer"@de;
  skos:altLabel "sakristei"@de;
  skos:altLabel "sacristie"@fr;
  skos:altLabel "sacristie"@nl;
  skos:inScheme dccd:objectElementType.
dccd:a7a1a8e0-6b80-11e5-aa60-ff1241ceddd8 rdf:type skos:Concept;
  skos:scopeNote """Use for the outside, overhead enclosures of buildings or other structures, including the roofing and its structural framing """@en;
  skos:exactMatch aat:300002098;
  skos:altLabel "dak"@nl;
  skos:altLabel "toit, toiture"@fr;
  skos:altLabel "roof"@en;
  skos:altLabel "dach"@de;
  skos:inScheme dccd:objectElementType.
dccd:a7a1a994-6b80-11e5-aa61-7b19d7861439 rdf:type skos:Concept;
  skos:scopeNote """Interior walls separating one portion of a space from another; sometimes permanent inside walls that divide buildings into various rooms, sometimes designed to move aside and open up a space. For entities other than walls that divide interior spaces, often incorporating bookshelves, cabinets, or drawers, use 'room dividers.'"""@en;
  skos:exactMatch aat:300002538;
  skos:altLabel "partition wall"@en;
  skos:altLabel "tussenmuur"@nl;
  skos:altLabel "mur de séparation"@fr;
  skos:altLabel "mur de refend"@fr;
  skos:altLabel "tussenwand"@nl;
  skos:altLabel "scheidemauer"@de;
  skos:altLabel "partition"@en;
  skos:altLabel "trennwand"@de;
  skos:inScheme dccd:objectElementType.
dccd:a7a1aaf2-6b80-11e5-aa63-63855abd6c6f rdf:type skos:Concept;
  skos:scopeNote """shipsterm """@en;
  skos:exactMatch aat:300263189;
  skos:altLabel "deck"@de;
  skos:altLabel "deck"@en;
  skos:altLabel "pont"@fr;
  skos:altLabel "dek"@nl;
  skos:inScheme dccd:objectElementType.
dccd:a7a1ab9c-6b80-11e5-aa64-6b11fae244dd rdf:type skos:Concept;
  skos:scopeNote """Chests with deep storage space, at least one drawer, and a hinged lid. Frequently used for the storage of blankets."""@en;
  skos:exactMatch aat:300172507;
  skos:altLabel "dekenkist"@nl;
  skos:altLabel "bahut"@fr;
  skos:altLabel "blanket chest"@en;
  skos:altLabel "truhe"@de;
  skos:inScheme dccd:objectElementType.
dccd:a7a1ac46-6b80-11e5-aa65-f7acd75b8d1d rdf:type skos:Concept;
  skos:scopeNote """Braces, such as struts, which strengthen a structure or framework against the wind."""@en;
  skos:exactMatch aat:300001839;
  skos:altLabel "kopfstrebe"@de;
  skos:altLabel "strebe"@de;
  skos:altLabel "windrispe"@de;
  skos:altLabel "strut"@en;
  skos:altLabel "contreventement"@fr;
  skos:altLabel "drukschoor"@nl;
  skos:altLabel "windstrebe"@de;
  skos:altLabel "wind brace"@en;
  skos:altLabel "écharpe"@fr;
  skos:altLabel "windschoor"@nl;
  skos:inScheme dccd:objectElementType.
dccd:a7a1acf0-6b80-11e5-aa66-c3b32d16aed6 rdf:type skos:Concept;
  skos:scopeNote """Buildings belonging to and for the assembly of members of crafts, trades, or merchants' guilds"""@en;
  skos:exactMatch aat:300007077;
  skos:altLabel "handwerkshaus"@de;
  skos:altLabel "guildhall"@en;
  skos:altLabel "maison de l'artisanat"@fr;
  skos:altLabel "ambachtshuis"@nl;
  skos:inScheme dccd:objectElementType.
dccd:a7a1ada4-6b80-11e5-aa67-7f361ee65bb8 rdf:type skos:Concept;
  skos:scopeNote """Crosses in the form of the letter X, used as a heraldic symbol in the form of a diagonal cross or letter X and as a symbol for Saint Andrew, who is said to have been martyred on such a cross."""@en;
  skos:exactMatch aat:300010079;
  skos:altLabel "andreaskreuz"@de;
  skos:altLabel "saint andrew's cross"@en;
  skos:altLabel "croix de saint-andré"@fr;
  skos:altLabel "andreaskruis"@nl;
  skos:inScheme dccd:objectElementType.
dccd:a7a1ae4e-6b80-11e5-aa68-c38266563250 rdf:type skos:Concept;
  skos:scopeNote """Use for square or rectangular upright, masonry, supporting elements, and for similar elements of wood when classically treated; use also for massive upright supporting elements of any shape in Medieval architecture. For cylindrical uprights, except when Medieval as described above, and for all uprights in steel and concrete frames, use 'columns (architectural elements)'; for square wooden uprights when not classically treated, use 'posts.'"""@en;
  skos:exactMatch aat:300078728;
  skos:altLabel "pile"@fr;
  skos:altLabel "brugpijler"@nl;
  skos:altLabel "pfeiler"@de;
  skos:altLabel "pier"@en;
  skos:altLabel "pilier"@fr;
  skos:altLabel "pijler"@nl;
  skos:inScheme dccd:objectElementType.
dccd:a7a1af02-6b80-11e5-aa69-db2c32fe2881 rdf:type skos:Concept;
  skos:scopeNote """Small subordinate ribs, inserted between the main ribs of Gothic vaults."""@en;
  skos:exactMatch aat:300266287;
  skos:altLabel "verbindingsrib"@nl;
  skos:altLabel "lierne"@fr;
  skos:altLabel "lierne rib"@en;
  skos:altLabel "nebenrippe"@de;
  skos:inScheme dccd:objectElementType.
dccd:a7a1afac-6b80-11e5-aa6a-136a044ccba0 rdf:type skos:Concept;
  skos:scopeNote """A long narrow flat-bottomed boat, square at both ends and propelled with a long pole, used on inland waters chiefly for recreation"""@en;
  skos:narrower aat:300178749;
  skos:altLabel "pünte-artiges fahrzeug"@de;
  skos:altLabel "punt-like vessel"@en;
  skos:altLabel "navire aux elements constructifs de plate"@fr;
  skos:altLabel "punter-achtig vaartuig"@nl;
  skos:narrower dccd:a7a1ba74-6b80-11e5-aa7a-7b1dc4c873b5;
  skos:inScheme dccd:objectElementType.
dccd:a7a1b060-6b80-11e5-aa6b-2b06c868f4c9 rdf:type skos:Concept;
  skos:scopeNote """General term for any works made to oppose a small number of troops against a greater
Use for the habitable spaces between two floors of a building or between a floor and the roof, and for the horizontal divisions of the exteriors of buildings which tend to correspond to this division of the interior spaces"""@en;
  skos:exactMatch aat:300006888;
  skos:altLabel "fortification"@fr;
  skos:altLabel "befestigung"@de;
  skos:altLabel "versterking"@nl;
  skos:altLabel "fortification"@en;
  skos:altLabel "construction défensive"@fr;
  skos:altLabel "verdedigingswerk"@nl;
  skos:altLabel "befestigungsanlage"@de;
  skos:altLabel "festungswerk"@de;
  skos:altLabel "wehrbau"@de;
  skos:altLabel "defensive work"@en;
  skos:altLabel "ouvrage de défense"@fr;
  skos:inScheme dccd:objectElementType.
dccd:a7a1b3bc-6b80-11e5-aa70-6b98467e51b7 rdf:type skos:Concept;
  skos:narrower aat:300003632;
  skos:altLabel "roof turret"@en;
  skos:altLabel "dachreiter"@de;
  skos:altLabel "ridge turret"@en;
  skos:altLabel "dakruiter"@nl;
  skos:inScheme dccd:objectElementType.
dccd:a7a1b470-6b80-11e5-aa71-f3477fb25391 rdf:type skos:Concept;
  skos:closeMatch aat:300004188;
  skos:altLabel "achtervleugel"@nl;
  skos:altLabel "rear wing"@en;
  skos:altLabel "achterhuis"@nl;
  skos:altLabel "hinterhaus"@de;
  skos:altLabel "arrière-corps (de la maison)"@fr;
  skos:altLabel "aisle arriere"@fr;
  skos:inScheme dccd:objectElementType.
dccd:a7a1b51a-6b80-11e5-aa72-474f43f89a5f rdf:type skos:Concept;
  skos:scopeNote """Use for watercraft generally smaller and less seaworthy than ships and generally not designed to cross large open waters """@en;
  skos:exactMatch aat:300178749;
  skos:altLabel "boot"@de;
  skos:altLabel "boat"@en;
  skos:altLabel "bateau"@fr;
  skos:altLabel "boot"@nl;
  skos:narrower dccd:a7a1ba74-6b80-11e5-aa7a-7b1dc4c873b5;
  skos:inScheme dccd:objectElementType.
dccd:a7a1b5c4-6b80-11e5-aa73-bf4c2f38f1f2 rdf:type skos:Concept;
  skos:narrower aat:300000888;
  skos:altLabel "abutment"@en;
  skos:altLabel "brückenkopf"@de;
  skos:altLabel "bridge head"@en;
  skos:altLabel "tête de pont"@fr;
  skos:altLabel "bruggenhoofd"@nl;
  skos:inScheme dccd:objectElementType.
dccd:a7a1b66e-6b80-11e5-aa74-cb5e23f46409 rdf:type skos:Concept;
  skos:scopeNote """Use for small unfinished attic spaces immediately below roof ridges; Use for enclosed spaces under sloping roofs, between the roof and the ceiling of the uppermost story, especially in houses, whether used for storage or habitation. For open platforms in houses set close to ceilings or for large spaces below the roofs of commercial buildings or warehouses, use 'lofts (upper level floors)"""@en;
  skos:exactMatch aat:300004076;
  skos:altLabel "loft"@en;
  skos:altLabel "dachboden"@de;
  skos:altLabel "grenier"@fr;
  skos:altLabel "oberes dachgeschoss"@de;
  skos:altLabel "cockloft"@en;
  skos:altLabel "soupente"@fr;
  skos:altLabel "attic"@en;
  skos:altLabel "vliering"@nl;
  skos:inScheme dccd:objectElementType.
dccd:a7a1b7c2-6b80-11e5-aa76-fba313e9a5db rdf:type skos:Concept;
  skos:scopeNote """Part of the shell of the hull of a boat or ship which, in conjunction with the other strakes, keeps the sea out and the vessel afloat"""@en;
  skos:narrower aat:300212614;
  skos:altLabel "bordgang"@de;
  skos:altLabel "side strake"@en;
  skos:altLabel "bordage"@fr;
  skos:altLabel "berghout"@nl;
  skos:inScheme dccd:objectElementType.
dccd:a7a1b876-6b80-11e5-aa77-efc72bb9da1b rdf:type skos:Concept;
  skos:scopeNote """a facing of planks and piles placed along the bank of a river to prevent erosion"""@en;
  skos:narrower aat:300006136;
  skos:altLabel "uferbefestigung"@de;
  skos:altLabel "campsheeting"@en;
  skos:altLabel "palée"@fr;
  skos:altLabel "oeverbeschoeiing"@nl;
  skos:inScheme dccd:objectElementType.
dccd:a7a1b9ca-6b80-11e5-aa79-b78d5a08cec5 rdf:type skos:Concept;
  skos:scopeNote """Individual dwellings designed to be occupied by a single tenant or family. May also refer to a building for human occupation, for some purpose other than that of an ordinary dwelling; with this usage, 'house' is generally prefaced (e.g., 'cowhouse,' 'almshouse')."""@en;
  skos:exactMatch aat:300005433;
  skos:altLabel "wohnung"@de;
  skos:altLabel "residence"@en;
  skos:altLabel "demeure"@fr;
  skos:altLabel "domicile"@fr;
  skos:altLabel "habitation"@fr;
  skos:altLabel "woning"@nl;
  skos:altLabel "wohnhaus"@de;
  skos:altLabel "maison d'habitation"@fr;
  skos:altLabel "woonhuis"@nl;
  skos:altLabel "haus"@de;
  skos:altLabel "house"@en;
  skos:altLabel "maison"@fr;
  skos:altLabel "huis"@nl;
  skos:inScheme dccd:objectElementType.
dccd:a7a1ba74-6b80-11e5-aa7a-7b1dc4c873b5 rdf:type skos:Concept;
  skos:scopeNote """Top level concept for all watercraft"""@en;
  skos:exactMatch aat:300042940;
  skos:altLabel "waterscooter"@nl;
  skos:altLabel "motomarine"@fr;
  skos:altLabel "Wasserfahrzeuge"@de;
  skos:altLabel "watercraft"@en;
  skos:broader dccd:a7a199ae-6b80-11e5-aa5a-5ffcedf4cb3e;
  skos:broader dccd:a7a1a4bc-6b80-11e5-aa5b-236804fe51af;
  skos:broader dccd:a7a1a606-6b80-11e5-aa5c-1b177227ec3d;
  skos:broader dccd:a7a1afac-6b80-11e5-aa6a-136a044ccba0;
  skos:broader dccd:a7a1b51a-6b80-11e5-aa72-474f43f89a5f;
  skos:broader dccd:a7a1c4ec-6b80-11e5-aa85-3b00c067cf0e;
  skos:broader dccd:a7a1d356-6b80-11e5-aa9b-8fe3ef82f828;
  skos:broader dccd:a7a1d400-6b80-11e5-aa9c-db85c58837ab;
  skos:broader dccd:a7a1d572-6b80-11e5-aa9e-475b95e2c6da;
  skos:broader dccd:a7a20ba0-6b80-11e5-aae9-af39bcc68cdd;
  skos:broader dccd:a7a26226-6b80-11e5-ab60-7f110d55838a;
  skos:broader dccd:a7a281de-6b80-11e5-ab8d-1b18cbbaafc5;
  skos:broader dccd:a7a2bfbe-6b80-11e5-abe2-cbd88e5cbc94;
  skos:inScheme dccd:objectElementType.
dccd:a7a1bb1e-6b80-11e5-aa7b-03d67a84e6dc rdf:type skos:Concept;
  skos:scopeNote """Framing or form made of wood, steel, or plastic that serves as a support during construction, particularly as used to support the load of an arch, vault or dome during construction, for the pouring of liquid concrete in a foundation, and in other contexts."""@en;
  skos:exactMatch aat:300380423;
  skos:altLabel "formwork"@en;
  skos:altLabel "casing"@en;
  skos:altLabel "schalung"@de;
  skos:altLabel "coffrage"@fr;
  skos:altLabel "bekisting"@nl;
  skos:inScheme dccd:objectElementType.
dccd:a7a1bf74-6b80-11e5-aa7d-6fa6721c0ed1 rdf:type skos:Concept;
  skos:scopeNote """Horizontal stages or levels of a building positioned one above the other and having a habitable or usable room or set of rooms on each level. The term may also refer to horizontal divisions of the exteriors of buildings that typically, but not always, correspond to the levels of interior spaces; exterior indications of stories include tiers or rows of orders, columns, window mullions, or other features disposed horizontally one above another."""@en;
  skos:exactMatch aat:300002667;
  skos:altLabel "storey"@en;
  skos:altLabel "étage"@fr;
  skos:altLabel "stockwerk"@de;
  skos:altLabel "verdieping"@nl;
  skos:altLabel "geschoss"@de;
  skos:altLabel "stock"@de;
  skos:altLabel "floor"@en;
  skos:altLabel "story"@en;
  skos:inScheme dccd:objectElementType.
dccd:a7a1c0e6-6b80-11e5-aa7f-bf274fdccbce rdf:type skos:Concept;
  skos:scopeNote """Transverse beam cogged or tenoned on wall or arcade plates directly supports a pair of rafters or furnished wit ha rafter plate."""@en;
  skos:narrower aat:300001497;
  skos:altLabel "roof-beam"@en;
  skos:altLabel "dachbalken"@de;
  skos:altLabel "roof timber"@en;
  skos:altLabel "poutre toit"@fr;
  skos:altLabel "dakbalk"@nl;
  skos:inScheme dccd:objectElementType.
dccd:a7a1c19a-6b80-11e5-aa80-93558bd0795b rdf:type skos:Concept;
  skos:narrower aat:300001497;
  skos:altLabel "bundbalken"@de;
  skos:altLabel "tie beam"@en;
  skos:altLabel "entrait"@fr;
  skos:altLabel "gebintbalk"@nl;
  skos:inScheme dccd:objectElementType.
dccd:a7a1c244-6b80-11e5-aa81-4fa1d7cb9225 rdf:type skos:Concept;
  skos:scopeNote """Roof structure whose light rafters are supported by purlins and in particular bear the roofing materials."""@en;
  skos:narrower aat:300002098;
  skos:altLabel "pfettendach"@de;
  skos:altLabel "side purlin roof"@en;
  skos:altLabel "charpente à chevrons et pannes"@fr;
  skos:altLabel "gordingenkap"@nl;
  skos:inScheme dccd:objectElementType.
dccd:a7a1c2ee-6b80-11e5-aa82-1f8acce0948c rdf:type skos:Concept;
  skos:scopeNote """Prehistoric cemetery, typically of Bronze Age and Iron Age Europe. Grave fields are distinguished from necropoleis by the former's lack of above-ground structures, buildings, or grave markers."""@en;
  skos:narrower aat:300266755;
  skos:altLabel "gräberfeld"@de;
  skos:altLabel "grave field"@en;
  skos:altLabel "terrain des tombes"@fr;
  skos:altLabel "grafveld"@nl;
  skos:inScheme dccd:objectElementType.
dccd:a7a1c8de-6b80-11e5-aa8b-67e97dd5e510 rdf:type skos:Concept;
  skos:exactMatch aat:300040444;
  skos:altLabel "running-board"@en;
  skos:altLabel "trittbrett"@de;
  skos:altLabel "footboard"@en;
  skos:altLabel "marchepied"@fr;
  skos:altLabel "treeplank"@nl;
  skos:inScheme dccd:objectElementType.
dccd:a7a1c97e-6b80-11e5-aa8c-230309882210 rdf:type skos:Concept;
  skos:scopeNote """A piece of art in three panels either placed side by side or hinged together"""@en;
  skos:exactMatch aat:300178234;
  skos:altLabel "triplik"@de;
  skos:altLabel "triptych"@en;
  skos:altLabel "triptyque"@fr;
  skos:altLabel "triptiek"@nl;
  skos:inScheme dccd:objectElementType.
dccd:a7a1d356-6b80-11e5-aa9b-8fe3ef82f828 rdf:type skos:Concept;
  skos:scopeNote """Watercraft designed for use on canals generally long and narrow with bow and stern often nearly vertical for increased cargo capacity."""@en;
  skos:exactMatch aat:300212687#http://vocab.getty.edu/aat/300212687;
  skos:altLabel "narrow boat"@en;
  skos:altLabel "kanaalschip"@nl;
  skos:altLabel "kanalboot"@de;
  skos:altLabel "canalboat"@en;
  skos:narrower dccd:a7a1ba74-6b80-11e5-aa7a-7b1dc4c873b5;
  skos:inScheme dccd:objectElementType.
dccd:a7a1d400-6b80-11e5-aa9c-db85c58837ab rdf:type skos:Concept;
  skos:scopeNote """Generally used for oared fighting ships, principally of the Mediterranean, in operation from the Early Bronze Age until the 18th century CE; most commonly with numerous oars on one or several decks and equipped with a ram with which to damage and sink enemy vessels. For post-18th century steamships equipped with an armored prow as a primary weapon, use 'rams.'"""@en;
  skos:exactMatch aat:300125456;
  skos:altLabel "galeere"@de;
  skos:altLabel "galley"@en;
  skos:altLabel "galère"@fr;
  skos:altLabel "galei"@nl;
  skos:narrower dccd:a7a1ba74-6b80-11e5-aa7a-7b1dc4c873b5;
  skos:inScheme dccd:objectElementType.
dccd:a7a1d4b4-6b80-11e5-aa9d-47df7af937f6 rdf:type skos:Concept;
  skos:scopeNote """Parallel beams used to support floor and ceiling loads and supported in turn by larger beams, girders, bearing walls, or other members."""@en;
  skos:exactMatch aat:300001544;
  skos:altLabel "solive"@fr;
  skos:altLabel "zwischenbalken"@de;
  skos:altLabel "bintlaag"@nl;
  skos:altLabel "vloerbalk"@nl;
  skos:altLabel "felderbalken"@de;
  skos:altLabel "poutaison"@fr;
  skos:altLabel "solivage"@fr;
  skos:altLabel "solivure"@fr;
  skos:altLabel "balkenlagen"@de;
  skos:altLabel "bintwerk"@nl;
  skos:altLabel "gebälk"@de;
  skos:altLabel "potrage"@fr;
  skos:altLabel "balklaag"@nl;
  skos:altLabel "joist"@en;
  skos:inScheme dccd:objectElementType.
dccd:a7a1d572-6b80-11e5-aa9e-475b95e2c6da rdf:type skos:Concept;
  skos:scopeNote """Shipsterm Capacious, flat-bottomed vessels, usually intended to be pushed or towed, primarily for transporting cargo """@en;
  skos:exactMatch aat:300262616;
  skos:altLabel "kahn"@de;
  skos:altLabel "barge"@en;
  skos:altLabel "barge"@fr;
  skos:altLabel "aak"@nl;
  skos:narrower dccd:a7a1ba74-6b80-11e5-aa7a-7b1dc4c873b5;
  skos:inScheme dccd:objectElementType.
dccd:a7a1da90-6b80-11e5-aaa2-abbbc790ddd7 rdf:type skos:Concept;
  skos:scopeNote """Use for buildings equipped with machinery for grinding grain into flour """@en;
  skos:exactMatch aat:300006286;
  skos:altLabel "corn mill"@en;
  skos:altLabel "flour mill"@en;
  skos:altLabel "moulin à céréales"@fr;
  skos:altLabel "kornmühle"@de;
  skos:altLabel "moulin à farine"@fr;
  skos:altLabel "korenmolen"@nl;
  skos:inScheme dccd:objectElementType.
dccd:a7a1de82-6b80-11e5-aaa8-03e18eb79e22 rdf:type skos:Concept;
  skos:scopeNote """Institutions that are staffed and equipped for the diagnosis of disease, for medical and surgical treatment of the sick and the injured, and for their housing during this process. The modern hospital also often serves as a center for investigation and for teaching."""@en;
  skos:exactMatch aat:300343473;
  skos:altLabel "ziekenhuis"@nl;
  skos:altLabel "hôpital"@fr;
  skos:altLabel "hospital"@en;
  skos:altLabel "krankenhaus"@de;
  skos:inScheme dccd:objectElementType.
dccd:a7a1e3b4-6b80-11e5-aab0-c76256113241 rdf:type skos:Concept;
  skos:scopeNote """Refers to the horizontal timbers laid across the principal rafters and supporting the common rafters in a roof."""@en;
  skos:exactMatch aat:300002399;
  skos:altLabel "gording"@nl;
  skos:altLabel "worm"@nl;
  skos:altLabel "filière"@fr;
  skos:altLabel "pfette"@de;
  skos:altLabel "purlin"@en;
  skos:altLabel "fliering"@nl;
  skos:altLabel "panne"@fr;
  skos:inScheme dccd:objectElementType.
dccd:a7a1e508-6b80-11e5-aab2-ffd373add096 rdf:type skos:Concept;
  skos:scopeNote """ at the eastern side of the cloister """@en;
  skos:exactMatch aat:300007495;
  skos:altLabel "abteikirche"@de;
  skos:altLabel "abbey church"@en;
  skos:altLabel "abbatiale"@fr;
  skos:altLabel "abdijkerk"@nl;
  skos:inScheme dccd:objectElementType.
dccd:a7a1e85a-6b80-11e5-aab7-27a784c5bedf rdf:type skos:Concept;
  skos:scopeNote """Structures designed or used for the storage of commodities or merchandise """@en;
  skos:exactMatch aat:300007722;
  skos:altLabel "storehouse"@en;
  skos:altLabel "spijker"@nl;
  skos:altLabel "warehouse"@en;
  skos:altLabel "speicher"@de;
  skos:altLabel "grenier"@fr;
  skos:altLabel "spieker"@nl;
  skos:inScheme dccd:objectElementType.
dccd:a7a1e8fa-6b80-11e5-aab8-27091bd7ccec rdf:type skos:Concept;
  skos:scopeNote """Use for clearly articulated, often towerlike, building appendages containing only stairs """@en;
  skos:exactMatch aat:300130963;
  skos:altLabel "treppenturm"@de;
  skos:altLabel "stair tower"@en;
  skos:altLabel "staircase turret"@en;
  skos:altLabel "tourelle d'escalier"@fr;
  skos:altLabel "tour-escalier"@fr;
  skos:altLabel "traptoren"@nl;
  skos:inScheme dccd:objectElementType.
dccd:a7a1e9a4-6b80-11e5-aab9-f36d2e9158c6 rdf:type skos:Concept;
  skos:scopeNote """Pendulum-driven floor clocks having cases about 6 feet high or larger, developed in England in the mid-17th century """@en;
  skos:exactMatch aat:300041586;
  skos:altLabel "grandfather clock"@en;
  skos:altLabel "staande klok"@nl;
  skos:altLabel "horloge de parquet"@fr;
  skos:altLabel "standuhr"@de;
  skos:altLabel "long-case clock"@en;
  skos:inScheme dccd:objectElementType.
dccd:a7a1ea4e-6b80-11e5-aaba-f7315e356c04 rdf:type skos:Concept;
  skos:scopeNote """Use for structures of varying forms in gardens or parks designed to provide cool shady places of relaxation or retreats from summer heat """@en;
  skos:narrower aat:300006822;
  skos:altLabel "pavillion"@en;
  skos:altLabel "summerhouse"@en;
  skos:altLabel "teepavillon"@de;
  skos:altLabel "pavillon de thé"@fr;
  skos:altLabel "theekoepel"@nl;
  skos:altLabel "tea pavillion"@en;
  skos:inScheme dccd:objectElementType.
dccd:a7a1ec4c-6b80-11e5-aabd-77998b69834e rdf:type skos:Concept;
  skos:scopeNote """Refers to the ropes, wires, or chains on watercraft for securing or supporting masts, yards, and for hoisting, lowering, or trimming the sails."""@en;
  skos:exactMatch aat:300213053;
  skos:altLabel "rig"@en;
  skos:altLabel "rigging"@en;
  skos:altLabel "gréement"@fr;
  skos:altLabel "tuig"@nl;
  skos:altLabel "takelage"@de;
  skos:inScheme dccd:objectElementType.
dccd:a7a1ecf6-6b80-11e5-aabe-733b1edb25b6 rdf:type skos:Concept;
  skos:scopeNote """The strong outer works of a fortification, usually low enough to permit defensive fire"""@en;
  skos:exactMatch aat:300387515;
  skos:altLabel "bolwerk"@nl;
  skos:altLabel "bollwerk"@de;
  skos:altLabel "verschansing"@nl;
  skos:altLabel "pavois"@fr;
  skos:altLabel "bulwark"@en;
  skos:altLabel "schanzkleid"@de;
  skos:inScheme dccd:objectElementType.
dccd:a7a1eda0-6b80-11e5-aabf-4f74aad96181 rdf:type skos:Concept;
  skos:scopeNote """Openings in the wall of a building, serving to admit light, usually to permit vision, and often to admit air."""@en;
  skos:exactMatch aat:300002944;
  skos:altLabel "venster"@nl;
  skos:altLabel "fenêtre"@fr;
  skos:altLabel "window"@en;
  skos:altLabel "fenster"@de;
  skos:inScheme dccd:objectElementType.
dccd:a7a1ee4a-6b80-11e5-aac0-f39e6fcad391 rdf:type skos:Concept;
  skos:scopeNote """Use broadly for all sorts of walls constructed to resist attack."""@en;
  skos:exactMatch aat:300002485;
  skos:altLabel "mauern"@de;
  skos:altLabel "defensive wall"@en;
  skos:altLabel "verdedigingsmuur"@nl;
  skos:altLabel "mur défensif"@fr;
  skos:inScheme dccd:objectElementType.
dccd:a7a1f17e-6b80-11e5-aac5-03f16b00739e rdf:type skos:Concept;
  skos:closeMatch aat:300133704;
  skos:altLabel "kamer"@nl;
  skos:altLabel "zimmer"@de;
  skos:altLabel "room"@en;
  skos:altLabel "chambre"@fr;
  skos:altLabel "kammer"@de;
  skos:altLabel "raum"@de;
  skos:altLabel "chamber"@en;
  skos:altLabel "pièce"@fr;
  skos:altLabel "vertrek"@nl;
  skos:inScheme dccd:objectElementType.
dccd:a7a1f228-6b80-11e5-aac6-93686ee9d3e0 rdf:type skos:Concept;
  skos:scopeNote """Large, permanent, heavily fortified, defensive military positions, sometimes including a town. Larger and stronger than 'forts.'"""@en;
  skos:exactMatch aat:300006894;
  skos:altLabel "vesting"@nl;
  skos:altLabel "forteresse"@fr;
  skos:altLabel "fortress"@en;
  skos:altLabel "festung"@de;
  skos:inScheme dccd:objectElementType.
dccd:a7a1f6b0-6b80-11e5-aacd-2b888e92ae79 rdf:type skos:Concept;
  skos:scopeNote """Towers attached to churches"""@en;
  skos:exactMatch aat:300003625;
  skos:altLabel "steeple"@en;
  skos:altLabel "clocher"@fr;
  skos:altLabel "kirchturm"@de;
  skos:altLabel "churchtower"@en;
  skos:altLabel "tour d'une église"@fr;
  skos:altLabel "kerktoren"@nl;
  skos:inScheme dccd:objectElementType.
dccd:a7a1f75a-6b80-11e5-aace-73b5fb21de31 rdf:type skos:Concept;
  skos:scopeNote """Large boxes with hinged lids intended for the storage of textiles, clothing, and other articles """@en;
  skos:closeMatch aat:300038992;
  skos:altLabel "truhe"@de;
  skos:altLabel "box"@en;
  skos:altLabel "kiste"@de;
  skos:altLabel "chest"@en;
  skos:altLabel "huche"@fr;
  skos:altLabel "kist"@nl;
  skos:inScheme dccd:objectElementType.
dccd:a7a1f804-6b80-11e5-aacf-570f27e75fec rdf:type skos:Concept;
  skos:scopeNote """Use for the rooms or spaces in which bells are hung in a tower; for the entire tower structure, use 'bell towers.' """@en;
  skos:exactMatch aat:300137347;
  skos:altLabel "beffroi"@fr;
  skos:altLabel "belfry"@en;
  skos:altLabel "glockenstuhl"@de;
  skos:altLabel "klokkenstoel"@nl;
  skos:inScheme dccd:objectElementType.
dccd:a7a1f8a4-6b80-11e5-aad0-136968eb5e43 rdf:type skos:Concept;
  skos:narrower aat:300178758;
  skos:altLabel "scheibenrad"@de;
  skos:altLabel "disc wheel"@en;
  skos:altLabel "roue à toile pleine"@fr;
  skos:altLabel "schijfwiel"@nl;
  skos:inScheme dccd:objectElementType.
dccd:a7a1f96c-6b80-11e5-aad1-af8e72a87100 rdf:type skos:Concept;
  skos:scopeNote """Artificial navigable waterways."""@en;
  skos:exactMatch aat:300006075;
  skos:altLabel "canal"@en;
  skos:altLabel "canal"@fr;
  skos:altLabel "kanal"@de;
  skos:altLabel "kanaal"@nl;
  skos:altLabel "gracht"@nl;
  skos:inScheme dccd:objectElementType.
dccd:a7a206fa-6b80-11e5-aae2-03b9997c048d rdf:type skos:Concept;
  skos:closeMatch aat:300000824;
  skos:altLabel "abfallgrube"@de;
  skos:altLabel "waste pit"@en;
  skos:altLabel "fosse à déchets"@fr;
  skos:altLabel "afvalkuil"@nl;
  skos:inScheme dccd:objectElementType.
dccd:a7a207a4-6b80-11e5-aae3-c770eb3e56e5 rdf:type skos:Concept;
  skos:scopeNote """Use for constructions upon which religious sacrifice is offered. Includes both small, tablelike fixtures and larger, free-standing, outdoor structures. For the surface at which communion is celebrated in Protestant churches, use 'communion tables.' """@en;
  skos:exactMatch aat:300003725;
  skos:altLabel "altar"@de;
  skos:altLabel "altar"@en;
  skos:altLabel "autel"@fr;
  skos:altLabel "altaar"@nl;
  skos:inScheme dccd:objectElementType.
dccd:a7a2084e-6b80-11e5-aae4-97359a184c70 rdf:type skos:Concept;
  skos:scopeNote """Religious images on, above, or behind the altar of a Christian church """@en;
  skos:exactMatch aat:300075940;
  skos:altLabel "altar"@de;
  skos:altLabel "altarpiece"@en;
  skos:altLabel "retable"@fr;
  skos:altLabel "altaarstuk"@nl;
  skos:inScheme dccd:objectElementType.
dccd:a7a208f8-6b80-11e5-aae5-9709414dec40 rdf:type skos:Concept;
  skos:scopeNote """Stringed instrument.  Smallest in the violin family"""@en;
  skos:exactMatch aat:300042215;
  skos:altLabel "violin"@en;
  skos:altLabel "violon"@fr;
  skos:altLabel "viool"@nl;
  skos:altLabel "violine"@de;
  skos:inScheme dccd:objectElementType.
dccd:a7a209a2-6b80-11e5-aae6-87f34dd417e1 rdf:type skos:Concept;
  skos:exactMatch aat:300263195;
  skos:altLabel "rähm"@de;
  skos:altLabel "basting"@fr;
  skos:altLabel "bohle"@de;
  skos:altLabel "board"@en;
  skos:altLabel "madrier"@fr;
  skos:altLabel "badding"@nl;
  skos:inScheme dccd:objectElementType.
dccd:a7a20a4c-6b80-11e5-aae7-df8a7c01f739 rdf:type skos:Concept;
  skos:scopeNote """Parapets or low screens composed of balusters and carrying a rail or other horizontal member that is usually heavy in proportion to the balusters themselves """@en;
  skos:exactMatch aat:300001989;
  skos:altLabel "geländer"@de;
  skos:altLabel "balustrade"@en;
  skos:altLabel "balustrade"@fr;
  skos:altLabel "balustrade"@nl;
  skos:inScheme dccd:objectElementType.
dccd:a7a20af6-6b80-11e5-aae8-e759a16cd4db rdf:type skos:Concept;
  skos:scopeNote """Use for buildings or sets of buildings erected as common living quarters for groups of soldiers or workers"""@en;
  skos:exactMatch aat:300005665;
  skos:altLabel "barrack"@en;
  skos:altLabel "kaserne"@de;
  skos:altLabel "kazerne"@nl;
  skos:altLabel "baracke"@de;
  skos:altLabel "barak"@nl;
  skos:altLabel "barracks"@en;
  skos:altLabel "caserne"@fr;
  skos:inScheme dccd:objectElementType.
dccd:a7a20ba0-6b80-11e5-aae9-af39bcc68cdd rdf:type skos:Concept;
  skos:scopeNote """shipsterm """@en;
  skos:exactMatch aat:300233046;
  skos:altLabel "bark (ship)"@en;
  skos:altLabel "kahn"@de;
  skos:altLabel "barque"@en;
  skos:altLabel "barque"@fr;
  skos:altLabel "bark"@nl;
  skos:narrower dccd:a7a1ba74-6b80-11e5-aa7a-7b1dc4c873b5;
  skos:inScheme dccd:objectElementType.
dccd:a7a20c4a-6b80-11e5-aaea-af22b1d087a7 rdf:type skos:Concept;
  skos:exactMatch aat:300042216;
  skos:altLabel "bass"@de;
  skos:altLabel "double bass"@en;
  skos:altLabel "basse"@fr;
  skos:altLabel "bas"@nl;
  skos:inScheme dccd:objectElementType.
dccd:a7a20cea-6b80-11e5-aaeb-3b48181d1012 rdf:type skos:Concept;
  skos:scopeNote """The projecting portions of the outer wall of a fortification """@en;
  skos:exactMatch aat:300002495;
  skos:altLabel "bastei"@de;
  skos:altLabel "bastion"@de;
  skos:altLabel "bulwark"@en;
  skos:altLabel "vallum"@en;
  skos:altLabel "bastion"@nl;
  skos:altLabel "bollwerk"@de;
  skos:altLabel "bastion"@en;
  skos:altLabel "bastion"@fr;
  skos:altLabel "bolwerk"@nl;
  skos:inScheme dccd:objectElementType.
dccd:a7a20d94-6b80-11e5-aaec-2f78bc5dd7b7 rdf:type skos:Concept;
  skos:scopeNote """Use for works of art in which images and forms are carried out primarily in three dimensions, especially those that retain the quality of being tangible objects or groups of objects. """@en;
  skos:exactMatch aat:300047090;
  skos:altLabel "beeld"@nl;
  skos:altLabel "skulptur"@de;
  skos:altLabel "sculpture"@en;
  skos:altLabel "sculpture"@fr;
  skos:altLabel "beeldhouwwerk"@nl;
  skos:inScheme dccd:objectElementType.
dccd:a7a20e48-6b80-11e5-aaed-3310364db131 rdf:type skos:Concept;
  skos:exactMatch aat:300052556;
  skos:altLabel "senkgrube"@de;
  skos:altLabel "cesspit"@en;
  skos:altLabel "fosse d'aisances"@fr;
  skos:altLabel "beerput"@nl;
  skos:inScheme dccd:objectElementType.
dccd:a7a20ee8-6b80-11e5-aaee-8b094e94944d rdf:type skos:Concept;
  skos:scopeNote """Areas used for burial or entombment """@en;
  skos:exactMatch aat:300266755;
  skos:altLabel "friedhof"@de;
  skos:altLabel "cemetery"@en;
  skos:altLabel "cimetière"@fr;
  skos:altLabel "begraafplaats"@nl;
  skos:inScheme dccd:objectElementType.
dccd:a7a20f92-6b80-11e5-aaef-afc8ef4162cd rdf:type skos:Concept;
  skos:scopeNote """shipsterm """@en;
  skos:exactMatch aat:300012825;
  skos:altLabel "beplankung"@de;
  skos:altLabel "planking"@en;
  skos:altLabel "planchéiage"@fr;
  skos:altLabel "bekleding"@nl;
  skos:inScheme dccd:objectElementType.
dccd:a7a2117c-6b80-11e5-aaf2-031aa7096b69 rdf:type skos:Concept;
  skos:scopeNote """Decorative or protective facings applied to the lower portion of an interior partition or wall, such as wood paneling; Wall coverings consisting of panels of wood or other material joined in a continuous surface """@en;
  skos:exactMatch aat:300014658;
  skos:altLabel "wainscoting"@en;
  skos:altLabel "lambris"@fr;
  skos:altLabel "holzverkleidung"@de;
  skos:altLabel "panelling"@en;
  skos:altLabel "boiserie"@fr;
  skos:altLabel "labrisering"@nl;
  skos:inScheme dccd:objectElementType.
dccd:a7a21226-6b80-11e5-aaf3-4ff4cf501724 rdf:type skos:Concept;
  skos:exactMatch aat:300001993;
  skos:altLabel "poller"@de;
  skos:altLabel "rolle"@de;
  skos:altLabel "bitt"@en;
  skos:altLabel "dolphin"@en;
  skos:altLabel "bitte"@fr;
  skos:altLabel "bitte (d'amarrage)"@fr;
  skos:altLabel "bitton"@fr;
  skos:altLabel "beting"@nl;
  skos:altLabel "beting"@de;
  skos:altLabel "bollard"@en;
  skos:altLabel "bollard"@fr;
  skos:altLabel "bolder"@nl;
  skos:inScheme dccd:objectElementType.
dccd:a7a212d0-6b80-11e5-aaf4-db19f7192b77 rdf:type skos:Concept;
  skos:scopeNote """Use for subsidiary supplementary structures, whether additions to a main building or separate from it, but usually visibly distinct and often with a separate entrance. """@en;
  skos:exactMatch aat:300077063;
  skos:altLabel "dépendance"@fr;
  skos:altLabel "nebengebäude"@de;
  skos:altLabel "annex"@en;
  skos:altLabel "annexe"@fr;
  skos:altLabel "bijgebouw"@nl;
  skos:inScheme dccd:objectElementType.
dccd:a7a2137a-6b80-11e5-aaf5-7bb1cc12186c rdf:type skos:Concept;
  skos:scopeNote """shipsterm """@en;
  skos:exactMatch aat:300262666;
  skos:altLabel "stringer"@de;
  skos:altLabel "inwale"@en;
  skos:altLabel "stringer"@en;
  skos:altLabel "serre"@fr;
  skos:altLabel "dollbaum"@de;
  skos:altLabel "inboard"@en;
  skos:altLabel "préceinte interne"@fr;
  skos:altLabel "binnenboord"@nl;
  skos:inScheme dccd:objectElementType.
dccd:a7a21424-6b80-11e5-aaf6-373c7762323d rdf:type skos:Concept;
  skos:scopeNote """shipsterm """@en;
  skos:exactMatch aat:300257611;
  skos:altLabel "block"@en;
  skos:altLabel "blok"@nl;
  skos:altLabel "block"@de;
  skos:altLabel "pulley"@en;
  skos:altLabel "poulie"@fr;
  skos:altLabel "katrol"@nl;
  skos:inScheme dccd:objectElementType.
dccd:a7a214ce-6b80-11e5-aaf7-bb6b5b679f12 rdf:type skos:Concept;
  skos:exactMatch aat:300005605;
  skos:altLabel "blockbau"@de;
  skos:altLabel "log building"@en;
  skos:altLabel "construction en pièce sur pièce"@fr;
  skos:altLabel "blokbouw"@nl;
  skos:inScheme dccd:objectElementType.
dccd:a7a21618-6b80-11e5-aaf9-473905d5169b rdf:type skos:Concept;
  skos:scopeNote """shipsterm """@en;
  skos:exactMatch aat:300184745;
  skos:altLabel "galionsfigur"@de;
  skos:altLabel "figurehead"@en;
  skos:altLabel "figure de proue"@fr;
  skos:altLabel "boegbeeld"@nl;
  skos:inScheme dccd:objectElementType.
dccd:a7a216b8-6b80-11e5-aafa-630e988a1afb rdf:type skos:Concept;
  skos:scopeNote """shipsterm """@en;
  skos:exactMatch aat:300387515;
  skos:altLabel "gunwale"@en;
  skos:altLabel "wash strake"@en;
  skos:altLabel "coulisses"@fr;
  skos:altLabel "boeisel"@nl;
  skos:altLabel "dolboord"@nl;
  skos:altLabel "dollbord"@de;
  skos:altLabel "bulwark"@en;
  skos:altLabel "plat-bord"@fr;
  skos:altLabel "opboeisel"@nl;
  skos:inScheme dccd:objectElementType.
dccd:a7a21762-6b80-11e5-aafb-43033fc42c9e rdf:type skos:Concept;
  skos:scopeNote """Complexes where plants or animals are raised for livelihood or commerce """@en;
  skos:exactMatch aat:300005574;
  skos:altLabel "bauernhof"@de;
  skos:altLabel "farmhouse"@en;
  skos:altLabel "ferme"@fr;
  skos:altLabel "boerderij"@nl;
  skos:inScheme dccd:objectElementType.
dccd:a7a218b6-6b80-11e5-aafd-231cef94b760 rdf:type skos:Concept;
  skos:exactMatch aat:300004790;
  skos:altLabel "édifice"@fr;
  skos:altLabel "gebäude"@de;
  skos:altLabel "building"@en;
  skos:altLabel "bâtiment"@fr;
  skos:altLabel "gebouw"@nl;
  skos:inScheme dccd:objectElementType.
dccd:a7a21956-6b80-11e5-aafe-671430d308ae rdf:type skos:Concept;
  skos:scopeNote """shipsterm """@en;
  skos:exactMatch aat:300007951;
  skos:altLabel "gemak"@nl;
  skos:altLabel "latrine"@de;
  skos:altLabel "latrine"@en;
  skos:altLabel "latrine"@fr;
  skos:altLabel "latrine"@nl;
  skos:inScheme dccd:objectElementType.
dccd:a7a21a00-6b80-11e5-aaff-5b6dd7cf9be2 rdf:type skos:Concept;
  skos:scopeNote """Use for simple watercraft constructed by hollowing out and carving a single log; found in cultures all over the world and developed at least during the Paleolithic era """@en;
  skos:exactMatch aat:300212722;
  skos:altLabel "einbaum"@de;
  skos:altLabel "dugout"@en;
  skos:altLabel "boomstamkano"@nl;
  skos:altLabel "piroque monoxyle"@fr;
  skos:inScheme dccd:objectElementType.
dccd:a7a21cda-6b80-11e5-ab00-0f0715311ad9 rdf:type skos:Concept;
  skos:scopeNote """Horizontal structural members that span an opening in a wall and that carry the superimposed weight of the wall """@en;
  skos:exactMatch aat:300003161;
  skos:altLabel "sturz"@de;
  skos:altLabel "lintel"@en;
  skos:altLabel "linteau"@fr;
  skos:altLabel "latei"@nl;
  skos:inScheme dccd:objectElementType.
dccd:a7a21dc0-6b80-11e5-ab01-e784143b85e4 rdf:type skos:Concept;
  skos:scopeNote """Structures spanning and providing passage over waterways, topographic depressions, transportation routes, or similar circulation barriers """@en;
  skos:exactMatch aat:300007836;
  skos:altLabel "brücke"@de;
  skos:altLabel "bridge"@en;
  skos:altLabel "pont"@fr;
  skos:altLabel "brug"@nl;
  skos:inScheme dccd:objectElementType.
dccd:a7a21e6a-6b80-11e5-ab02-4f85fec033c5 rdf:type skos:Concept;
  skos:scopeNote """shipsterm """@en;
  skos:narrower aat:300263189;
  skos:altLabel "oberdeck"@de;
  skos:altLabel "upper deck"@en;
  skos:altLabel "pont supérieur"@fr;
  skos:altLabel "bovendek"@nl;
  skos:inScheme dccd:objectElementType.
dccd:a7a21fc8-6b80-11e5-ab04-7316a38eb4c3 rdf:type skos:Concept;
  skos:closeMatch aat:300197197;
  skos:altLabel "dose"@de;
  skos:altLabel "box"@en;
  skos:altLabel "boîte"@fr;
  skos:altLabel "doos"@nl;
  skos:inScheme dccd:objectElementType.
dccd:a7a22112-6b80-11e5-ab06-8f4da5958741 rdf:type skos:Concept;
  skos:scopeNote """Generally, the rear portions of watercraft."""@en;
  skos:exactMatch aat:300262678;
  skos:altLabel "achtersteven"@de;
  skos:altLabel "hintersteven"@de;
  skos:altLabel "stern"@en;
  skos:altLabel "étambot"@fr;
  skos:altLabel "achtersteven"@nl;
  skos:inScheme dccd:objectElementType.
dccd:a7a22310-6b80-11e5-ab09-233eab22434f rdf:type skos:Concept;
  skos:exactMatch aat:300038697;
  skos:altLabel "bett"@de;
  skos:altLabel "bed"@en;
  skos:altLabel "lit"@fr;
  skos:altLabel "bed"@nl;
  skos:inScheme dccd:objectElementType.
dccd:a7a2245a-6b80-11e5-ab0b-13dcf3d23b15 rdf:type skos:Concept;
  skos:scopeNote """Foremost end of a beam or joist which is usually visible as poart of the façade and often decorated."""@en;
  skos:narrower aat:300001497;
  skos:altLabel "balkenende"@de;
  skos:altLabel "balkenköpf"@de;
  skos:altLabel "beam end"@en;
  skos:altLabel "about"@fr;
  skos:altLabel "balkkop"@nl;
  skos:inScheme dccd:objectElementType.
dccd:a7a22504-6b80-11e5-ab0c-73197baed170 rdf:type skos:Concept;
  skos:scopeNote """shipsterm. A structural crosspiece sometimes forming a seat for a rower"""@en;
  skos:narrower aat:300212614;
  skos:altLabel "ruderbank"@de;
  skos:altLabel "thwart"@en;
  skos:altLabel "banc de nage"@fr;
  skos:altLabel "roeibank"@nl;
  skos:inScheme dccd:objectElementType.
dccd:a7a225a4-6b80-11e5-ab0d-afd5893ffec6 rdf:type skos:Concept;
  skos:scopeNote """Short horizontal timber lying across a wall top which receives the end of a rafter"""@en;
  skos:narrower aat:300002382;
  skos:altLabel "sattelbalken"@de;
  skos:altLabel "sole piece"@en;
  skos:altLabel "blochet"@fr;
  skos:altLabel "blokkeel"@nl;
  skos:inScheme dccd:objectElementType.
dccd:a7a226f8-6b80-11e5-ab0f-338af312608a rdf:type skos:Concept;
  skos:scopeNote """Central woody stem of a tree"""@en;
  skos:narrower aat:300375171;
  skos:altLabel "stam"@nl;
  skos:altLabel "stamm"@de;
  skos:altLabel "(tree-)trunk"@en;
  skos:altLabel "tronc"@fr;
  skos:altLabel "boomstam"@nl;
  skos:inScheme dccd:objectElementType.
dccd:a7a228f6-6b80-11e5-ab12-ef3ddd8efce1 rdf:type skos:Concept;
  skos:scopeNote """Use for buildings or groups of buildings intended primarily to serve as a fortified residence of a prince or nobleman """@en;
  skos:exactMatch aat:300006891;
  skos:altLabel "burg"@de;
  skos:altLabel "burcht"@nl;
  skos:altLabel "château"@fr;
  skos:altLabel "castle"@en;
  skos:altLabel "château fort"@fr;
  skos:altLabel "kasteel"@nl;
  skos:altLabel "kastell"@de;
  skos:inScheme dccd:objectElementType.
dccd:a7a22996-6b80-11e5-ab13-bfb96fa50660 rdf:type skos:Concept;
  skos:scopeNote """Small, ancient Roman fortified towns or outposts """@en;
  skos:exactMatch aat:300008450;
  skos:altLabel "castellum"@de;
  skos:altLabel "castellum"@en;
  skos:altLabel "castellum"@fr;
  skos:altLabel "castellum"@nl;
  skos:inScheme dccd:objectElementType.
dccd:a7a22a40-6b80-11e5-ab14-3f630f3ccb52 rdf:type skos:Concept;
  skos:exactMatch aat:300209202;
  skos:altLabel "cello"@de;
  skos:altLabel "cello"@en;
  skos:altLabel "violoncelle"@fr;
  skos:altLabel "cello"@nl;
  skos:inScheme dccd:objectElementType.
dccd:a7a22b8a-6b80-11e5-ab16-47bca7020ecc rdf:type skos:Concept;
  skos:scopeNote """Largest and lowest-pitched instruments of the violin family, having four, or more rarely, five strings, and varying considerably in size and shape. """@en;
  skos:exactMatch aat:300042216;
  skos:altLabel "kontrabass"@de;
  skos:altLabel "double bass"@en;
  skos:altLabel "contrebasse"@fr;
  skos:altLabel "contrabas"@nl;
  skos:inScheme dccd:objectElementType.
dccd:a7a22c34-6b80-11e5-ab17-87ee6d5c0187 rdf:type skos:Concept;
  skos:scopeNote """Use for barriers to confine, control, or obstruct the flow of water """@en;
  skos:exactMatch aat:300006084;
  skos:altLabel "damm"@de;
  skos:altLabel "dam"@en;
  skos:altLabel "digue"@fr;
  skos:altLabel "dam"@nl;
  skos:inScheme dccd:objectElementType.
dccd:a7a22e28-6b80-11e5-ab1a-bf248ca1c87c rdf:type skos:Concept;
  skos:scopeNote """Barriers which swing, slide, tilt, or fold to close a doorway, usually of solid and finished construction and usually leading to or separating interior spaces. Use also for similar features that close a container or a piece of case furniture. For barriers of less solid or finished construction, and usually separating two exterior spaces, use 'gates.'"""@en;
  skos:exactMatch aat:300002803;
  skos:altLabel "tür"@de;
  skos:altLabel "door"@en;
  skos:altLabel "porte"@fr;
  skos:altLabel "deur"@nl;
  skos:inScheme dccd:objectElementType.
dccd:a7a22ed2-6b80-11e5-ab1b-6f3f7fe4f155 rdf:type skos:Concept;
  skos:scopeNote """Assemblies built into a wall, consisting of two upright members (doorjambs) and a horizontal member (doorhead) and providing support on which to hang the door """@en;
  skos:exactMatch aat:300002785;
  skos:altLabel "chambranle"@fr;
  skos:altLabel "türstock"@de;
  skos:altLabel "door frame"@en;
  skos:altLabel "cadre de porte"@fr;
  skos:altLabel "deurkozijn"@nl;
  skos:inScheme dccd:objectElementType.
dccd:a7a22f7c-6b80-11e5-ab1c-4bc325430632 rdf:type skos:Concept;
  skos:exactMatch aat:300069081;
  skos:altLabel "türpfosten"@de;
  skos:altLabel "door post"@en;
  skos:altLabel "türständer"@de;
  skos:altLabel "door jamb"@en;
  skos:altLabel "piédroit d'une porte"@fr;
  skos:altLabel "deurstijl"@nl;
  skos:inScheme dccd:objectElementType.
dccd:a7a23026-6b80-11e5-ab1d-6b5cd5ffbeca rdf:type skos:Concept;
  skos:scopeNote """Use for embankments built along a river or sea and set at some distance from it to control or retain flood waters. For embankments built only to prevent flooding of low-lying land use 'levees.' """@en;
  skos:exactMatch aat:300170882;
  skos:altLabel "deich"@de;
  skos:altLabel "dike"@en;
  skos:altLabel "digue"@fr;
  skos:altLabel "dijk"@nl;
  skos:inScheme dccd:objectElementType.
dccd:a7a23170-6b80-11e5-ab1f-739f81c2d49c rdf:type skos:Concept;
  skos:scopeNote """The strongest and securest parts of castles, often used as residences """@en;
  skos:exactMatch aat:300003694;
  skos:altLabel "turmburg"@de;
  skos:altLabel "donjon"@de;
  skos:altLabel "keep"@en;
  skos:altLabel "donjon"@fr;
  skos:altLabel "donjon"@nl;
  skos:inScheme dccd:objectElementType.
dccd:a7a23210-6b80-11e5-ab20-0b39385c7414 rdf:type skos:Concept;
  skos:exactMatch aat:300197585;
  skos:altLabel "sarg"@de;
  skos:altLabel "coffin"@en;
  skos:altLabel "cercueil"@fr;
  skos:altLabel "doodkist"@nl;
  skos:inScheme dccd:objectElementType.
dccd:a7a232ba-6b80-11e5-ab21-07bb844f9fc5 rdf:type skos:Concept;
  skos:scopeNote """Strips fastened to the floor beneath a door, usually required to cover the joint when two types of floor material meet; may provide weather protection on external doors; for the lower sides and bottom of doorways, use 'doorsills'"""@en;
  skos:exactMatch aat:300002800;
  skos:altLabel "schwell"@de;
  skos:altLabel "türschwelle"@de;
  skos:altLabel "doorstep"@en;
  skos:altLabel "sill"@en;
  skos:altLabel "seuil de porte"@fr;
  skos:altLabel "dorpel"@nl;
  skos:altLabel "onderdorpel"@nl;
  skos:altLabel "voetplaat"@nl;
  skos:altLabel "schwelle"@de;
  skos:altLabel "threshold"@en;
  skos:altLabel "seuil"@fr;
  skos:altLabel "drempel"@nl;
  skos:inScheme dccd:objectElementType.
dccd:a7a23364-6b80-11e5-ab22-eff9c2a3f34b rdf:type skos:Concept;
  skos:scopeNote """Use for drainage structures that extend across and beneath roadways, canals, embankments, or traveled ways other than bridges. """@en;
  skos:exactMatch aat:300006116;
  skos:altLabel "düker"@de;
  skos:altLabel "culvert"@en;
  skos:altLabel "ponceau"@fr;
  skos:altLabel "duiker"@nl;
  skos:inScheme dccd:objectElementType.
dccd:a7a2340e-6b80-11e5-ab23-cb99667f375d rdf:type skos:Concept;
  skos:exactMatch aat:300001525;
  skos:altLabel "quergurt"@de;
  skos:altLabel "querriegel"@de;
  skos:altLabel "quervergurtung"@de;
  skos:altLabel "transverse timber"@en;
  skos:altLabel "barrot"@fr;
  skos:altLabel "poutre transversale"@fr;
  skos:altLabel "dwarshout"@nl;
  skos:altLabel "querbalken"@de;
  skos:altLabel "sommier transversal"@fr;
  skos:altLabel "cross beam"@en;
  skos:altLabel "dwarsbalk"@nl;
  skos:inScheme dccd:objectElementType.
dccd:a7a234b8-6b80-11e5-ab24-e366a2f6f212 rdf:type skos:Concept;
  skos:scopeNote """Transverse arms of cruciform churches A series of steps or flights of steps connected by landings for passing from one level to another """@en;
  skos:exactMatch aat:300004645;
  skos:altLabel "querschiff"@de;
  skos:altLabel "dwarsschip"@nl;
  skos:altLabel "kreuzschiff"@de;
  skos:altLabel "transept"@en;
  skos:altLabel "transept"@fr;
  skos:altLabel "transept"@nl;
  skos:inScheme dccd:objectElementType.
dccd:a7a23562-6b80-11e5-ab25-0f4dcd1c05e8 rdf:type skos:Concept;
  skos:scopeNote """Use for those parts of structures, usually located below ground level, that transmit building loads to the soil or rock underneath; when specifically distinguishing the support systems and areas of structures below ground, including the foundation, from the above-ground portions, use 'substructures.'"""@en;
  skos:exactMatch aat:300000919;
  skos:altLabel "fundament"@de;
  skos:altLabel "foundation"@en;
  skos:altLabel "fondation"@fr;
  skos:altLabel "fundering"@nl;
  skos:inScheme dccd:objectElementType.
dccd:a7a23602-6b80-11e5-ab26-2719b631ebe1 rdf:type skos:Concept;
  skos:exactMatch aat:300000923;
  skos:altLabel "gründungspfahl"@de;
  skos:altLabel "foundation pile"@en;
  skos:altLabel "pilot de fondation"@fr;
  skos:altLabel "funderingspaal"@nl;
  skos:inScheme dccd:objectElementType.
dccd:a7a236ac-6b80-11e5-ab27-6f988d915f57 rdf:type skos:Concept;
  skos:scopeNote """Implements punishment for hanging criminals, consisting of two, three or four poles connected by a crossbar and equipped with nooses."""@en;
  skos:exactMatch aat:300266883;
  skos:altLabel "galgen"@de;
  skos:altLabel "gallow"@en;
  skos:altLabel "potence"@fr;
  skos:altLabel "galg"@nl;
  skos:inScheme dccd:objectElementType.
dccd:a7a2264e-6b80-11e5-ab0e-ff0eba6d3e67 rdf:type skos:Concept;
  skos:scopeNote """The fronts or forwardmost ends of watercraft"""@en;
  skos:exactMatch aat:300248152;
  skos:altLabel "bug"@de;
  skos:altLabel "proue"@fr;
  skos:altLabel "boeg"@nl;
  skos:altLabel "prow"@en;
  skos:altLabel "bow"@en;
  skos:inScheme dccd:objectElementType.
dccd:a7a237f6-6b80-11e5-ab29-6308fe52a0ff rdf:type skos:Concept;
  skos:scopeNote """Use for passages affording entrance to the rooms of a building"""@en;
  skos:exactMatch aat:300004294;
  skos:altLabel "corridor"@en;
  skos:altLabel "gang"@de;
  skos:altLabel "hallway"@en;
  skos:altLabel "couloir"@fr;
  skos:altLabel "gang"@nl;
  skos:inScheme dccd:objectElementType.
dccd:a7a23c38-6b80-11e5-ab2c-03574548406f rdf:type skos:Concept;
  skos:scopeNote """Narrow boards used to build up a curved surface """@en;
  skos:exactMatch aat:300014680;
  skos:altLabel "daube"@de;
  skos:altLabel "stave"@en;
  skos:altLabel "douelle"@fr;
  skos:altLabel "duig"@nl;
  skos:inScheme dccd:objectElementType.
dccd:a7a23cec-6b80-11e5-ab2d-37c99bdad629 rdf:type skos:Concept;
  skos:scopeNote """The covering, usually wood boards, plywood, or wallboard, placed over the exterior studding or rafters of a building; provides a base for the application of wall or roof siding."""@en;
  skos:exactMatch aat:300014900;
  skos:altLabel "doublage"@fr;
  skos:altLabel "huidbeplating"@nl;
  skos:altLabel "plankenbeslag"@de;
  skos:altLabel "sheathing"@en;
  skos:altLabel "revêtement"@fr;
  skos:altLabel "dubbeling"@nl;
  skos:inScheme dccd:objectElementType.
dccd:a7a23eae-6b80-11e5-ab2e-4fcae47a03e2 rdf:type skos:Concept;
  skos:scopeNote """Remains of a tree when it has been cut down"""@en;
  skos:narrower aat:300375171;
  skos:altLabel "baumstumpf"@de;
  skos:altLabel "tree stump"@en;
  skos:altLabel "souche"@fr;
  skos:altLabel "boomstronk"@nl;
  skos:inScheme dccd:objectElementType.
dccd:a7a23f80-6b80-11e5-ab2f-cfb996b6cf65 rdf:type skos:Concept;
  skos:scopeNote """Use for those surfaces or portions of objects that face forward or are regarded as the most important or useful. For the adjective describing the location of something at or near the front of something, use 'front' from the Attributes and Properties hierarchy; Use for those exterior faces of a building which are substantially in one plane and seem to have been designed with special regard to their conspicuousness or association with entrance. Distinct from 'elevations (building divisions),' which may constitute any side or face of a building or large interior space"""@en;
  skos:exactMatch aat:300002526;
  skos:altLabel "gevel"@nl;
  skos:altLabel "pui"@nl;
  skos:altLabel "giebel"@de;
  skos:altLabel "façade"@en;
  skos:altLabel "façade"@fr;
  skos:altLabel "voorgevel"@nl;
  skos:inScheme dccd:objectElementType.
dccd:a7a24034-6b80-11e5-ab30-3bafcc09ae77 rdf:type skos:Concept;
  skos:exactMatch aat:300001324;
  skos:altLabel "gewölbe"@de;
  skos:altLabel "vault"@en;
  skos:altLabel "voûte"@fr;
  skos:altLabel "gewelf"@nl;
  skos:inScheme dccd:objectElementType.
dccd:a7a240de-6b80-11e5-ab31-3f3010557bc2 rdf:type skos:Concept;
  skos:exactMatch aat:300042025;
  skos:altLabel "gitarre"@de;
  skos:altLabel "guitar"@en;
  skos:altLabel "guitare"@fr;
  skos:altLabel "gitaar"@nl;
  skos:inScheme dccd:objectElementType.
dccd:a7a24188-6b80-11e5-ab32-e3504b08f149 rdf:type skos:Concept;
  skos:scopeNote """Storehouses or other repositories for grain, especially after it has been threshed or husked; sometimes also used to store corn """@en;
  skos:exactMatch aat:300004929;
  skos:altLabel "getreidespeicher"@de;
  skos:altLabel "granary"@en;
  skos:altLabel "grange"@fr;
  skos:altLabel "graanschuur"@nl;
  skos:inScheme dccd:objectElementType.
dccd:a7a24228-6b80-11e5-ab33-b35d8e4f08a0 rdf:type skos:Concept;
  skos:scopeNote """Excavations in the earth used for burial; for constructions raised over or around burial sites, use 'tombs.' """@en;
  skos:exactMatch aat:300005907;
  skos:altLabel "grab"@de;
  skos:altLabel "grave"@en;
  skos:altLabel "sépulture"@fr;
  skos:altLabel "graf"@nl;
  skos:inScheme dccd:objectElementType.
dccd:a7a242d2-6b80-11e5-ab34-bf914e9572a7 rdf:type skos:Concept;
  skos:exactMatch aat:300236072;
  skos:altLabel "sattelholz"@de;
  skos:altLabel "bolster"@en;
  skos:altLabel "chapeau"@fr;
  skos:altLabel "sleutelstuk"@nl;
  skos:inScheme dccd:objectElementType.
dccd:a7a2437c-6b80-11e5-ab35-1f9ef4aefe4f rdf:type skos:Concept;
  skos:scopeNote """Mansions belonging to, or used by, the lord of a manor"""@en;
  skos:exactMatch aat:300005579;
  skos:altLabel "demeure"@fr;
  skos:altLabel "herrenhaus"@de;
  skos:altLabel "versterkt huis"@nl;
  skos:altLabel "manor house"@en;
  skos:altLabel "buitenplaats"@nl;
  skos:altLabel "manor"@en;
  skos:inScheme dccd:objectElementType.
dccd:a7a244c6-6b80-11e5-ab37-db050af39099 rdf:type skos:Concept;
  skos:scopeNote """Rafters which are at right angles to the eaves of a roof and extend from the plate to the ridgeboard """@en;
  skos:closeMatch aat:300002424;
  skos:altLabel "dachsparren"@de;
  skos:altLabel "rafe"@de;
  skos:altLabel "rofe"@de;
  skos:altLabel "common rafter"@en;
  skos:altLabel "spar"@en;
  skos:altLabel "dakspoor"@nl;
  skos:altLabel "keper"@nl;
  skos:altLabel "spar"@nl;
  skos:altLabel "sparren"@de;
  skos:altLabel "rafter"@en;
  skos:altLabel "chevron"@fr;
  skos:altLabel "spoor"@nl;
  skos:inScheme dccd:objectElementType.
dccd:a7a24570-6b80-11e5-ab38-038b649415d6 rdf:type skos:Concept;
  skos:scopeNote """Beam running transversely across a building tying together two or more parts of a structure"""@en;
  skos:narrower aat:300001497;
  skos:altLabel "deckbalken"@de;
  skos:altLabel "deckbinderbalken"@de;
  skos:altLabel "superimposed tiebeam"@en;
  skos:altLabel "solive"@fr;
  skos:altLabel "dekbalk"@nl;
  skos:inScheme dccd:objectElementType.
dccd:a7a2461a-6b80-11e5-ab39-6349af355cf8 rdf:type skos:Concept;
  skos:narrower aat:300001497;
  skos:altLabel "tragbalken"@de;
  skos:altLabel "supporting beam"@en;
  skos:altLabel "poutre"@fr;
  skos:altLabel "draagbalk"@nl;
  skos:inScheme dccd:objectElementType.
dccd:a7a246ba-6b80-11e5-ab3a-3f1c0aa96493 rdf:type skos:Concept;
  skos:scopeNote """shipsterm """@en;
  skos:exactMatch aat:300002022;
  skos:altLabel "handlauf"@de;
  skos:altLabel "handrail"@en;
  skos:altLabel "main courante"@fr;
  skos:altLabel "handlijst"@nl;
  skos:inScheme dccd:objectElementType.
dccd:a7a24764-6b80-11e5-ab3b-d36a7e0aaa6b rdf:type skos:Concept;
  skos:scopeNote """Horizontal members which tie together and stiffen two opposite rafters, usually at a point about halfway up the rafters. """@en;
  skos:exactMatch aat:300078937;
  skos:altLabel "collar"@en;
  skos:altLabel "kehlbalken"@de;
  skos:altLabel "collar beam"@en;
  skos:altLabel "petit-entrait"@fr;
  skos:altLabel "hanenbalk"@nl;
  skos:inScheme dccd:objectElementType.
dccd:a7a24804-6b80-11e5-ab3c-e789163eed6c rdf:type skos:Concept;
  skos:exactMatch aat:300004575;
  skos:altLabel "heiligtum"@de;
  skos:altLabel "sanctuary"@en;
  skos:altLabel "sanctuaire"@fr;
  skos:altLabel "heiligdom"@nl;
  skos:inScheme dccd:objectElementType.
dccd:a7a248ae-6b80-11e5-ab3d-8f2c726266cc rdf:type skos:Concept;
  skos:scopeNote """Use for piles driven into position at the site """@en;
  skos:exactMatch aat:300000948;
  skos:altLabel "rammpfahl"@de;
  skos:altLabel "driven pile"@en;
  skos:altLabel "pilot"@fr;
  skos:altLabel "heipaal"@nl;
  skos:inScheme dccd:objectElementType.
dccd:a7a249ee-6b80-11e5-ab3f-cfe14f6349a7 rdf:type skos:Concept;
  skos:scopeNote """Designates ancient Roman storage buildings or warehouses, commonly used as granaries or for wine storage """@en;
  skos:exactMatch aat:300120504;
  skos:altLabel "horreum"@de;
  skos:altLabel "horreum"@en;
  skos:altLabel "horreum"@fr;
  skos:altLabel "horreum"@nl;
  skos:inScheme dccd:objectElementType.
dccd:a7a24c82-6b80-11e5-ab43-87d2a39ba864 rdf:type skos:Concept;
  skos:scopeNote """Images produced in the Eastern Rite churches, since the 6th century, according to prescribed formulas of subject (Christ, the Virgin, saints, and the great feasts) and composition, for devotional use in the church or home. Most commonly tempera on panel, but may be in any two-dimensional or relief medium, including fresco."""@en;
  skos:exactMatch aat:300033945;
  skos:altLabel "ikone"@de;
  skos:altLabel "icon"@en;
  skos:altLabel "icône"@fr;
  skos:altLabel "icoon"@nl;
  skos:inScheme dccd:objectElementType.
dccd:a7a24e76-6b80-11e5-ab46-bb78bbf94d92 rdf:type skos:Concept;
  skos:scopeNote """Shaped wooden bars resting on the shoulders of one or more animals to allow them to pull together, especially for drawing a plow or a load """@en;
  skos:exactMatch aat:300255560;
  skos:altLabel "joch"@de;
  skos:altLabel "yoke"@en;
  skos:altLabel "joug"@fr;
  skos:altLabel "juk"@nl;
  skos:inScheme dccd:objectElementType.
dccd:a7a24fc0-6b80-11e5-ab48-3b0d498a7626 rdf:type skos:Concept;
  skos:scopeNote """Case furniture consisting of a set of shelves, small drawers, or pigeonholes, fronted by one or more doors, and intended for the storage and sometimes the display of small objects. Also, similar built-in or fitted cases often designed for specific purposes, as in a kitchen or bathroom."""@en;
  skos:exactMatch aat:300038888;
  skos:altLabel "kabinettschrank"@de;
  skos:altLabel "cabinet"@en;
  skos:altLabel "cabinet"@fr;
  skos:altLabel "kabinet"@nl;
  skos:inScheme dccd:objectElementType.
dccd:a7a25060-6b80-11e5-ab49-bfcd805f1279 rdf:type skos:Concept;
  skos:scopeNote """Use for the outside, overhead enclosures of buildings or other structures, including the roofing and its structural framing """@en;
  skos:exactMatch aat:300002098;
  skos:altLabel "dachstuhl"@de;
  skos:altLabel "roof"@en;
  skos:altLabel "charpente"@fr;
  skos:altLabel "kap"@nl;
  skos:inScheme dccd:objectElementType.
dccd:a7a2510a-6b80-11e5-ab4a-7becef25d48f rdf:type skos:Concept;
  skos:scopeNote """Rooms or buildings that serve as sanctuaries or places of Christian worship. A chapel may be used for private worship in or attached to a church, palace, house, prison, monastery, or school, or it may be used for public worship of the established Church, subordinate to or dependent upon the parish church, the accommodation supplied by which it in some way supplements. The concept includes both freestanding chapels and rooms or recesses serving as chapels in churches or other buildings."""@en;
  skos:exactMatch aat:300004590;
  skos:altLabel "kapelle"@de;
  skos:altLabel "chapel"@en;
  skos:altLabel "chapelle"@fr;
  skos:altLabel "kapel"@nl;
  skos:inScheme dccd:objectElementType.
dccd:a7a251b4-6b80-11e5-ab4b-e3cc6d9519b7 rdf:type skos:Concept;
  skos:exactMatch aat:300004759;
  skos:altLabel "keller"@de;
  skos:altLabel "cellar"@en;
  skos:altLabel "cellier"@fr;
  skos:altLabel "kelder"@nl;
  skos:inScheme dccd:objectElementType.
dccd:a7a25254-6b80-11e5-ab4c-3f4a22eedb62 rdf:type skos:Concept;
  skos:exactMatch aat:300312247;
  skos:altLabel "kirche"@de;
  skos:altLabel "church"@en;
  skos:altLabel "église"@fr;
  skos:altLabel "kerk"@nl;
  skos:inScheme dccd:objectElementType.
dccd:a7a252f4-6b80-11e5-ab4d-5f76b1514f4d rdf:type skos:Concept;
  skos:scopeNote """Yards which belong to churches and are used as places for burial """@en;
  skos:exactMatch aat:300008170;
  skos:altLabel "kirchhof"@de;
  skos:altLabel "churchyard"@en;
  skos:altLabel "cimetière"@fr;
  skos:altLabel "kerkhof"@nl;
  skos:inScheme dccd:objectElementType.
dccd:a7a25394-6b80-11e5-ab4e-6701c4959f11 rdf:type skos:Concept;
  skos:scopeNote """Main structural members running for and aft along the bottom of a ship or boat, to which the frame of the vessel is attached shipsterm """@en;
  skos:exactMatch aat:300263190;
  skos:altLabel "scheepskiel"@nl;
  skos:altLabel "kiel"@de;
  skos:altLabel "keel"@en;
  skos:altLabel "quille"@fr;
  skos:altLabel "kiel"@nl;
  skos:inScheme dccd:objectElementType.
dccd:a7a25b78-6b80-11e5-ab56-6721a968c026 rdf:type skos:Concept;
  skos:narrower aat:300002098;
  skos:altLabel "dachstuhl"@de;
  skos:altLabel "roof framing"@en;
  skos:altLabel "dachwerk"@de;
  skos:altLabel "roof construction"@en;
  skos:altLabel "combles"@fr;
  skos:altLabel "kapconstructie"@nl;
  skos:inScheme dccd:objectElementType.
dccd:a7a25c22-6b80-11e5-ab57-eb22fc13837a rdf:type skos:Concept;
  skos:scopeNote """Parallel beams used to support floor and ceiling loads and supported in turn by larger beams, girders, bearing walls, or other members. """@en;
  skos:closeMatch aat:300001544;
  skos:altLabel "common joist"@en;
  skos:altLabel "kindbalken"@de;
  skos:altLabel "joist"@en;
  skos:altLabel "solive"@fr;
  skos:altLabel "kinderbalk"@nl;
  skos:inScheme dccd:objectElementType.
dccd:a7a25ccc-6b80-11e5-ab58-13cee7d43029 rdf:type skos:Concept;
  skos:scopeNote """Furniture that encloses a space and is generally boxlike in structure; intended for storage or display """@en;
  skos:exactMatch aat:300039240;
  skos:altLabel "schrein"@de;
  skos:altLabel "kästchen"@de;
  skos:altLabel "kisten"@de;
  skos:altLabel "case"@en;
  skos:altLabel "closet"@en;
  skos:altLabel "cupboard"@en;
  skos:altLabel "kast"@nl;
  skos:altLabel "schrank"@de;
  skos:altLabel "case furniture"@en;
  skos:altLabel "armoire"@fr;
  skos:altLabel "kastmeubilair"@nl;
  skos:inScheme dccd:objectElementType.
dccd:a7a25d8a-6b80-11e5-ab59-ab0cee14e514 rdf:type skos:Concept;
  skos:scopeNote """Use for instruments that measure and indicate the passage of time, especially by mechanical means producing a regularly recurring action and indicating, usually by hands or changing numbers, the hours and minutes; not designed to be worn or otherwise carried about on a person. For wearable timepieces, use 'watches.'"""@en;
  skos:exactMatch aat:300041575;
  skos:altLabel "uhr"@de;
  skos:altLabel "clock"@en;
  skos:altLabel "horloge"@fr;
  skos:altLabel "klok"@nl;
  skos:inScheme dccd:objectElementType.
dccd:a7a25e34-6b80-11e5-ab5a-e75d745e341b rdf:type skos:Concept;
  skos:scopeNote """Places of religious retirement or seclusion from the world for persons under religious vows """@en;
  skos:exactMatch aat:300000641;
  skos:altLabel "convent"@en;
  skos:altLabel "couvent"@fr;
  skos:altLabel "kloster"@de;
  skos:altLabel "monastery"@en;
  skos:altLabel "monastère"@fr;
  skos:altLabel "klooster"@nl;
  skos:inScheme dccd:objectElementType.
dccd:a7a25f88-6b80-11e5-ab5c-0bf38ec1ed1d rdf:type skos:Concept;
  skos:exactMatch aat:300203596;
  skos:altLabel "schale"@de;
  skos:altLabel "schüssel"@de;
  skos:altLabel "bowl"@en;
  skos:altLabel "bol"@fr;
  skos:altLabel "kom"@nl;
  skos:inScheme dccd:objectElementType.
dccd:a7a26028-6b80-11e5-ab5d-df35d48c16ab rdf:type skos:Concept;
  skos:scopeNote """Use for watercraft engaged in commercial transport on oceans or large inland bodies of water """@en;
  skos:exactMatch aat:300232781;
  skos:altLabel "kauffahrer"@de;
  skos:altLabel "kauffahrteischiff"@de;
  skos:altLabel "trader"@en;
  skos:altLabel "trading ship"@en;
  skos:altLabel "navire marchand"@fr;
  skos:altLabel "handelsschiff"@de;
  skos:altLabel "merchant vessel"@en;
  skos:altLabel "navire de commerce"@fr;
  skos:altLabel "koopvaardijschip"@nl;
  skos:inScheme dccd:objectElementType.
dccd:a7a260d2-6b80-11e5-ab5e-47fa35ea433e rdf:type skos:Concept;
  skos:scopeNote """Use for spaces in Christian churches containing the high altar and reserved for the use of the clergy. Includes the choir when present. Use 'choirs' for the spaces in Christian churches, generally between the altar area and the nave, reserved for choristers."""@en;
  skos:exactMatch aat:300001840;
  skos:altLabel "chor"@de;
  skos:altLabel "chancel"@en;
  skos:altLabel "choeur"@fr;
  skos:altLabel "koor"@nl;
  skos:inScheme dccd:objectElementType.
dccd:a7a2617c-6b80-11e5-ab5f-1fbeea9534ad rdf:type skos:Concept;
  skos:exactMatch aat:300076128;
  skos:altLabel "chorstuhl"@de;
  skos:altLabel "choir stall"@en;
  skos:altLabel "stalle"@fr;
  skos:altLabel "koorstoel"@nl;
  skos:inScheme dccd:objectElementType.
dccd:a7a26226-6b80-11e5-ab60-7f110d55838a rdf:type skos:Concept;
  skos:scopeNote """Bottom-based merchant ships of the 13th to the 15th century, clinker-built with rounded bow and stern, fore and after castles, and very broad in the beam; occasionaly used as warships"""@en;
  skos:exactMatch aat:300232923;
  skos:altLabel "cog ship"@en;
  skos:altLabel "kogge"@de;
  skos:altLabel "cog"@en;
  skos:altLabel "cogue"@fr;
  skos:altLabel "kogge"@nl;
  skos:narrower dccd:a7a1ba74-6b80-11e5-aa7a-7b1dc4c873b5;
  skos:inScheme dccd:objectElementType.
dccd:a7a262d0-6b80-11e5-ab61-bf572e76a7e4 rdf:type skos:Concept;
  skos:scopeNote """Three-dimensional structure consisting of pendant posts, struts and straining beams."""@en;
  skos:narrower aat:300001497;
  skos:altLabel "hängewerk"@de;
  skos:altLabel "hanging truss"@en;
  skos:altLabel "supports du premier faux-entrait"@fr;
  skos:altLabel "hangwerk"@nl;
  skos:inScheme dccd:objectElementType.
dccd:a7a26370-6b80-11e5-ab62-6beeaf6283d3 rdf:type skos:Concept;
  skos:scopeNote """Upright post forming part of two distinct types of standing trusses.  Has two rows of posts or single axis row."""@en;
  skos:exactMatch aat:300002456;
  skos:altLabel "queenpost"@en;
  skos:altLabel "hangstijlstifl van een staande dakstoel"@nl;
  skos:altLabel "poinçon"@fr;
  skos:altLabel "poteau"@fr;
  skos:altLabel "jukstijl"@nl;
  skos:altLabel "stuflstander"@de;
  skos:altLabel "stuhlsaule"@de;
  skos:altLabel "mittelsaule"@de;
  skos:inScheme dccd:objectElementType.
dccd:a7a264c4-6b80-11e5-ab64-fb2cb060f063 rdf:type skos:Concept;
  skos:scopeNote """The projecting, uppermost features of classical entablatures; use also for similar features crowning a wall, in any style; corona: Overhanging vertical members of a cornice in classical architecture, supported by bed moldings and crowned by cymatia, usually with a drip to throw rainwater clear of the building."""@en;
  skos:exactMatch aat:300001788;
  skos:altLabel "corona"@en;
  skos:altLabel "kranzgesims"@de;
  skos:altLabel "cornice"@en;
  skos:altLabel "corniche"@fr;
  skos:altLabel "kroonlijst"@nl;
  skos:inScheme dccd:objectElementType.
dccd:a7a2656e-6b80-11e5-ab65-7f24dce16cb6 rdf:type skos:Concept;
  skos:exactMatch aat:300008027;
  skos:altLabel "loch"@de;
  skos:altLabel "mulde"@de;
  skos:altLabel "vertiefung"@de;
  skos:altLabel "hole"@en;
  skos:altLabel "fosse"@fr;
  skos:altLabel "grube"@de;
  skos:altLabel "pit"@en;
  skos:altLabel "trou"@fr;
  skos:altLabel "kuil"@nl;
  skos:inScheme dccd:objectElementType.
dccd:a7a26618-6b80-11e5-ab66-ab8d9e6fc590 rdf:type skos:Concept;
  skos:scopeNote """Large casks for holding liquids, especially wine, ale, or beer """@en;
  skos:exactMatch aat:300194514;
  skos:altLabel "fass"@de;
  skos:altLabel "kübel"@de;
  skos:altLabel "tub"@en;
  skos:altLabel "tun"@en;
  skos:altLabel "vat"@en;
  skos:altLabel "cuve"@fr;
  skos:altLabel "kuip"@nl;
  skos:altLabel "vat"@nl;
  skos:altLabel "tonne"@de;
  skos:altLabel "barrel"@en;
  skos:altLabel "tonneau"@fr;
  skos:altLabel "ton"@nl;
  skos:inScheme dccd:objectElementType.
dccd:a7a266c2-6b80-11e5-ab67-0b2994282775 rdf:type skos:Concept;
  skos:scopeNote """Frames, usually of wood or metal, consisting of two side pieces called stiles which are connected by crosspieces, usually round, called rungs; used as a means of climbing up or down. """@en;
  skos:exactMatch aat:300022376;
  skos:altLabel "leiter"@de;
  skos:altLabel "ladder"@en;
  skos:altLabel "échelle"@fr;
  skos:altLabel "ladder"@nl;
  skos:inScheme dccd:objectElementType.
dccd:a7a26762-6b80-11e5-ab68-6780e4cc4d70 rdf:type skos:Concept;
  skos:exactMatch aat:300040558;
  skos:altLabel "schublade"@de;
  skos:altLabel "drawer"@en;
  skos:altLabel "tiroir"@fr;
  skos:altLabel "lade"@nl;
  skos:inScheme dccd:objectElementType.
dccd:a7a2680c-6b80-11e5-ab69-cb98b6ec69b6 rdf:type skos:Concept;
  skos:closeMatch aat:300005567;
  skos:altLabel "landgut"@de;
  skos:altLabel "country estate"@en;
  skos:altLabel "domaine"@fr;
  skos:altLabel "landgoed"@nl;
  skos:inScheme dccd:objectElementType.
dccd:a7a268ac-6b80-11e5-ab6a-8bd9b38f7f29 rdf:type skos:Concept;
  skos:scopeNote """In contemporary military contexts, use for groups of huts, tents, or other shelters set up temporarily for troops; in historical contexts use for permanent or semipermanent places of encampment; use 'military bases' for contemporary permanent installations."""@en;
  skos:exactMatch aat:300000476;
  skos:altLabel "militärlager"@de;
  skos:altLabel "military camp"@en;
  skos:altLabel "camp militaire"@fr;
  skos:altLabel "legerplaats"@nl;
  skos:inScheme dccd:objectElementType.
dccd:a7a26956-6b80-11e5-ab6b-bb114e6ff487 rdf:type skos:Concept;
  skos:scopeNote """Parapets or balustrades of a lightweight, partly open, metal or wood construction; Use for railings that are intended to be grasped by the hand in order to serve as a support; may also refer to the top members of balustrades or railings """@en;
  skos:exactMatch aat:300002018;
  skos:altLabel "geländer"@de;
  skos:altLabel "railing"@en;
  skos:altLabel "rampe"@fr;
  skos:altLabel "leuning"@nl;
  skos:inScheme dccd:objectElementType.
dccd:a7a26a00-6b80-11e5-ab6c-0b87195c7120 rdf:type skos:Concept;
  skos:exactMatch aat:300001989;
  skos:altLabel "balustrade"@de;
  skos:altLabel "balustrade"@en;
  skos:altLabel "balustrade"@fr;
  skos:altLabel "balustrade"@nl;
  skos:inScheme dccd:objectElementType.
dccd:a7a26aaa-6b80-11e5-ab6d-3fafe99830a7 rdf:type skos:Concept;
  skos:scopeNote """shipsterm """@en;
  skos:exactMatch aat:300022367;
  skos:altLabel "winde"@de;
  skos:altLabel "winch"@en;
  skos:altLabel "treuil"@fr;
  skos:altLabel "windas"@nl;
  skos:inScheme dccd:objectElementType.
dccd:a7a26b4a-6b80-11e5-ab6e-2771c25a14f4 rdf:type skos:Concept;
  skos:scopeNote """Shallow piers or rectangular columns projecting only slightly from a wall and, in classical architecture, conforming with one of the orders. Shipsterm"""@en;
  skos:exactMatch aat:300002737;
  skos:altLabel "pilaster"@de;
  skos:altLabel "pilaster"@en;
  skos:altLabel "pilastre"@fr;
  skos:altLabel "pilaster"@nl;
  skos:inScheme dccd:objectElementType.
dccd:a7a26bf4-6b80-11e5-ab6f-3f4f98fb0e84 rdf:type skos:Concept;
  skos:exactMatch aat:300042101;
  skos:altLabel "laute"@de;
  skos:altLabel "lute"@en;
  skos:altLabel "luth"@fr;
  skos:altLabel "luit"@nl;
  skos:inScheme dccd:objectElementType.
dccd:a7a26e88-6b80-11e5-ab73-3b0269fd93c5 rdf:type skos:Concept;
  skos:exactMatch aat:300037680;
  skos:altLabel "möbel"@de;
  skos:altLabel "furniture"@en;
  skos:altLabel "meuble"@fr;
  skos:altLabel "meubel"@nl;
  skos:inScheme dccd:objectElementType.
dccd:a7a26fd2-6b80-11e5-ab75-eb16ea4df421 rdf:type skos:Concept;
  skos:exactMatch aat:300003092;
  skos:altLabel "montant"@fr;
  skos:altLabel "montant"@nl;
  skos:altLabel "post"@nl;
  skos:altLabel "pfosten"@de;
  skos:altLabel "mullion"@en;
  skos:altLabel "meneau"@fr;
  skos:altLabel "vensterstijl"@nl;
  skos:inScheme dccd:objectElementType.
dccd:a7a2707c-6b80-11e5-ab76-5fcac7fc7f5e rdf:type skos:Concept;
  skos:scopeNote """Steep mounds, a main feature of certain 11th- and 12th-century castles """@en;
  skos:exactMatch aat:300175482;
  skos:altLabel "burghügel"@de;
  skos:altLabel "motte"@en;
  skos:altLabel "mound"@fr;
  skos:altLabel "motte"@nl;
  skos:inScheme dccd:objectElementType.
dccd:a7a27126-6b80-11e5-ab77-a337a411c5f4 rdf:type skos:Concept;
  skos:exactMatch aat:300005768;
  skos:altLabel "museum"@de;
  skos:altLabel "museum"@en;
  skos:altLabel "musée"@fr;
  skos:altLabel "museum"@nl;
  skos:inScheme dccd:objectElementType.
dccd:a7a271c6-6b80-11e5-ab78-2b24443b781b rdf:type skos:Concept;
  skos:scopeNote """Vertical architectural members used to define and divide spaces """@en;
  skos:exactMatch aat:300002469;
  skos:altLabel "pan de mur"@fr;
  skos:altLabel "paroi"@fr;
  skos:altLabel "wand"@de;
  skos:altLabel "wall"@en;
  skos:altLabel "mur"@fr;
  skos:altLabel "wand"@nl;
  skos:inScheme dccd:objectElementType.
dccd:a7a27270-6b80-11e5-ab79-affe6c8be6a3 rdf:type skos:Concept;
  skos:scopeNote """Sound-producing apparatuses whose primary function is to play music """@en;
  skos:exactMatch aat:300041620;
  skos:altLabel "musikinstrument"@de;
  skos:altLabel "musical instrument"@en;
  skos:altLabel "instrument de musique"@fr;
  skos:altLabel "muziekinstrument"@nl;
  skos:inScheme dccd:objectElementType.
dccd:a7a27540-6b80-11e5-ab7a-6b825593ddbd rdf:type skos:Concept;
  skos:scopeNote """Designates places or areas occupied, modified, or planned to be inhabited by communities of human populations and that contain enough societal functions to be relatively self-sufficient. """@en;
  skos:exactMatch aat:300008347;
  skos:altLabel "siedlung"@de;
  skos:altLabel "settlement"@en;
  skos:altLabel "établissement humain"@fr;
  skos:altLabel "nederzetting"@nl;
  skos:inScheme dccd:objectElementType.
dccd:a7a27612-6b80-11e5-ab7b-7f0859f2568e rdf:type skos:Concept;
  skos:scopeNote """Use for chancel screens surmounted by a cross or crucifix; generally found in English church architecture;"""@en;
  skos:exactMatch aat:300265155;
  skos:altLabel "chorbühne"@de;
  skos:altLabel "lettner"@de;
  skos:altLabel "rood screen"@en;
  skos:altLabel "jubé"@fr;
  skos:altLabel "doksaal"@nl;
  skos:inScheme dccd:objectElementType.
dccd:a7a276bc-6b80-11e5-ab7c-0ba85b4da745 rdf:type skos:Concept;
  skos:scopeNote """Broad embankments or mounds of earth raised as a fortification """@en;
  skos:exactMatch aat:300002505;
  skos:altLabel "schutzwall"@de;
  skos:altLabel "rampart"@en;
  skos:altLabel "rempart"@fr;
  skos:altLabel "omwalling"@nl;
  skos:inScheme dccd:objectElementType.
dccd:a7a278b0-6b80-11e5-ab7f-3b511552498a rdf:type skos:Concept;
  skos:exactMatch aat:300001833;
  skos:altLabel "onderslag"@nl;
  skos:altLabel "unterzug"@de;
  skos:altLabel "binder"@en;
  skos:altLabel "poutre"@fr;
  skos:altLabel "onderslagbalk"@nl;
  skos:inScheme dccd:objectElementType.
dccd:a7a2795a-6b80-11e5-ab80-eba838a4233a rdf:type skos:Concept;
  skos:narrower aat:300001834;
  skos:altLabel "langschoor"@nl;
  skos:altLabel "strebe"@de;
  skos:altLabel "(long) brace"@en;
  skos:altLabel "décharge"@fr;
  skos:altLabel "schoor"@nl;
  skos:inScheme dccd:objectElementType.
dccd:a7a27b44-6b80-11e5-ab83-c3e6ee19986d rdf:type skos:Concept;
  skos:scopeNote """Intersections of the sloping sides of roofs."""@en;
  skos:exactMatch aat:300002352;
  skos:altLabel "ridge"@en;
  skos:altLabel "faîte"@fr;
  skos:altLabel "nok"@nl;
  skos:altLabel "first"@de;
  skos:altLabel "dachfirst"@de;
  skos:altLabel "firstlinie"@de;
  skos:inScheme dccd:objectElementType.
dccd:a7a27bee-6b80-11e5-ab84-9fa70eab82a4 rdf:type skos:Concept;
  skos:scopeNote """Non-earthfast post rising from the group up to the ridge and usually supports a ridge purlin."""@en;
  skos:narrower aat:300001609;
  skos:altLabel "firstständer"@de;
  skos:altLabel "ridge post"@en;
  skos:altLabel "poteau de fond porteur de la faîtière"@fr;
  skos:altLabel "nokstijl"@nl;
  skos:inScheme dccd:objectElementType.
dccd:a7a27d4c-6b80-11e5-ab86-471faf96367b rdf:type skos:Concept;
  skos:scopeNote """Cavities in the earth resulting from removal of soil and rock for purposes of building construction or archaeology."""@en;
  skos:exactMatch aat:300108265;
  skos:altLabel "ausgrabung"@de;
  skos:altLabel "excavation"@en;
  skos:altLabel "excavation"@fr;
  skos:altLabel "opgraving"@nl;
  skos:inScheme dccd:objectElementType.
dccd:a7a27f40-6b80-11e5-ab89-1347ece9c897 rdf:type skos:Concept;
  skos:scopeNote """Complex aerophones consisting of one or more rows of individual pipes which are made to sound by air under pressure directed from a wind-raising device and admitted to the pipes by means of valves operated from a keyboard or set of levers """@en;
  skos:exactMatch aat:300041686;
  skos:altLabel "orgel"@de;
  skos:altLabel "organ"@en;
  skos:altLabel "orgue"@fr;
  skos:altLabel "orgel"@nl;
  skos:inScheme dccd:objectElementType.
dccd:a7a2808a-6b80-11e5-ab8b-6bc286283761 rdf:type skos:Concept;
  skos:scopeNote """Use for official residences, frequently large and impressively appointed, of sovereigns or other high dignitaries; for other large stately dwellings but not official residences, use 'mansions.' """@en;
  skos:exactMatch aat:300005734;
  skos:altLabel "palast"@de;
  skos:altLabel "palace"@en;
  skos:altLabel "palais"@fr;
  skos:altLabel "paleis"@nl;
  skos:inScheme dccd:objectElementType.
dccd:a7a28134-6b80-11e5-ab8c-3f0457a8e4dd rdf:type skos:Concept;
  skos:scopeNote """Barriers composed of long stakes, usually with pointed tops, driven into the earth close together, sometimes connected by horizontal beams """@en;
  skos:exactMatch aat:300003717;
  skos:altLabel "palisade"@de;
  skos:altLabel "palisade"@en;
  skos:altLabel "palissade"@fr;
  skos:altLabel "palissade"@nl;
  skos:inScheme dccd:objectElementType.
dccd:a7a281de-6b80-11e5-ab8d-1b18cbbaafc5 rdf:type skos:Concept;
  skos:exactMatch aat:300212606;
  skos:altLabel "kriegsschiff"@de;
  skos:altLabel "warship"@en;
  skos:altLabel "navire de querre"@fr;
  skos:altLabel "oorlogsschip"@nl;
  skos:narrower dccd:a7a1ba74-6b80-11e5-aa7a-7b1dc4c873b5;
  skos:inScheme dccd:objectElementType.
dccd:a7a28328-6b80-11e5-ab8f-bf21795005df rdf:type skos:Concept;
  skos:scopeNote """The residences provided for clergymen, usually parsons/vicars """@en;
  skos:exactMatch aat:300005650;
  skos:altLabel "presbytère"@fr;
  skos:altLabel "pfarrhaus"@de;
  skos:altLabel "vicarage"@en;
  skos:altLabel "cure"@fr;
  skos:altLabel "pastorie"@nl;
  skos:inScheme dccd:objectElementType.
dccd:a7a283d2-6b80-11e5-ab90-f712f9ff8d3d rdf:type skos:Concept;
  skos:scopeNote """shipsterm """@en;
  skos:exactMatch aat:300213080;
  skos:altLabel "paddel"@de;
  skos:altLabel "paddle"@en;
  skos:altLabel "pagaie"@fr;
  skos:altLabel "peddel"@nl;
  skos:inScheme dccd:objectElementType.
dccd:a7a28472-6b80-11e5-ab91-17072903c8e8 rdf:type skos:Concept;
  skos:exactMatch aat:300010262;
  skos:altLabel "platte"@de;
  skos:altLabel "plaque"@en;
  skos:altLabel "plate"@fr;
  skos:altLabel "plaat"@nl;
  skos:inScheme dccd:objectElementType.
dccd:a7a2851c-6b80-11e5-ab92-17a3c6e09055 rdf:type skos:Concept;
  skos:scopeNote """The overhead surfaces of interior spaces, sometimes constructed to mask building systems or structural elements """@en;
  skos:exactMatch aat:300002031;
  skos:altLabel "decke"@de;
  skos:altLabel "ceiling"@en;
  skos:altLabel "plafond"@fr;
  skos:altLabel "plafond"@nl;
  skos:inScheme dccd:objectElementType.
dccd:a7a285bc-6b80-11e5-ab93-97ea9bfe9e3c rdf:type skos:Concept;
  skos:scopeNote """Long, wide, square-sawn thick piece of wood; Thin, flat, rigid objects, of considerable length or breadth compared to thickness, most often of wood, paperboard, or composite fiber materials. shipsterm """@en;
  skos:exactMatch aat:300126969;
  skos:altLabel "board"@en;
  skos:altLabel "brett"@de;
  skos:altLabel "plank"@en;
  skos:altLabel "planche"@fr;
  skos:altLabel "plank"@nl;
  skos:inScheme dccd:objectElementType.
dccd:a7a28666-6b80-11e5-ab94-ef208231c551 rdf:type skos:Concept;
  skos:scopeNote """Passages through fences or walls separating two exterior spaces, or the structures or ornamental constructions enclosing such passages; (Portal) Use for impressive, monumental entrances, gateways, or doorways usually to buildings or courtyards, especially those emphasized by stately architectural treatment"""@en;
  skos:exactMatch aat:300069189;
  skos:altLabel "tor"@de;
  skos:altLabel "gateway"@en;
  skos:altLabel "porte"@fr;
  skos:altLabel "poort"@nl;
  skos:inScheme dccd:objectElementType.
dccd:a7a28710-6b80-11e5-ab95-57acef8170ff rdf:type skos:Concept;
  skos:scopeNote """Use for structures at, near, or over entrance gateways, usually containing a gatekeeper's dwelling. For subordinate buildings on the grounds of estates or parks used as the dwellings of employees, such as gatekeepers, but not located at entranceways, prefer 'lodges (caretakers' houses).'"""@en;
  skos:exactMatch aat:300005621;
  skos:altLabel "torbau"@de;
  skos:altLabel "gatehouse"@en;
  skos:altLabel "guérite"@fr;
  skos:altLabel "poortgebouw"@nl;
  skos:inScheme dccd:objectElementType.
dccd:a7a287ba-6b80-11e5-ab96-d3e8d3934350 rdf:type skos:Concept;
  skos:scopeNote """Use for miniature scale houses or sets of rooms designed to hold or display miniature furniture and furnishings and usually to be used in conjunction with like-sized dolls; known since the 16th century """@en;
  skos:exactMatch aat:300136025;
  skos:altLabel "puppenhaus"@de;
  skos:altLabel "dollhouse"@en;
  skos:altLabel "maison de poupée"@fr;
  skos:altLabel "poppenhuis"@nl;
  skos:inScheme dccd:objectElementType.
dccd:a7a28904-6b80-11e5-ab98-cbd964da20b9 rdf:type skos:Concept;
  skos:scopeNote """Stands for a speaker, especially the preacher of a sermon """@en;
  skos:exactMatch aat:300003790;
  skos:altLabel "kanzel"@de;
  skos:altLabel "pulpit"@en;
  skos:altLabel "chaire à prêcher"@fr;
  skos:altLabel "preekstoel"@nl;
  skos:inScheme dccd:objectElementType.
dccd:a7a28a4e-6b80-11e5-ab9a-9342a386dc36 rdf:type skos:Concept;
  skos:exactMatch aat:300024976;
  skos:altLabel "wagenrad"@de;
  skos:altLabel "rad"@de;
  skos:altLabel "wheel"@en;
  skos:altLabel "roue"@fr;
  skos:altLabel "wiel"@nl;
  skos:inScheme dccd:objectElementType.
dccd:a7a28ba2-6b80-11e5-ab9c-5f9eed2dbfb9 rdf:type skos:Concept;
  skos:scopeNote """Use for the dining halls of monasteries or other religious institutions """@en;
  skos:exactMatch aat:300004347;
  skos:altLabel "refektorium"@de;
  skos:altLabel "refectory"@en;
  skos:altLabel "réfectoire"@fr;
  skos:altLabel "refectorium"@nl;
  skos:inScheme dccd:objectElementType.
dccd:a7a28cec-6b80-11e5-ab9e-3f07ebd3a8c3 rdf:type skos:Concept;
  skos:scopeNote """Use for images, especially pictorial compositions, executed in relief """@en;
  skos:exactMatch aat:300047230;
  skos:altLabel "relief"@de;
  skos:altLabel "relief"@en;
  skos:altLabel "relief"@fr;
  skos:altLabel "reliëf"@nl;
  skos:inScheme dccd:objectElementType.
dccd:a7a28d8c-6b80-11e5-ab9f-335ee90cfd84 rdf:type skos:Concept;
  skos:scopeNote """Use for painted or sculpted panels attached at the back of a Christian altar's mensa. For the Mexican and Spanish American paintings of Christian saints and other holy figures from Roman Catholicism, use 'retablos.' """@en;
  skos:exactMatch aat:300075940;
  skos:altLabel "altarbild"@de;
  skos:altLabel "altar piece"@en;
  skos:altLabel "retable"@fr;
  skos:altLabel "retabel"@nl;
  skos:inScheme dccd:objectElementType.
dccd:a7a28e36-6b80-11e5-aba0-839ba2ddbd34 rdf:type skos:Concept;
  skos:exactMatch aat:300079019;
  skos:altLabel "deckwerk"@de;
  skos:altLabel "revetment"@en;
  skos:altLabel "revêtement"@fr;
  skos:altLabel "dijkbeslag"@nl;
  skos:inScheme dccd:objectElementType.
dccd:a7a28f76-6b80-11e5-aba2-4bd79c1a7610 rdf:type skos:Concept;
  skos:scopeNote """Use for long slender shafts, usually wood, shaped to a round handle or grip at one end and flat-tipped blade at the other; for rowing. For similar but shorter devices with round-tipped blades for propelling small boats, use 'paddles (watercraft equipment).'
shipsterm"""@en;
  skos:exactMatch aat:300213077;
  skos:altLabel "riemen"@de;
  skos:altLabel "aviron"@fr;
  skos:altLabel "riem"@nl;
  skos:altLabel "roeiriem"@nl;
  skos:altLabel "ruder"@de;
  skos:altLabel "oar"@en;
  skos:altLabel "rame"@fr;
  skos:altLabel "roeispaan"@nl;
  skos:inScheme dccd:objectElementType.
dccd:a7a29020-6b80-11e5-aba3-db1826e02d86 rdf:type skos:Concept;
  skos:scopeNote """shipsterm """@en;
  skos:exactMatch aat:300212841;
  skos:altLabel "ruder"@de;
  skos:altLabel "rudder"@en;
  skos:altLabel "gouvernail"@fr;
  skos:altLabel "roer"@nl;
  skos:inScheme dccd:objectElementType.
dccd:a7a290ca-6b80-11e5-aba4-9b5bfadc261a rdf:type skos:Concept;
  skos:scopeNote """Designates Roman villas serving agricultural purposes """@en;
  skos:exactMatch aat:300005518;
  skos:altLabel "Romische villa (rustica)"@de;
  skos:altLabel "Roman villa (rustica)"@en;
  skos:altLabel "villa Romaine (rustica)"@fr;
  skos:altLabel "romeinse villa (rustica)"@nl;
  skos:inScheme dccd:objectElementType.
dccd:a7a2939a-6b80-11e5-aba5-67a9c77e0515 rdf:type skos:Concept;
  skos:scopeNote """shipsterm """@en;
  skos:exactMatch aat:300213040;
  skos:altLabel "schiffsrumpf"@de;
  skos:altLabel "hull"@en;
  skos:altLabel "coque"@fr;
  skos:altLabel "scheepsromp"@nl;
  skos:inScheme dccd:objectElementType.
dccd:a7a29462-6b80-11e5-aba6-479824864dcb rdf:type skos:Concept;
  skos:scopeNote """shipsterm """@en;
  skos:exactMatch aat:300012784;
  skos:altLabel "rundholz"@de;
  skos:altLabel "log"@en;
  skos:altLabel "grume"@fr;
  skos:altLabel "rondhout"@nl;
  skos:inScheme dccd:objectElementType.
dccd:a7a2950c-6b80-11e5-aba7-6305061c8f37 rdf:type skos:Concept;
  skos:exactMatch aat:300042973;
  skos:altLabel "schüssel"@de;
  skos:altLabel "coupe"@fr;
  skos:altLabel "schale"@de;
  skos:altLabel "dish"@en;
  skos:altLabel "plat"@fr;
  skos:altLabel "schaal"@nl;
  skos:inScheme dccd:objectElementType.
dccd:a7a295b6-6b80-11e5-aba8-af39f5fa29c5 rdf:type skos:Concept;
  skos:scopeNote """The structures inclined toward the water on which a ship may be built or lowered into the water; may also be used for the guides that support the ship's hull """@en;
  skos:exactMatch aat:300006433;
  skos:altLabel "schiffwerft"@de;
  skos:altLabel "slipway"@en;
  skos:altLabel "cale de carénage"@fr;
  skos:altLabel "scheepshelling"@nl;
  skos:inScheme dccd:objectElementType.
dccd:a7a2970a-6b80-11e5-abaa-3755b50cf3ef rdf:type skos:Concept;
  skos:scopeNote """Places or enclosures where boats or ships are built or repaired """@en;
  skos:exactMatch aat:300000403;
  skos:altLabel "schiffswerft"@de;
  skos:altLabel "shipyard"@en;
  skos:altLabel "chantier naval"@fr;
  skos:altLabel "scheepswerf"@nl;
  skos:inScheme dccd:objectElementType.
dccd:a7a297aa-6b80-11e5-abab-ef549e0d00c9 rdf:type skos:Concept;
  skos:scopeNote """Wood in the form of broad, thin, flat or sometimes curved pieces as, for example, in polyptychs, doors, and plywood construction"""@en;
  skos:exactMatch aat:300014657;
  skos:altLabel "täfelung"@de;
  skos:altLabel "panel"@en;
  skos:altLabel "panneau"@fr;
  skos:altLabel "paneel"@nl;
  skos:inScheme dccd:objectElementType.
dccd:a7a29854-6b80-11e5-abac-a3ffe44283cb rdf:type skos:Concept;
  skos:scopeNote """Use both for the parts of buildings that project outward from the rest, especially common as corner, central, or terminal features in French architecture, and for the detached or semidetached units into which a building (as a hospital) is sometimes divided"""@en;
  skos:exactMatch aat:300002660;
  skos:altLabel "pavillon"@de;
  skos:altLabel "pavillion"@en;
  skos:altLabel "pavillon"@fr;
  skos:altLabel "paviljoen"@nl;
  skos:inScheme dccd:objectElementType.
dccd:a7a298fe-6b80-11e5-abad-b3623830f445 rdf:type skos:Concept;
  skos:scopeNote """Arched rppf truss made of two or more overlapping layers of curved boards or planks.  The French Philivert de l'Orme can be considered to be its inventor."""@en;
  skos:narrower aat:300002098;
  skos:altLabel "bohlenbinder"@de;
  skos:altLabel "Philibert Delorme roof"@en;
  skos:altLabel "charpente à la Philibert-Delorme"@fr;
  skos:altLabel "philibertspant"@nl;
  skos:inScheme dccd:objectElementType.
dccd:a7a299a8-6b80-11e5-abae-0bbe844336cd rdf:type skos:Concept;
  skos:scopeNote """Flat surfaces, blocks, or floors, generally raised above the adjoining floor."""@en;
  skos:exactMatch aat:300132129;
  skos:altLabel "plattform"@de;
  skos:altLabel "platform"@en;
  skos:altLabel "estrade"@fr;
  skos:altLabel "platform"@nl;
  skos:inScheme dccd:objectElementType.
dccd:a7a29a52-6b80-11e5-abaf-937d30e962ce rdf:type skos:Concept;
  skos:scopeNote """Open structure with a movable roof for storing loose hay on a farm"""@en;
  skos:narrower aat:300004895;
  skos:altLabel "rutenberg"@de;
  skos:altLabel "hay barrack"@en;
  skos:altLabel "hooiberg (bâtiment agricole des Pays-Bas utilisé pour le stockage du grain)"@fr;
  skos:altLabel "hooiberg"@nl;
  skos:inScheme dccd:objectElementType.
dccd:a7a29af2-6b80-11e5-abb0-bb92e9e3115e rdf:type skos:Concept;
  skos:scopeNote """Flat-bottomed boat with a square-cut bow, designed for use in small rivers or other shallow water."""@en;
  skos:narrower aat:300232951;
  skos:altLabel "pünte"@de;
  skos:altLabel "punt"@en;
  skos:altLabel "plate"@fr;
  skos:altLabel "punter"@nl;
  skos:inScheme dccd:objectElementType.
dccd:a7a29c5a-6b80-11e5-abb2-4ff0ed7338ae rdf:type skos:Concept;
  skos:exactMatch aat:300036869;
  skos:altLabel "buckler"@en;
  skos:altLabel "schild"@de;
  skos:altLabel "shield"@en;
  skos:altLabel "bouclier"@fr;
  skos:altLabel "schild"@nl;
  skos:inScheme dccd:objectElementType.
dccd:a7a29d04-6b80-11e5-abb3-ab8e57f3d3bb rdf:type skos:Concept;
  skos:scopeNote """Use for unique works in which images are formed primarily by the direct application of pigments suspended in oil, water, egg yolk, molten wax, or other liquid, arranged in masses of color, onto a generally two-dimensional surface """@en;
  skos:exactMatch aat:300033618;
  skos:altLabel "gemälde"@de;
  skos:altLabel "painting"@en;
  skos:altLabel "peinture"@fr;
  skos:altLabel "schilderij"@nl;
  skos:inScheme dccd:objectElementType.
dccd:a7a29dae-6b80-11e5-abb4-174609336039 rdf:type skos:Concept;
  skos:scopeNote """Individual buildings or groups of buildings designed or used as places of instruction """@en;
  skos:exactMatch aat:300006495;
  skos:altLabel "school building"@en;
  skos:altLabel "école"@fr;
  skos:altLabel "schulgebäude"@de;
  skos:altLabel "schoolgebouw"@nl;
  skos:altLabel "school"@en;
  skos:altLabel "bâtiment scolaire"@fr;
  skos:inScheme dccd:objectElementType.
dccd:a7a29e58-6b80-11e5-abb5-5feae86e5bc9 rdf:type skos:Concept;
  skos:scopeNote """Agricultural buildings with large, usually sliding doors, prominent roofs, and predominantly open spaces on the interior, primarily used as storage buildings for hay, grains, and farm equipment and shelters for livestock; does not include those structures, often termed barns, used for the processing of food and other agricultural produce, such as hop barns and tobacco barns"""@en;
  skos:exactMatch aat:300004900;
  skos:altLabel "stadel"@de;
  skos:altLabel "scheune"@de;
  skos:altLabel "barn"@en;
  skos:altLabel "grange"@fr;
  skos:altLabel "schuur"@nl;
  skos:inScheme dccd:objectElementType.
dccd:a7a2a056-6b80-11e5-abb8-73d4c2a47abf rdf:type skos:Concept;
  skos:scopeNote """Artificial passages for water, fitted with a valve or gate for stopping or regulating the flow """@en;
  skos:exactMatch aat:300006082;
  skos:altLabel "lock"@en;
  skos:altLabel "schleuse"@de;
  skos:altLabel "sluice"@en;
  skos:altLabel "écluse"@fr;
  skos:altLabel "sluis"@nl;
  skos:inScheme dccd:objectElementType.
dccd:a7a2a0f6-6b80-11e5-abb9-4f73d1cc241c rdf:type skos:Concept;
  skos:exactMatch aat:300024300;
  skos:altLabel "schaufel"@de;
  skos:altLabel "shovel"@en;
  skos:altLabel "pelle"@fr;
  skos:altLabel "schop"@nl;
  skos:inScheme dccd:objectElementType.
dccd:a7a2a24a-6b80-11e5-abbb-c37499110f0f rdf:type skos:Concept;
  skos:exactMatch aat:300211037;
  skos:altLabel "spielzeug"@de;
  skos:altLabel "jouet"@fr;
  skos:altLabel "speelgoed"@nl;
  skos:altLabel "toy"@en;
  skos:inScheme dccd:objectElementType.
dccd:a7a2a2ea-6b80-11e5-abbc-b33c0bfe4663 rdf:type skos:Concept;
  skos:scopeNote """Stairs whose tapered treads wind around, and engage in, a solid, central newel; Staircases that are circular in plan, consisting entirely of winders or wedge-shaped steps """@en;
  skos:exactMatch aat:300003243;
  skos:altLabel "newel-post stair"@en;
  skos:altLabel "solid newel stair"@en;
  skos:altLabel "escalier à noyeau"@fr;
  skos:altLabel "spindeltreppe"@de;
  skos:altLabel "spiral staircase"@en;
  skos:altLabel "escalier à vis"@fr;
  skos:altLabel "spiltrap"@nl;
  skos:inScheme dccd:objectElementType.
dccd:a7a2a43e-6b80-11e5-abbe-33cf5627f9a6 rdf:type skos:Concept;
  skos:scopeNote """Distinctions among villages, towns, and cities are relative and vary according to their individual regional contexts. Generally, cities designate large or important communities with population, status, and internal complexity greater than most towns in the region."""@en;
  skos:exactMatch aat:300008375;
  skos:altLabel "city"@en;
  skos:altLabel "stadt"@de;
  skos:altLabel "town"@en;
  skos:altLabel "ville"@fr;
  skos:altLabel "stad"@nl;
  skos:inScheme dccd:objectElementType.
dccd:a7a2a4e8-6b80-11e5-abbf-3fad96516361 rdf:type skos:Concept;
  skos:scopeNote """Use for the principal public administration buildings of towns and villages housing offices for transaction of government business and places for public assembly """@en;
  skos:exactMatch aat:300006063;
  skos:altLabel "stadhaus"@de;
  skos:altLabel "city hall"@en;
  skos:altLabel "rathaus"@de;
  skos:altLabel "town hall"@en;
  skos:altLabel "hötel de ville"@fr;
  skos:altLabel "stadhuis"@nl;
  skos:inScheme dccd:objectElementType.
dccd:a7a2a592-6b80-11e5-abc0-2b73c7d752c7 rdf:type skos:Concept;
  skos:scopeNote """Fortification walls of cities """@en;
  skos:exactMatch aat:300005072;
  skos:altLabel "stadtmauer"@de;
  skos:altLabel "city wall"@en;
  skos:altLabel "enceinte de ville"@fr;
  skos:altLabel "stadsmuur"@nl;
  skos:inScheme dccd:objectElementType.
dccd:a7a2a664-6b80-11e5-abc1-8737c248c661 rdf:type skos:Concept;
  skos:scopeNote """Buildings or portions of buildings for the housing and feeding of horses, cattle, and other such domestic animals, and often also for storing riding equipment and vehicles, and which occasionally have living quarters for associated personnel. For barnlike structures used primarily for housing farmstock and feed, use, for example, 'horse barns' or 'cattle barns.'"""@en;
  skos:exactMatch aat:300005015;
  skos:altLabel "stalle"@de;
  skos:altLabel "stable"@en;
  skos:altLabel "écurie"@fr;
  skos:altLabel "stal"@nl;
  skos:inScheme dccd:objectElementType.
dccd:a7a2a70e-6b80-11e5-abc2-3fd4bc6d6f38 rdf:type skos:Concept;
  skos:exactMatch aat:300006155;
  skos:altLabel "steg"@de;
  skos:altLabel "jetty"@en;
  skos:altLabel "appontement"@fr;
  skos:altLabel "steiger"@nl;
  skos:inScheme dccd:objectElementType.
dccd:a7a2a7ae-6b80-11e5-abc3-17e8cf913e19 rdf:type skos:Concept;
  skos:scopeNote """Pierlike masonry elements built to strengthen or support walls or resist the lateral thrust of vaults """@en;
  skos:exactMatch aat:300000891;
  skos:altLabel "mauerstrebe"@de;
  skos:altLabel "buttress"@en;
  skos:altLabel "contrefort"@fr;
  skos:altLabel "steunbeer"@nl;
  skos:inScheme dccd:objectElementType.
dccd:a7a2aab0-6b80-11e5-abc7-53d5d4ab51f8 rdf:type skos:Concept;
  skos:scopeNote """Seats for one person with a back or a back and arms. Distinct from 'stools' which have no back. """@en;
  skos:exactMatch aat:300037772;
  skos:altLabel "stuhl"@de;
  skos:altLabel "chair"@en;
  skos:altLabel "chaise"@fr;
  skos:altLabel "stoel"@nl;
  skos:inScheme dccd:objectElementType.
dccd:a7a2abc8-6b80-11e5-abc8-a3f29716528e rdf:type skos:Concept;
  skos:scopeNote """Use for openings or recesses in chimneys or walls in which fires may be built, as for heating or cooking; may also refer to low fireproof structures erected outdoors for cooking over open flames """@en;
  skos:exactMatch aat:300052267;
  skos:altLabel "herd"@de;
  skos:altLabel "hearth"@en;
  skos:altLabel "feuerstelle"@de;
  skos:altLabel "fireplace"@en;
  skos:altLabel "foyer"@fr;
  skos:altLabel "stookplaats"@nl;
  skos:inScheme dccd:objectElementType.
dccd:a7a2ae02-6b80-11e5-abcb-376f41674327 rdf:type skos:Concept;
  skos:exactMatch aat:300007590;
  skos:altLabel "synagoge"@de;
  skos:altLabel "synagogue"@en;
  skos:altLabel "synagogue"@fr;
  skos:altLabel "synagoge"@nl;
  skos:inScheme dccd:objectElementType.
dccd:a7a2aeac-6b80-11e5-abcc-9f4a262ef628 rdf:type skos:Concept;
  skos:scopeNote """Articles of furniture consisting of a flat, slablike top supported on one or more legs or supports """@en;
  skos:exactMatch aat:300039548;
  skos:altLabel "tisch"@de;
  skos:altLabel "table"@en;
  skos:altLabel "table"@fr;
  skos:altLabel "tafel"@nl;
  skos:inScheme dccd:objectElementType.
dccd:a7a2b1b8-6b80-11e5-abcd-6bbbe3957081 rdf:type skos:Concept;
  skos:scopeNote """Refers to places devoted to the worship of a deity or deities. In the strictest sense, it refers to the dwelling place of a deity, and thus often houses a cult image. In modern usage a temple is generally a structure, but it was originally derived from the Latin 'templum' and historically has referred to an uncovered place affording a view of the surrounding region. For Christian or Islamic religious buildings the terms 'churches' or 'mosques' are generally used, but an exception is that 'temples' is used for Protestant, as opposed to Roman Catholic, places of worship in France and some French-speaking regions"""@en;
  skos:exactMatch aat:300007595;
  skos:altLabel "tempel"@de;
  skos:altLabel "temple"@en;
  skos:altLabel "temple"@fr;
  skos:altLabel "tempel"@nl;
  skos:inScheme dccd:objectElementType.
dccd:a7a2b28a-6b80-11e5-abce-63fa6a297629 rdf:type skos:Concept;
  skos:scopeNote """Roofs which rise to a peak or ridge by inclined planes on all, usually four, sides, therefore requiring hip rafters."""@en;
  skos:exactMatch aat:300002147;
  skos:altLabel "walmdach"@de;
  skos:altLabel "toit à croupes"@fr;
  skos:altLabel "schilddak"@nl;
  skos:altLabel "hip roof"@en;
  skos:altLabel "hipped roof"@en;
  skos:altLabel "walmdak"@nl;
  skos:altLabel "wolfdak"@nl;
  skos:inScheme dccd:objectElementType.
dccd:a7a2b334-6b80-11e5-abcf-1fad00f6e162 rdf:type skos:Concept;
  skos:narrower aat:300024617;
  skos:altLabel "schaufelrad"@de;
  skos:altLabel "paddle wheel"@en;
  skos:altLabel "roue à aubes"@fr;
  skos:altLabel "schoepenrad"@nl;
  skos:inScheme dccd:objectElementType.
dccd:a7a2b5dc-6b80-11e5-abd3-e3bae058fc38 rdf:type skos:Concept;
  skos:scopeNote """Roof structure whose load-bearing rafters are the most important elements.  Their side pressure can be absorbed in different ways."""@en;
  skos:narrower aat:300002098;
  skos:altLabel "sparrendach"@de;
  skos:altLabel "common rafter roof"@en;
  skos:altLabel "charpente à chevrons"@fr;
  skos:altLabel "sporenkap"@nl;
  skos:inScheme dccd:objectElementType.
dccd:a7a2b686-6b80-11e5-abd4-e3a107f963ff rdf:type skos:Concept;
  skos:scopeNote """Mill with a tower supported by struts"""@en;
  skos:narrower aat:300006273;
  skos:altLabel "galerieholländer"@de;
  skos:altLabel "tower mill"@en;
  skos:altLabel "moulin à galerie"@fr;
  skos:altLabel "stellingmolen"@nl;
  skos:inScheme dccd:objectElementType.
dccd:a7a2b730-6b80-11e5-abd5-230ca0274fb1 rdf:type skos:Concept;
  skos:scopeNote """Artificial passages of wood or masonry, a dam or embankment, used for impounding the water of river, stream, or canal, and fitted with a valve or gate for stopping or regulating the flow."""@en;
  skos:exactMatch aat:300006082;
  skos:altLabel "outlet sluice"@en;
  skos:altLabel "siel"@de;
  skos:altLabel "drainage sluice"@en;
  skos:altLabel "spuisluis"@nl;
  skos:altLabel "écluse"@fr;
  skos:inScheme dccd:objectElementType.
dccd:a7a2b884-6b80-11e5-abd7-5349e90beb55 rdf:type skos:Concept;
  skos:scopeNote """Short vertical member in a common rafter roof, rarely in trasverse frames of a purlin roof."""@en;
  skos:narrower aat:300002450;
  skos:altLabel "sparrenknecht"@de;
  skos:altLabel "ashlar piece"@en;
  skos:altLabel "potelet"@fr;
  skos:altLabel "standzoon"@nl;
  skos:altLabel "ashlar post"@en;
  skos:altLabel "voetschoor"@nl;
  skos:inScheme dccd:objectElementType.
dccd:a7a2ba78-6b80-11e5-abda-7f85f79c435a rdf:type skos:Concept;
  skos:scopeNote """Wheels used as the primary means of maneuvering vehicles."""@en;
  skos:exactMatch aat:300212892;
  skos:altLabel "steuerrad"@de;
  skos:altLabel "steering wheel"@en;
  skos:altLabel "roue de gouvernail"@fr;
  skos:altLabel "stuurwiel"@nl;
  skos:inScheme dccd:objectElementType.
dccd:a7a2bb22-6b80-11e5-abdb-57403151de1c rdf:type skos:Concept;
  skos:scopeNote """Leg of a table"""@en;
  skos:narrower aat:300039548;
  skos:altLabel "tischbein"@de;
  skos:altLabel "table leg"@en;
  skos:altLabel "pied de table"@fr;
  skos:altLabel "tafelpoot"@nl;
  skos:inScheme dccd:objectElementType.
dccd:a7a2bbd6-6b80-11e5-abdc-9b09981608e9 rdf:type skos:Concept;
  skos:scopeNote """Use for tall structures that are at least roughly pyramidal, polygonal, or conical and that rise from towers or roofs """@en;
  skos:exactMatch aat:300003615;
  skos:closeMatch aat:300004847;
  skos:altLabel "turm"@de;
  skos:altLabel "tower"@en;
  skos:altLabel "tour"@fr;
  skos:altLabel "toren"@nl;
  skos:inScheme dccd:objectElementType.
dccd:a7a2bc80-6b80-11e5-abdd-cb5d31bf2950 rdf:type skos:Concept;
  skos:exactMatch aat:300002360;
  skos:altLabel "turmspitze"@de;
  skos:altLabel "spire"@en;
  skos:altLabel "flèche"@fr;
  skos:altLabel "torenspits"@nl;
  skos:inScheme dccd:objectElementType.
dccd:a7a2bd2a-6b80-11e5-abde-dbc036c4f7fc rdf:type skos:Concept;
  skos:exactMatch aat:300003228;
  skos:altLabel "staircase"@en;
  skos:altLabel "treppe"@de;
  skos:altLabel "stairs"@en;
  skos:altLabel "escaliers"@fr;
  skos:altLabel "trap"@nl;
  skos:inScheme dccd:objectElementType.
dccd:a7a2bdd4-6b80-11e5-abdf-4b8727f4114f rdf:type skos:Concept;
  skos:scopeNote """Stair units that consist of one tread and one riser, or any similar element providing a horizontal surface on which to support the foot of a person descending or ascending; The horizontal parts of steps"""@en;
  skos:exactMatch aat:300003312;
  skos:altLabel "giron"@fr;
  skos:altLabel "stair"@en;
  skos:altLabel "tread"@en;
  skos:altLabel "treppenstufe"@de;
  skos:altLabel "step"@en;
  skos:altLabel "marche d'escalier"@fr;
  skos:altLabel "traptrede"@nl;
  skos:inScheme dccd:objectElementType.
dccd:a7a2be74-6b80-11e5-abe0-7793fcbf4177 rdf:type skos:Concept;
  skos:exactMatch aat:300178749;
  skos:altLabel "boat"@en;
  skos:altLabel "boot"@nl;
  skos:altLabel "bateau"@fr;
  skos:altLabel "boot"@de;
  skos:inScheme dccd:objectElementType.
dccd:a7a2bf1e-6b80-11e5-abe1-ef397b44811b rdf:type skos:Concept;
  skos:scopeNote """Stringed instrument of the violin family.  Tuned a 5th lower than a true violin"""@en;
  skos:exactMatch aat:300042225;
  skos:altLabel "viola"@en;
  skos:altLabel "altviool"@nl;
  skos:altLabel "viola"@de;
  skos:altLabel "alto"@fr;
  skos:inScheme dccd:objectElementType.
dccd:a7a2bfbe-6b80-11e5-abe2-cbd88e5cbc94 rdf:type skos:Concept;
  skos:scopeNote """Use for watercraft generally larger and more seaworthy than boats; usually propelled by sails or engines"""@en;
  skos:exactMatch aat:300082981;
  skos:altLabel "schiff"@de;
  skos:altLabel "ship"@en;
  skos:altLabel "bateau"@fr;
  skos:altLabel "schip"@nl;
  skos:narrower dccd:a7a1ba74-6b80-11e5-aa7a-7b1dc4c873b5;
  skos:inScheme dccd:objectElementType.
dccd:a7a2c068-6b80-11e5-abe3-173c576ad20e rdf:type skos:Concept;
  skos:scopeNote """Refers broadly to devices or contrivances by which people, animals, or objects are conveyed or carried."""@en;
  skos:exactMatch aat:300219258;
  skos:altLabel "vehicle"@en;
  skos:altLabel "véhicule"@fr;
  skos:altLabel "fahrzeug"@de;
  skos:altLabel "voertuig"@nl;
  skos:inScheme dccd:objectElementType.
dccd:a7a2c112-6b80-11e5-abe4-e3f2fbd024f6 rdf:type skos:Concept;
  skos:scopeNote """The surfaces of rooms or spaces on which one walks"""@en;
  skos:exactMatch aat:300002060;
  skos:altLabel "floor"@en;
  skos:altLabel "vloer"@nl;
  skos:altLabel "sol"@fr;
  skos:altLabel "fußboden"@de;
  skos:inScheme dccd:objectElementType.
dccd:a7a2c25c-6b80-11e5-abe6-cf08b09f60f2 rdf:type skos:Concept;
  skos:scopeNote """Designates independent and canonically erected monasteries, ruled by an abbot if occupied by monks and by an abbess if occupied by nuns """@en;
  skos:exactMatch aat:300000642;
  skos:altLabel "abtei"@de;
  skos:altLabel "abbey"@en;
  skos:altLabel "abbaye"@fr;
  skos:altLabel "abdij"@nl;
  skos:inScheme dccd:objectElementType.
dccd:a7a2c306-6b80-11e5-abe7-7fea5db06107 rdf:type skos:Concept;
  skos:scopeNote """Use for watercraft designed primarily to transport cargo """@en;
  skos:exactMatch aat:300212694;
  skos:altLabel "freighter"@en;
  skos:altLabel "vrachtschip"@nl;
  skos:altLabel "frachtschiff"@de;
  skos:altLabel "lastschiff"@de;
  skos:altLabel "cargo vessel"@en;
  skos:altLabel "frachter"@de;
  skos:altLabel "cargo"@fr;
  skos:inScheme dccd:objectElementType.
dccd:a7a2c4fa-6b80-11e5-abea-0b5625eff428 rdf:type skos:Concept;
  skos:scopeNote """Passages or rooms just inside the entrance of a residence, but sometimes with a vestibule between it and the outdoors. Prefer 'lobbies' for such spaces in larger public buildings."""@en;
  skos:exactMatch aat:300004263;
  skos:altLabel "entrance hall"@en;
  skos:altLabel "flur"@de;
  skos:altLabel "hall d'entrée"@fr;
  skos:altLabel "entreehal"@nl;
  skos:inScheme dccd:objectElementType.
dccd:a7a2c5a4-6b80-11e5-abeb-5f2542d3673a rdf:type skos:Concept;
  skos:scopeNote """Rooms or closets in which food, groceries, and other provisions, or silverware, dishes, and other items are kept."""@en;
  skos:exactMatch aat:300004499;
  skos:altLabel "provisiekamer"@nl;
  skos:altLabel "voorraadkamer"@nl;
  skos:altLabel "pantry"@en;
  skos:altLabel "garde-manger"@fr;
  skos:altLabel "speisekammer"@de;
  skos:inScheme dccd:objectElementType.
dccd:a7a2c644-6b80-11e5-abec-33b88023131e rdf:type skos:Concept;
  skos:scopeNote """A pair of small oars used by a single rower"""@en;
  skos:narrower aat:300213077;
  skos:altLabel "scull"@en;
  skos:altLabel "skull"@de;
  skos:altLabel "godille"@fr;
  skos:altLabel "wrikriem"@nl;
  skos:inScheme dccd:objectElementType.
dccd:a7a2c6ee-6b80-11e5-abed-bb1ab0b1dad9 rdf:type skos:Concept;
  skos:scopeNote """General term referring to all long outdoor passages used by and generally created by humans, intended to allow people to pass between different places, usually one wide enough to admit of the passage of wheeled vehicles, horses, or travellers on foot."""@en;
  skos:exactMatch aat:300008217;
  skos:altLabel "way"@en;
  skos:altLabel "chemin"@fr;
  skos:altLabel "road"@en;
  skos:altLabel "weg"@nl;
  skos:altLabel "route"@fr;
  skos:altLabel "straße"@de;
  skos:altLabel "weg"@de;
  skos:inScheme dccd:objectElementType.
dccd:a7a2c798-6b80-11e5-abee-07164408d7de rdf:type skos:Concept;
  skos:scopeNote """Rigid sheaths made of wood, metal, or leather, used to enclose and carry edged weapons or tools, or hand weapons such as carbines and rifles."""@en;
  skos:exactMatch aat:300037139;
  skos:altLabel "scabbard"@en;
  skos:altLabel "fourreau"@fr;
  skos:altLabel "schede"@nl;
  skos:altLabel "schwertscheide"@de;
  skos:altLabel "sheath"@en;
  skos:inScheme dccd:objectElementType.
dccd:a7a2c842-6b80-11e5-abef-5f1fbac074f8 rdf:type skos:Concept;
  skos:scopeNote """Use generally for rooms large in proportion to rooms for domestic functions, circulation, or storage; use also for the principal rooms of a Medieval house and for large central rooms in certain 19th- and 20th-century English and American houses. """@en;
  skos:exactMatch aat:300004441;
  skos:altLabel "parlour"@en;
  skos:altLabel "hall"@en;
  skos:altLabel "best room"@en;
  skos:altLabel "sejour"@fr;
  skos:altLabel "pronkkamer"@nl;
  skos:altLabel "beste Stube"@de;
  skos:inScheme dccd:objectElementType.
dccd:a7a2ca36-6b80-11e5-abf2-9bda48c69379 rdf:type skos:Concept;
  skos:scopeNote """Material derived from or comprising roots, which are parts of a plant that develop, growing typically from the radicle and downward into the soil."""@en;
  skos:exactMatch aat:300081475;
  skos:altLabel "wurzelwerk"@de;
  skos:altLabel "racines"@fr;
  skos:altLabel "wortelstelsel"@nl;
  skos:altLabel "roots"@en;
  skos:inScheme dccd:objectElementType.
dccd:a7a2d580-6b80-11e5-abff-c7cea56e4e4a rdf:type skos:Concept;
  skos:scopeNote """Buildings that house facilities for the housing and care of orphans, who are children whose parents are either dead or otherwise unable to care for their child."""@en;
  skos:exactMatch aat:300006769;
  skos:altLabel "weeshuis"@nl;
  skos:altLabel "orphelinat"@fr;
  skos:altLabel "waisenhaus"@de;
  skos:altLabel "orphanage"@en;
  skos:inScheme dccd:objectElementType.
dccd:a7a2d968-6b80-11e5-ac05-cfc3cb9d6c6a rdf:type skos:Concept;
  skos:scopeNote """Bodies of water serving as ways or routes for travel or transportation """@en;
  skos:exactMatch aat:300263418;
  skos:altLabel "voie d'eau"@fr;
  skos:altLabel "waterway"@en;
  skos:altLabel "waterweg"@nl;
  skos:altLabel "voie navigable"@fr;
  skos:altLabel "wasserstraße"@de;
  skos:inScheme dccd:objectElementType.
dccd:a7a2db34-6b80-11e5-ac06-3b3e4859a6b1 rdf:type skos:Concept;
  skos:scopeNote """A castle or stately home whose site is entirely surrounded by water-filled moats (moated castles) or natural waterbodies such as island castles in a river or offshore."""@en;
  skos:narrower aat:300005656;
  skos:altLabel "waterburcht"@nl;
  skos:altLabel "château-fort à douves"@fr;
  skos:altLabel "watercastle"@en;
  skos:altLabel "wasserburg"@de;
  skos:inScheme dccd:objectElementType.
dccd:a7a2dbe8-6b80-11e5-ac07-3bd42eaae36b rdf:type skos:Concept;
  skos:scopeNote """Implements or mechanisms used for defense or attack in combat, hunting, or war."""@en;
  skos:exactMatch aat:300036926;
  skos:altLabel "wapen"@nl;
  skos:altLabel "arme"@fr;
  skos:altLabel "weapon"@en;
  skos:altLabel "waffe"@de;
  skos:inScheme dccd:objectElementType.
dccd:a7a2dfd0-6b80-11e5-ac0d-cf2fdfdfbc96 rdf:type skos:Concept;
  skos:scopeNote """Any built structure used as a lookout station that affords observation of a surrounding area."""@en;
  skos:exactMatch aat:300134522;
  skos:altLabel "lookout tower"@en;
  skos:altLabel "wachttoren"@nl;
  skos:altLabel "watchtower"@en;
  skos:altLabel "tour de guet"@fr;
  skos:altLabel "wachtturm"@de;
  skos:altLabel "wachturm"@de;
  skos:altLabel "uitkijktoren"@nl;
  skos:inScheme dccd:objectElementType.
dccd:a7a2e58e-6b80-11e5-ac16-e7b5b004826d rdf:type skos:Concept;
  skos:narrower aat:300045611;
  skos:altLabel "coffre"@fr;
  skos:altLabel "bac"@fr;
  skos:altLabel "behälter"@de;
  skos:altLabel "bak"@nl;
  skos:altLabel "container"@en;
  skos:altLabel "récipient"@fr;
  skos:inScheme dccd:objectElementType.
dccd:a7a2e638-6b80-11e5-ac17-6f09e2d2ba87 rdf:type skos:Concept;
  skos:scopeNote """Use for rafters placed at the juncture of the inclined planes forming hip roofs """@en;
  skos:exactMatch aat:300002431;
  skos:altLabel "gratsparren"@de;
  skos:altLabel "hip rafter"@en;
  skos:altLabel "chevron d'arêtier"@fr;
  skos:altLabel "hoekkeper"@nl;
  skos:inScheme dccd:objectElementType.
dccd:a7a2e6e2-6b80-11e5-ac18-bf94913bb2da rdf:type skos:Concept;
  skos:scopeNote """Use for rafters that do not extend from the roof plates to the ridgeboards; employed in hip roofs to reach from roof plates to hip rafters. For rafters spanning between valley rafters and ridgeboards, use 'valley jacks """@en;
  skos:exactMatch aat:300002434;
  skos:altLabel "jack rafter"@en;
  skos:altLabel "schifter"@de;
  skos:altLabel "schiftsparren"@de;
  skos:altLabel "karbeel"@nl;
  skos:altLabel "verkorte spoor die tot aan de hoekkeper loopt"@nl;
  skos:altLabel "moise"@fr;
  skos:altLabel "empanon"@fr;
  skos:inScheme dccd:objectElementType.
dccd:a7a2e782-6b80-11e5-ac19-6f5c5e97030d rdf:type skos:Concept;
  skos:scopeNote """Use for the main central part of an interior divided into a high center with lower side portions divided by columns or piers, usually but not always in a church. Use also for the main part of a church without aisles but with a distinct chancel"""@en;
  skos:exactMatch aat:300004627;
  skos:altLabel "kerkruimte"@nl;
  skos:altLabel "kirchenschiff"@de;
  skos:altLabel "nave"@en;
  skos:altLabel "nef"@fr;
  skos:inScheme dccd:objectElementType.
dccd:a7a2e82c-6b80-11e5-ac1a-ef7a55429a6a rdf:type skos:Concept;
  skos:scopeNote """Upward brace at the upper end of a frame running for example from a post to a wall plate"""@en;
  skos:narrower aat:300001834;
  skos:altLabel "curved brace"@en;
  skos:altLabel "kopfband"@de;
  skos:altLabel "guette"@fr;
  skos:altLabel "arch brace"@en;
  skos:altLabel "korbeel"@nl;
  skos:altLabel "upward brace"@en;
  skos:altLabel "ascending bracae"@en;
  skos:altLabel "schoor"@nl;
  skos:inScheme dccd:objectElementType.
dccd:a7a2e8d6-6b80-11e5-ac1b-af89ca1bff4a rdf:type skos:Concept;
  skos:scopeNote """Inclined timber rising from a beam to a rafter or principal rafter in roof constructions with knee walls."""@en;
  skos:narrower aat:300001834;
  skos:altLabel "schubverteiler"@de;
  skos:altLabel "sling brace"@en;
  skos:altLabel "jambe de force"@fr;
  skos:altLabel "kreupele stijl"@nl;
  skos:altLabel "post"@en;
  skos:altLabel "knee brace"@en;
  skos:inScheme dccd:objectElementType.
dccd:a7a2e980-6b80-11e5-ac1c-a324938ec043 rdf:type skos:Concept;
  skos:scopeNote """Long brace which crosses one or more vertical timbers"""@en;
  skos:narrower aat:300001834;
  skos:altLabel "langstrebe"@de;
  skos:altLabel "passing brace"@en;
  skos:altLabel "écharpe"@fr;
  skos:altLabel "kruisschoor"@nl;
  skos:inScheme dccd:objectElementType.
dccd:a7a2ea2a-6b80-11e5-ac1d-7feff7a3f669 rdf:type skos:Concept;
  skos:scopeNote """Horizontal members placed along the tops of walls or a series of studs to support joists or rafters """@en;
  skos:exactMatch aat:300001868;
  skos:altLabel "mauerlatte"@de;
  skos:altLabel "wall plate"@en;
  skos:altLabel "sablière"@fr;
  skos:altLabel "muurplaat"@nl;
  skos:inScheme dccd:objectElementType.
dccd:a7a2eaca-6b80-11e5-ac1e-6b2d55b7e84a rdf:type skos:Concept;
  skos:scopeNote """Series of vertical structural members which act as the supporting elements in a wall or partition."""@en;
  skos:exactMatch aat:300001882;
  skos:altLabel "wandstijl"@nl;
  skos:altLabel "wandständer"@de;
  skos:altLabel "stud"@en;
  skos:altLabel "poteau intermédiaire"@fr;
  skos:altLabel "muurstijl"@nl;
  skos:inScheme dccd:objectElementType.
dccd:a7a2eb74-6b80-11e5-ac1f-c775f5e8323d rdf:type skos:Concept;
  skos:narrower aat:300002424;
  skos:altLabel "auflanger"@de;
  skos:altLabel "aisle rafter"@en;
  skos:altLabel "chevron de bas-côté"@fr;
  skos:altLabel "oplanger"@nl;
  skos:inScheme dccd:objectElementType.
dccd:a7a2ecc8-6b80-11e5-ac21-8fac672b5a7b rdf:type skos:Concept;
  skos:scopeNote """A ram was a weapon carried by varied types of ships, dating back to antiquity. The weapon comprised an underwater prolongation of the bow of the ship to form an armoured beak, usually between six and 12 feet (2–4 m) in length. This would be driven into the hull of an enemy ship in order to puncture the hull and sink, or at least disable, that ship."""@en;
  skos:narrower aat:300203726;
  skos:altLabel "rammbock"@de;
  skos:altLabel "ram"@en;
  skos:altLabel "bélier"@fr;
  skos:altLabel "stormram"@nl;
  skos:inScheme dccd:objectElementType.
dccd:a7a2efde-6b80-11e5-ac22-a7ca8d1e7b86 rdf:type skos:Concept;
  skos:scopeNote """A type of manor house specific to Utrecht in Holland owner by one of the knighthood"""@en;
  skos:narrower aat:300005579;
  skos:altLabel "ridderhofstad"@nl;
  skos:inScheme dccd:objectElementType.
dccd:a7a2f0b0-6b80-11e5-ac23-c7c7d44f97b3 rdf:type skos:Concept;
  skos:scopeNote """Small, usually isolated, fortification works of any form, commonly square or polygonal in plan, used to defend a prominent point"""@en;
  skos:narrower aat:300006888;
  skos:altLabel "schanze"@de;
  skos:altLabel "entrenchment"@en;
  skos:altLabel "retranchement"@fr;
  skos:altLabel "schans"@nl;
  skos:inScheme dccd:objectElementType.
dccd:a7a2f15a-6b80-11e5-ac24-8f9cdaba8bb1 rdf:type skos:Concept;
  skos:scopeNote """Wide plate of wood at the bottom of a posthold which prevents the post from sinking into the ground."""@en;
  skos:narrower aat:300078047;
  skos:altLabel "pfostenschuh"@de;
  skos:altLabel "post-pad"@en;
  skos:altLabel "sabot"@fr;
  skos:altLabel "paalschoen"@nl;
  skos:altLabel "patin (de bois)"@fr;
  skos:inScheme dccd:objectElementType.
dccd:a7a2f204-6b80-11e5-ac25-afb7ba91f44c rdf:type skos:Concept;
  skos:scopeNote """Blade in context of a water wheel"""@en;
  skos:narrower aat:300024617;
  skos:altLabel "schaufel"@de;
  skos:altLabel "blade"@en;
  skos:altLabel "aube"@fr;
  skos:altLabel "schoep"@nl;
  skos:inScheme dccd:objectElementType.
dccd:a7a2f2b8-6b80-11e5-ac26-23537fe2b26d rdf:type skos:Concept;
  skos:scopeNote """Inclined timber in the roof plane of a common rafter roof which crosses several rafters to provide lengthwise stability."""@en;
  skos:narrower aat:300001834;
  skos:altLabel "schwertlatte"@de;
  skos:altLabel "sturmlatte"@de;
  skos:altLabel "windlatte"@de;
  skos:altLabel "schrankhout"@nl;
  skos:altLabel "windrispe"@de;
  skos:altLabel "rafter brace"@en;
  skos:altLabel "écharpe de contreventement"@fr;
  skos:altLabel "windlat"@nl;
  skos:altLabel "sporenschrankhout"@nl;
  skos:inScheme dccd:objectElementType.
dccd:a7a2f362-6b80-11e5-ac27-db6fe564e933 rdf:type skos:Concept;
  skos:scopeNote """Types of construction in which walls, partitions, floors, and roof are wholly or partly made of wood; Use for constructions of any kind artificially fabricated of parts joined together in some definite manner and which may or may not provide enclosure or shelter??"""@en;
  skos:exactMatch aat:300111619;
  skos:altLabel "gerüstbau"@de;
  skos:altLabel "timber-framed construction"@en;
  skos:altLabel "construction sur ossature"@fr;
  skos:altLabel "houtskelebouw"@nl;
  skos:inScheme dccd:objectElementType.
dccd:a7a2f40c-6b80-11e5-ac28-cf95323d0a29 rdf:type skos:Concept;
  skos:scopeNote """Refers to the members that form the base of the roof truss and prevent the rafters from spreading."""@en;
  skos:exactMatch aat:300002419;
  skos:altLabel "stuhlbalken"@de;
  skos:altLabel "tie beam"@en;
  skos:altLabel "faux-entrait de portique"@fr;
  skos:altLabel "spantbalk"@nl;
  skos:inScheme dccd:objectElementType.
dccd:a7a2f4b6-6b80-11e5-ac29-bfb54ffedfd1 rdf:type skos:Concept;
  skos:scopeNote """Earliest type of European windmill. The defining feature is that the whole body of the mill that houses the machinery is mounted on a single vertical post, around which it can be turned to bring the sails into the wind."""@en;
  skos:narrower aat:300006273;
  skos:altLabel "bockwindmühle"@de;
  skos:altLabel "post mill"@en;
  skos:altLabel "moulin sur pivot"@fr;
  skos:altLabel "standerdmolen"@nl;
  skos:inScheme dccd:objectElementType.
dccd:a7a2f560-6b80-11e5-ac2a-8355c120e5f3 rdf:type skos:Concept;
  skos:scopeNote """Horizontal timber often resting on wooden or stone brackets or projection running adjacent to a wall but not an integrated part of the wall frame."""@en;
  skos:narrower aat:300001497;
  skos:altLabel "streichbalken"@de;
  skos:altLabel "applied beam"@en;
  skos:altLabel "solive de rive"@fr;
  skos:altLabel "strijkbalk"@nl;
  skos:inScheme dccd:objectElementType.
dccd:a7a2f60a-6b80-11e5-ac2b-afd750abcfb1 rdf:type skos:Concept;
  skos:scopeNote """Structural members whose primary function is to carry transverse loads"""@en;
  skos:exactMatch aat:300001497;
  skos:altLabel "beam"@en;
  skos:altLabel "balk"@nl;
  skos:altLabel "balken"@de;
  skos:altLabel "poutre"@fr;
  skos:inScheme dccd:objectElementType.
dccd:a7a2f6b4-6b80-11e5-ac2c-fb98219bacee rdf:type skos:Concept;
  skos:scopeNote """Small hills, small elevations in the earth's surface, or small mounds or heaps of earth or stones."""@en;
  skos:exactMatch aat:300008781;
  skos:altLabel "knoll"@en;
  skos:altLabel "butte"@fr;
  skos:altLabel "monticule"@fr;
  skos:altLabel "wurte"@de;
  skos:altLabel "tetre"@fr;
  skos:altLabel "terp"@nl;
  skos:altLabel "hillock"@en;
  skos:inScheme dccd:objectElementType.
dccd:a7a2f768-6b80-11e5-ac2d-0f3535f98c4b rdf:type skos:Concept;
  skos:scopeNote """Pieces of wood or metal tapering to a thin edge; used to adjust elevation or tighten formwork, or to split wood or rock."""@en;
  skos:exactMatch aat:300024101;
  skos:altLabel "wig"@nl;
  skos:altLabel "coin"@fr;
  skos:altLabel "wedge"@en;
  skos:altLabel "keil"@de;
  skos:inScheme dccd:objectElementType.
dccd:a7a2f808-6b80-11e5-ac2e-2bcc0d81be52 rdf:type skos:Concept;
  skos:scopeNote """Large artificial mound in the Netherlands used to provide refuge for during a seasonally flood"""@en;
  skos:narrower aat:300008024;
  skos:altLabel "wierde"@nl;
  skos:altLabel "tertre"@fr;
  skos:altLabel "terp"@en;
  skos:altLabel "warft"@de;
  skos:inScheme dccd:objectElementType.
dccd:a7a2f8c6-6b80-11e5-ac2f-9fe50a029482 rdf:type skos:Concept;
  skos:scopeNote """Artificial paved banks or solid landing places built parallel to and extending the shoreline to serve in the loading and unloading of vessels. For less fixed and solid structures built in similar locations and for similar purposes, use 'wharves'; use 'piers (marine landings)' when such lighter structures extend out over the water."""@en;
  skos:exactMatch aat:300120782;
  skos:altLabel "kai"@de;
  skos:altLabel "quay"@en;
  skos:altLabel "quai"@fr;
  skos:altLabel "kade"@nl;
  skos:inScheme dccd:objectElementType.
dccd:a7a2f970-6b80-11e5-ac30-67d32cb0131b rdf:type skos:Concept;
  skos:scopeNote """Structures, in post-Second World War contexts, built generally parallel to the shoreline so that vessels may moor alongside to receive or discharge cargo or passengers; prior to the mid-20th century, may refer broadly to any such landing places. For similar loading and unloading places built to extend from the shoreline out over water, use 'piers (marine landings)'; if such places are artificial solid banks or shoreline extensions built parallel to the shoreline, use 'quays.'"""@en;
  skos:exactMatch aat:300120786;
  skos:altLabel "wharf"@en;
  skos:altLabel "werf"@nl;
  skos:inScheme dccd:objectElementType.
dccd:a7a2fa1a-6b80-11e5-ac31-a3d029d44e0c rdf:type skos:Concept;
  skos:scopeNote """Use, in post-Second World War contexts, for structures built generally parallel to the shoreline so that vessels may moor alongside to receive or discharge cargo or passengers; prior to the mid-20th century, may refer broadly to any such landing places. For similar loading and unloading places built to extend from the shoreline out over water, use 'piers (marine landings)'; if such places are artificial solid banks or shoreline extensions built parallel to the shoreline, use 'quays.'
Use for any of various structures built for loading or unloading goods or embarking or disembarking passengers onto and off of watercraft.
Use for artificial paved banks or solid landing places built parallel to and extending the shoreline to serve in the loading and unloading of vessels. For less fixed and solid structures built in similar locations and for similar purposes, use 'wharves'; use 'piers (marine landings)' when such lighter structures extend out over the water"""@en;
  skos:exactMatch aat:300007928;
  skos:altLabel "anlege"@de;
  skos:altLabel "anlegeplatz"@de;
  skos:altLabel "anlegestelle"@de;
  skos:altLabel "bootssteg"@de;
  skos:altLabel "landungsbrücke"@de;
  skos:altLabel "landungsplatz"@de;
  skos:altLabel "landungsstelle"@de;
  skos:altLabel "steg"@de;
  skos:altLabel "landing stage"@en;
  skos:altLabel "débarcadère"@fr;
  skos:altLabel "embarcadère"@fr;
  skos:altLabel "ponton"@fr;
  skos:altLabel "aanlegplaats"@nl;
  skos:altLabel "aanlegsteiger"@nl;
  skos:altLabel "landing place"@en;
  skos:altLabel "landingsplaats"@nl;
  skos:altLabel "landung"@de;
  skos:altLabel "atterrissage"@fr;
  skos:inScheme dccd:objectElementType.
dccd:a7a2fae2-6b80-11e5-ac32-d3cdf7f09544 rdf:type skos:Concept;
  skos:scopeNote """Long narrow excavations, usually with sloping sides, dug in the earth for defense, drainage, or irrigation."""@en;
  skos:exactMatch aat:300006178;
  skos:altLabel "graben"@de;
  skos:altLabel "greppel"@nl;
  skos:altLabel "fossé"@fr;
  skos:altLabel "ditch"@en;
  skos:altLabel "sloot"@nl;
  skos:inScheme dccd:objectElementType.
dccd:a7a2fb8c-6b80-11e5-ac33-b7bbe7d0e283 rdf:type skos:Concept;
  skos:scopeNote """Beam carrying a floor which forms a ceiling covering of a room"""@en;
  skos:exactMatch aat:300375090;
  skos:altLabel "floor joists"@en;
  skos:altLabel "joisting"@en;
  skos:altLabel "floor frame"@en;
  skos:altLabel "sommier"@fr;
  skos:altLabel "vloerbalk"@nl;
  skos:altLabel "deckenbalken"@de;
  skos:altLabel "ceiling joist"@en;
  skos:inScheme dccd:objectElementType.
dccd:a7a2fc40-6b80-11e5-ac34-b388a286cdde rdf:type skos:Concept;
  skos:scopeNote """Refers to deep, wide defensive ditches surrounding towns, castles, or houses and usually filled with water."""@en;
  skos:exactMatch aat:300003716;
  skos:altLabel "wassergraben"@de;
  skos:altLabel "moat"@en;
  skos:altLabel "burggraben"@de;
  skos:inScheme dccd:objectElementType.
dccd:a7a2fcea-6b80-11e5-ac35-c7e2cc964ee6 rdf:type skos:Concept;
  skos:scopeNote """ Long, narrow, usually steep-sided cuts into the earth, as to receive pipes, wires, or footings; may also be used for defensive cuts, especially when the excavated earth is heaped in front as a barrier. For defensive cuts in which the earth is not used as added protection, use 'fosses' or 'moats.'"""@en;
  skos:exactMatch aat:300008022;
  skos:altLabel "r
tranchée"@fr;
  skos:altLabel "loopgraaf"@nl;
  skos:altLabel "graben"@de;
  skos:altLabel "channel"@en;
  skos:altLabel "cutting"@en;
  skos:altLabel "trench"@en;
  skos:inScheme dccd:objectElementType.
dccd:a7a2fd94-6b80-11e5-ac36-77cd38447a8c rdf:type skos:Concept;
  skos:scopeNote """Water distribution structures"""@en;
  skos:narrower aat:300006164;
  skos:altLabel "canalisation d'eau"@fr;
  skos:altLabel "waterleiding"@nl;
  skos:altLabel "wasserleitung"@de;
  skos:altLabel "water pipe"@en;
  skos:altLabel "water conduit"@en;
  skos:altLabel "conduite d'eau"@fr;
  skos:inScheme dccd:objectElementType.
dccd:a7a1b920-6b80-11e5-aa78-0f19e75e5a25 rdf:type skos:Concept;
  skos:scopeNote """Devices or assemblies of devices designed to support artillery and heavy small arms such as machine guns. They range from simple tripods to complex supporting, pivoting, and elevating mechanisms on gun carriages."""@en;
  skos:closeMatch aat:300221835;
  skos:altLabel "rolpaard"@nl;
  skos:altLabel "lafette"@de;
  skos:altLabel "carriage"@en;
  skos:altLabel "affût"@fr;
  skos:altLabel "affuit"@nl;
  skos:inScheme dccd:objectElementType.
