##############################################################
# This file was generated on Tue, 06 Oct 2015 14:52:14 -0600
# Number of checked and rejected concepts   : 103
# Number of checked and accepted concepts   : 370
# Number of concepts that need checking     : 10
# Number of concepts with AAT match assigned: 365
##############################################################
@prefix skos: <http://www.w3.org/2004/02/skos/core#> .
@prefix rdf: <http://www.w3.org/1999/02/22-rdf-syntax-ns#> .
@prefix rdfs: <http://www.w3.org/2000/01/rdf-schema#> .
@prefix owl: <http://www.w3.org/2002/07/owl#> .
@prefix dct: <http://purl.org/dc/terms/> .
@prefix foaf: <http://xmlns.com/foaf/0.1/> .
@prefix aat: <http://vocab.getty.edu/aat/> .
@prefix dccd: <http://dendro.dans.knaw.nl/dccd-terms/> .
dccd:objectElementType rdf:type skos:ConceptScheme;
  dct:title "DCCD TRiDaS Object/Element Type Dictionary";
  dct:creator dccd:DCCD.
dccd:a7a199ae-6b80-11e5-aa5a-5ffcedf4cb3e rdf:type skos:Concept;
  skos:scopeNote """Use for lightly built, slender, open craft of shallow draft that are paddled and not rowed and normally double-ended; may have sails """@en;
  skos:exactMatch aat:300212688;
  skos:altLabel "canot"@fr;
  skos:altLabel "pirogue"@fr;
  skos:prefLabel "kanu"@de;
  skos:prefLabel "canoe"@en;
  skos:prefLabel "canoë"@fr;
  skos:prefLabel "kano"@nl;
  skos:broader dccd:a7a1ba74-6b80-11e5-aa7a-7b1dc4c873b5;
  skos:inScheme dccd:objectElementType.
dccd:a7a1a4bc-6b80-11e5-aa5b-236804fe51af rdf:type skos:Concept;
  skos:scopeNote """shipsterm """@en;
  skos:exactMatch aat:300233025;
  skos:prefLabel "kutter"@de;
  skos:prefLabel "cutter"@en;
  skos:prefLabel "cottre"@fr;
  skos:prefLabel "kotter"@nl;
  skos:broader dccd:a7a1ba74-6b80-11e5-aa7a-7b1dc4c873b5;
  skos:inScheme dccd:objectElementType.
dccd:a7a1a606-6b80-11e5-aa5c-1b177227ec3d rdf:type skos:Concept;
  skos:scopeNote """shipsterm """@en;
  skos:exactMatch aat:300232673;
  skos:altLabel "platboomd schip"@nl;
  skos:prefLabel "plattbodenschiff"@de;
  skos:prefLabel "flat bottomed vessel"@en;
  skos:prefLabel "navire à fond plat"@fr;
  skos:prefLabel "platbodem"@nl;
  skos:broader dccd:a7a1ba74-6b80-11e5-aa7a-7b1dc4c873b5;
  skos:inScheme dccd:objectElementType.
dccd:a7a1a6c4-6b80-11e5-aa5d-3f5fa69529c9 rdf:type skos:Concept;
  skos:scopeNote """Rooms in or attached to churches where the sacred utensils and vestments are kept """@en;
  skos:exactMatch aat:300266764;
  skos:prefLabel "vestry"@en;
  skos:altLabel "sacristy"@en;
  skos:altLabel "almerei"@de;
  skos:altLabel "gerbekammer"@de;
  skos:prefLabel "sakristei"@de;
  skos:prefLabel "sacristie"@fr;
  skos:prefLabel "sacristie"@nl;
  skos:inScheme dccd:objectElementType.
dccd:a7a1a8e0-6b80-11e5-aa60-ff1241ceddd8 rdf:type skos:Concept;
  skos:scopeNote """Use for the outside, overhead enclosures of buildings or other structures, including the roofing and its structural framing """@en;
  skos:exactMatch aat:300002098;
  skos:prefLabel "dak"@nl;
  skos:prefLabel "toit, toiture"@fr;
  skos:prefLabel "roof"@en;
  skos:prefLabel "dach"@de;
  skos:inScheme dccd:objectElementType.
dccd:a7a1a994-6b80-11e5-aa61-7b19d7861439 rdf:type skos:Concept;
  skos:scopeNote """Interior walls separating one portion of a space from another; sometimes permanent inside walls that divide buildings into various rooms, sometimes designed to move aside and open up a space. For entities other than walls that divide interior spaces, often incorporating bookshelves, cabinets, or drawers, use 'room dividers.'"""@en;
  skos:exactMatch aat:300002538;
  skos:prefLabel "partition wall"@en;
  skos:prefLabel "tussenmuur"@nl;
  skos:prefLabel "mur de séparation"@fr;
  skos:altLabel "mur de refend"@fr;
  skos:altLabel "tussenwand"@nl;
  skos:altLabel "scheidemauer"@de;
  skos:altLabel "partition"@en;
  skos:prefLabel "trennwand"@de;
  skos:inScheme dccd:objectElementType.
dccd:a7a1aaf2-6b80-11e5-aa63-63855abd6c6f rdf:type skos:Concept;
  skos:scopeNote """shipsterm """@en;
  skos:exactMatch aat:300263189;
  skos:prefLabel "deck"@de;
  skos:prefLabel "deck"@en;
  skos:prefLabel "pont"@fr;
  skos:prefLabel "dek"@nl;
  skos:inScheme dccd:objectElementType.
dccd:a7a1ab9c-6b80-11e5-aa64-6b11fae244dd rdf:type skos:Concept;
  skos:scopeNote """Chests with deep storage space, at least one drawer, and a hinged lid. Frequently used for the storage of blankets."""@en;
  skos:exactMatch aat:300172507;
  skos:prefLabel "dekenkist"@nl;
  skos:prefLabel "bahut"@fr;
  skos:prefLabel "blanket chest"@en;
  skos:prefLabel "truhe"@de;
  skos:inScheme dccd:objectElementType.
dccd:a7a1ac46-6b80-11e5-aa65-f7acd75b8d1d rdf:type skos:Concept;
  skos:scopeNote """Braces, such as struts, which strengthen a structure or framework against the wind."""@en;
  skos:exactMatch aat:300001839;
  skos:altLabel "kopfstrebe"@de;
  skos:altLabel "strebe"@de;
  skos:altLabel "windrispe"@de;
  skos:altLabel "strut"@en;
  skos:altLabel "contreventement"@fr;
  skos:altLabel "drukschoor"@nl;
  skos:prefLabel "windstrebe"@de;
  skos:prefLabel "wind brace"@en;
  skos:prefLabel "écharpe"@fr;
  skos:prefLabel "windschoor"@nl;
  skos:inScheme dccd:objectElementType.
dccd:a7a1acf0-6b80-11e5-aa66-c3b32d16aed6 rdf:type skos:Concept;
  skos:scopeNote """Buildings belonging to and for the assembly of members of crafts, trades, or merchants' guilds"""@en;
  skos:exactMatch aat:300007077;
  skos:prefLabel "handwerkshaus"@de;
  skos:prefLabel "guildhall"@en;
  skos:prefLabel "maison de l'artisanat"@fr;
  skos:prefLabel "ambachtshuis"@nl;
  skos:inScheme dccd:objectElementType.
dccd:a7a1ada4-6b80-11e5-aa67-7f361ee65bb8 rdf:type skos:Concept;
  skos:scopeNote """Crosses in the form of the letter X, used as a heraldic symbol in the form of a diagonal cross or letter X and as a symbol for Saint Andrew, who is said to have been martyred on such a cross."""@en;
  skos:exactMatch aat:300010079;
  skos:prefLabel "andreaskreuz"@de;
  skos:prefLabel "saint andrew's cross"@en;
  skos:prefLabel "croix de saint-andré"@fr;
  skos:prefLabel "andreaskruis"@nl;
  skos:inScheme dccd:objectElementType.
dccd:a7a1ae4e-6b80-11e5-aa68-c38266563250 rdf:type skos:Concept;
  skos:scopeNote """Use for square or rectangular upright, masonry, supporting elements, and for similar elements of wood when classically treated; use also for massive upright supporting elements of any shape in Medieval architecture. For cylindrical uprights, except when Medieval as described above, and for all uprights in steel and concrete frames, use 'columns (architectural elements)'; for square wooden uprights when not classically treated, use 'posts.'"""@en;
  skos:exactMatch aat:300078728;
  skos:altLabel "pile"@fr;
  skos:altLabel "brugpijler"@nl;
  skos:prefLabel "pfeiler"@de;
  skos:prefLabel "pier"@en;
  skos:prefLabel "pilier"@fr;
  skos:prefLabel "pijler"@nl;
  skos:inScheme dccd:objectElementType.
dccd:a7a1af02-6b80-11e5-aa69-db2c32fe2881 rdf:type skos:Concept;
  skos:scopeNote """Small subordinate ribs, inserted between the main ribs of Gothic vaults."""@en;
  skos:exactMatch aat:300266287;
  skos:prefLabel "verbindingsrib"@nl;
  skos:prefLabel "lierne"@fr;
  skos:prefLabel "lierne rib"@en;
  skos:prefLabel "nebenrippe"@de;
  skos:inScheme dccd:objectElementType.
dccd:a7a1afac-6b80-11e5-aa6a-136a044ccba0 rdf:type skos:Concept;
  skos:scopeNote """A long narrow flat-bottomed boat, square at both ends and propelled with a long pole, used on inland waters chiefly for recreation"""@en;
  skos:broadMatch aat:300178749;
  skos:altLabel "pünte-artiges fahrzeug"@de;
  skos:altLabel "punt-like vessel"@en;
  skos:altLabel "navire aux elements constructifs de plate"@fr;
  skos:altLabel "punter-achtig vaartuig"@nl;
  skos:broader dccd:a7a1ba74-6b80-11e5-aa7a-7b1dc4c873b5;
  skos:inScheme dccd:objectElementType.
dccd:a7a1b060-6b80-11e5-aa6b-2b06c868f4c9 rdf:type skos:Concept;
  skos:scopeNote """General term for any works made to oppose a small number of troops against a greater
Use for the habitable spaces between two floors of a building or between a floor and the roof, and for the horizontal divisions of the exteriors of buildings which tend to correspond to this division of the interior spaces"""@en;
  skos:exactMatch aat:300006888;
  skos:prefLabel "fortification"@fr;
  skos:prefLabel "befestigung"@de;
  skos:prefLabel "versterking"@nl;
  skos:prefLabel "fortification"@en;
  skos:altLabel "construction défensive"@fr;
  skos:altLabel "verdedigingswerk"@nl;
  skos:altLabel "befestigungsanlage"@de;
  skos:altLabel "festungswerk"@de;
  skos:altLabel "wehrbau"@de;
  skos:altLabel "defensive work"@en;
  skos:altLabel "ouvrage de défense"@fr;
  skos:inScheme dccd:objectElementType.
dccd:a7a1b3bc-6b80-11e5-aa70-6b98467e51b7 rdf:type skos:Concept;
  skos:broadMatch aat:300003632;
  skos:altLabel "roof turret"@en;
  skos:prefLabel "dachreiter"@de;
  skos:prefLabel "ridge turret"@en;
  skos:prefLabel "dakruiter"@nl;
  skos:inScheme dccd:objectElementType.
dccd:a7a1b470-6b80-11e5-aa71-f3477fb25391 rdf:type skos:Concept;
  skos:closeMatch aat:300004188;
  skos:altLabel "achtervleugel"@nl;
  skos:prefLabel "rear wing"@en;
  skos:prefLabel "achterhuis"@nl;
  skos:prefLabel "hinterhaus"@de;
  skos:altLabel "arrière-corps (de la maison)"@fr;
  skos:prefLabel "aisle arriere"@fr;
  skos:inScheme dccd:objectElementType.
dccd:a7a1b51a-6b80-11e5-aa72-474f43f89a5f rdf:type skos:Concept;
  skos:scopeNote """Use for watercraft generally smaller and less seaworthy than ships and generally not designed to cross large open waters """@en;
  skos:exactMatch aat:300178749;
  skos:prefLabel "boot"@de;
  skos:prefLabel "boat"@en;
  skos:prefLabel "bateau"@fr;
  skos:prefLabel "boot"@nl;
  skos:broader dccd:a7a1ba74-6b80-11e5-aa7a-7b1dc4c873b5;
  skos:inScheme dccd:objectElementType.
dccd:a7a1b5c4-6b80-11e5-aa73-bf4c2f38f1f2 rdf:type skos:Concept;
  skos:broadMatch aat:300000888;
  skos:altLabel "abutment"@en;
  skos:prefLabel "brückenkopf"@de;
  skos:prefLabel "bridge head"@en;
  skos:prefLabel "tête de pont"@fr;
  skos:prefLabel "bruggenhoofd"@nl;
  skos:inScheme dccd:objectElementType.
dccd:a7a1b66e-6b80-11e5-aa74-cb5e23f46409 rdf:type skos:Concept;
  skos:scopeNote """Use for small unfinished attic spaces immediately below roof ridges; Use for enclosed spaces under sloping roofs, between the roof and the ceiling of the uppermost story, especially in houses, whether used for storage or habitation. For open platforms in houses set close to ceilings or for large spaces below the roofs of commercial buildings or warehouses, use 'lofts (upper level floors)"""@en;
  skos:exactMatch aat:300004076;
  skos:altLabel "loft"@en;
  skos:prefLabel "dachboden"@de;
  skos:prefLabel "grenier"@fr;
  skos:altLabel "oberes dachgeschoss"@de;
  skos:altLabel "cockloft"@en;
  skos:altLabel "soupente"@fr;
  skos:prefLabel "attic"@en;
  skos:prefLabel "vliering"@nl;
  skos:inScheme dccd:objectElementType.
dccd:a7a1b7c2-6b80-11e5-aa76-fba313e9a5db rdf:type skos:Concept;
  skos:scopeNote """Part of the shell of the hull of a boat or ship which, in conjunction with the other strakes, keeps the sea out and the vessel afloat"""@en;
  skos:broadMatch aat:300212614;
  skos:prefLabel "bordgang"@de;
  skos:prefLabel "side strake"@en;
  skos:prefLabel "bordage"@fr;
  skos:prefLabel "berghout"@nl;
  skos:inScheme dccd:objectElementType.
dccd:a7a1b876-6b80-11e5-aa77-efc72bb9da1b rdf:type skos:Concept;
  skos:scopeNote """a facing of planks and piles placed along the bank of a river to prevent erosion"""@en;
  skos:broadMatch aat:300006136;
  skos:prefLabel "uferbefestigung"@de;
  skos:prefLabel "campsheeting"@en;
  skos:prefLabel "palée"@fr;
  skos:prefLabel "oeverbeschoeiing"@nl;
  skos:inScheme dccd:objectElementType.
dccd:a7a1b9ca-6b80-11e5-aa79-b78d5a08cec5 rdf:type skos:Concept;
  skos:scopeNote """Individual dwellings designed to be occupied by a single tenant or family. May also refer to a building for human occupation, for some purpose other than that of an ordinary dwelling; with this usage, 'house' is generally prefaced (e.g., 'cowhouse,' 'almshouse')."""@en;
  skos:exactMatch aat:300005433;
  skos:altLabel "wohnung"@de;
  skos:altLabel "residence"@en;
  skos:altLabel "demeure"@fr;
  skos:altLabel "domicile"@fr;
  skos:altLabel "habitation"@fr;
  skos:altLabel "woning"@nl;
  skos:altLabel "wohnhaus"@de;
  skos:altLabel "maison d'habitation"@fr;
  skos:altLabel "woonhuis"@nl;
  skos:prefLabel "haus"@de;
  skos:prefLabel "house"@en;
  skos:prefLabel "maison"@fr;
  skos:prefLabel "huis"@nl;
  skos:inScheme dccd:objectElementType.
dccd:a7a1ba74-6b80-11e5-aa7a-7b1dc4c873b5 rdf:type skos:Concept;
  skos:scopeNote """Top level concept for all watercraft"""@en;
  skos:exactMatch aat:300042940;
  skos:prefLabel "waterscooter"@nl;
  skos:prefLabel "motomarine"@fr;
  skos:prefLabel "Wasserfahrzeuge"@de;
  skos:prefLabel "watercraft"@en;
  skos:broader dccd:a7a199ae-6b80-11e5-aa5a-5ffcedf4cb3e;
  skos:broader dccd:a7a1a4bc-6b80-11e5-aa5b-236804fe51af;
  skos:broader dccd:a7a1a606-6b80-11e5-aa5c-1b177227ec3d;
  skos:broader dccd:a7a1afac-6b80-11e5-aa6a-136a044ccba0;
  skos:broader dccd:a7a1b51a-6b80-11e5-aa72-474f43f89a5f;
  skos:broader dccd:a7a1c4ec-6b80-11e5-aa85-3b00c067cf0e;
  skos:broader dccd:a7a1d400-6b80-11e5-aa9c-db85c58837ab;
  skos:broader dccd:a7a1d572-6b80-11e5-aa9e-475b95e2c6da;
  skos:broader dccd:a7a1d356-6b80-11e5-aa9b-8fe3ef82f828;
  skos:broader dccd:a7a20ba0-6b80-11e5-aae9-af39bcc68cdd;
  skos:broader dccd:a7a26226-6b80-11e5-ab60-7f110d55838a;
  skos:broader dccd:a7a281de-6b80-11e5-ab8d-1b18cbbaafc5;
  skos:broader dccd:a7a2bfbe-6b80-11e5-abe2-cbd88e5cbc94;
  skos:inScheme dccd:objectElementType.
dccd:a7a1b312-6b80-11e5-aa6f-e3f307fdf0bd rdf:type skos:Concept;
  skos:scopeNote """Includes both passages between sections of seats and the side divisions of buildings where the interior is divided into parts by columns or piers """@en;
  skos:exactMatch aat:300004284;
  skos:prefLabel "aisle"@en;
  skos:prefLabel "nef latérale"@fr;
  skos:prefLabel "zijbeuk"@nl;
  skos:prefLabel "seitenschiff"@de;
  skos:inScheme dccd:objectElementType.
dccd:a7a1bb1e-6b80-11e5-aa7b-03d67a84e6dc rdf:type skos:Concept;
  skos:scopeNote """Framing or form made of wood, steel, or plastic that serves as a support during construction, particularly as used to support the load of an arch, vault or dome during construction, for the pouring of liquid concrete in a foundation, and in other contexts."""@en;
  skos:exactMatch aat:300380423;
  skos:prefLabel "formwork"@en;
  skos:altLabel "casing"@en;
  skos:prefLabel "schalung"@de;
  skos:prefLabel "coffrage"@fr;
  skos:prefLabel "bekisting"@nl;
  skos:inScheme dccd:objectElementType.
dccd:a7a1bf74-6b80-11e5-aa7d-6fa6721c0ed1 rdf:type skos:Concept;
  skos:scopeNote """Horizontal stages or levels of a building positioned one above the other and having a habitable or usable room or set of rooms on each level. The term may also refer to horizontal divisions of the exteriors of buildings that typically, but not always, correspond to the levels of interior spaces; exterior indications of stories include tiers or rows of orders, columns, window mullions, or other features disposed horizontally one above another."""@en;
  skos:exactMatch aat:300002667;
  skos:prefLabel "storey"@en;
  skos:prefLabel "étage"@fr;
  skos:prefLabel "stockwerk"@de;
  skos:prefLabel "verdieping"@nl;
  skos:altLabel "geschoss"@de;
  skos:altLabel "stock"@de;
  skos:altLabel "floor"@en;
  skos:altLabel "story"@en;
  skos:inScheme dccd:objectElementType.
dccd:a7a1c0e6-6b80-11e5-aa7f-bf274fdccbce rdf:type skos:Concept;
  skos:scopeNote """Transverse beam cogged or tenoned on wall or arcade plates directly supports a pair of rafters or furnished wit ha rafter plate."""@en;
  skos:broadMatch aat:300001497;
  skos:altLabel "roof-beam"@en;
  skos:prefLabel "dachbalken"@de;
  skos:prefLabel "roof timber"@en;
  skos:prefLabel "poutre toit"@fr;
  skos:prefLabel "dakbalk"@nl;
  skos:inScheme dccd:objectElementType.
dccd:a7a1c19a-6b80-11e5-aa80-93558bd0795b rdf:type skos:Concept;
  skos:broadMatch aat:300001497;
  skos:prefLabel "bundbalken"@de;
  skos:prefLabel "tie beam"@en;
  skos:prefLabel "entrait"@fr;
  skos:prefLabel "gebintbalk"@nl;
  skos:inScheme dccd:objectElementType.
dccd:a7a1c244-6b80-11e5-aa81-4fa1d7cb9225 rdf:type skos:Concept;
  skos:scopeNote """Roof structure whose light rafters are supported by purlins and in particular bear the roofing materials."""@en;
  skos:broadMatch aat:300002098;
  skos:prefLabel "pfettendach"@de;
  skos:prefLabel "side purlin roof"@en;
  skos:prefLabel "charpente à chevrons et pannes"@fr;
  skos:prefLabel "gordingenkap"@nl;
  skos:inScheme dccd:objectElementType.
dccd:a7a1c2ee-6b80-11e5-aa82-1f8acce0948c rdf:type skos:Concept;
  skos:scopeNote """Prehistoric cemetery, typically of Bronze Age and Iron Age Europe. Grave fields are distinguished from necropoleis by the former's lack of above-ground structures, buildings, or grave markers."""@en;
  skos:broadMatch aat:300266755;
  skos:prefLabel "gräberfeld"@de;
  skos:prefLabel "grave field"@en;
  skos:prefLabel "terrain des tombes"@fr;
  skos:prefLabel "grafveld"@nl;
  skos:inScheme dccd:objectElementType.
dccd:a7a1c8de-6b80-11e5-aa8b-67e97dd5e510 rdf:type skos:Concept;
  skos:exactMatch aat:300040444;
  skos:altLabel "running-board"@en;
  skos:prefLabel "trittbrett"@de;
  skos:prefLabel "footboard"@en;
  skos:prefLabel "marchepied"@fr;
  skos:prefLabel "treeplank"@nl;
  skos:inScheme dccd:objectElementType.
dccd:a7a1c97e-6b80-11e5-aa8c-230309882210 rdf:type skos:Concept;
  skos:scopeNote """A piece of art in three panels either placed side by side or hinged together"""@en;
  skos:exactMatch aat:300178234;
  skos:prefLabel "triplik"@de;
  skos:prefLabel "triptych"@en;
  skos:prefLabel "triptyque"@fr;
  skos:prefLabel "triptiek"@nl;
  skos:inScheme dccd:objectElementType.
dccd:a7a1d400-6b80-11e5-aa9c-db85c58837ab rdf:type skos:Concept;
  skos:scopeNote """Generally used for oared fighting ships, principally of the Mediterranean, in operation from the Early Bronze Age until the 18th century CE; most commonly with numerous oars on one or several decks and equipped with a ram with which to damage and sink enemy vessels. For post-18th century steamships equipped with an armored prow as a primary weapon, use 'rams.'"""@en;
  skos:exactMatch aat:300125456;
  skos:altLabel "galeere"@de;
  skos:altLabel "galley"@en;
  skos:altLabel "galère"@fr;
  skos:altLabel "galei"@nl;
  skos:broader dccd:a7a1ba74-6b80-11e5-aa7a-7b1dc4c873b5;
  skos:inScheme dccd:objectElementType.
dccd:a7a1d4b4-6b80-11e5-aa9d-47df7af937f6 rdf:type skos:Concept;
  skos:scopeNote """Parallel beams used to support floor and ceiling loads and supported in turn by larger beams, girders, bearing walls, or other members."""@en;
  skos:exactMatch aat:300001544;
  skos:prefLabel "solive"@fr;
  skos:prefLabel "zwischenbalken"@de;
  skos:altLabel "bintlaag"@nl;
  skos:prefLabel "vloerbalk"@nl;
  skos:altLabel "felderbalken"@de;
  skos:altLabel "poutaison"@fr;
  skos:altLabel "solivage"@fr;
  skos:altLabel "solivure"@fr;
  skos:altLabel "balkenlagen"@de;
  skos:altLabel "bintwerk"@nl;
  skos:altLabel "gebälk"@de;
  skos:altLabel "potrage"@fr;
  skos:altLabel "balklaag"@nl;
  skos:prefLabel "joist"@en;
  skos:inScheme dccd:objectElementType.
dccd:a7a1d572-6b80-11e5-aa9e-475b95e2c6da rdf:type skos:Concept;
  skos:scopeNote """Shipsterm Capacious, flat-bottomed vessels, usually intended to be pushed or towed, primarily for transporting cargo """@en;
  skos:exactMatch aat:300262616;
  skos:prefLabel "kahn"@de;
  skos:prefLabel "barge"@en;
  skos:prefLabel "barge"@fr;
  skos:prefLabel "aak"@nl;
  skos:broader dccd:a7a1ba74-6b80-11e5-aa7a-7b1dc4c873b5;
  skos:inScheme dccd:objectElementType.
dccd:a7a1cba4-6b80-11e5-aa8f-7b893ed983e4 rdf:type skos:Concept;
  skos:scopeNote """Specific type of strake"""@en;
  skos:broadMatch aat:300212614;
  skos:prefLabel "virure de bordage"@fr;
  skos:prefLabel "bottom strake"@en;
  skos:prefLabel "vlakgang"@nl;
  skos:prefLabel "bodengang"@de;
  skos:broader dccd:27171b0a-6c53-11e5-9a23-5739630d10e1;
  skos:inScheme dccd:objectElementType.
dccd:a7a1d356-6b80-11e5-aa9b-8fe3ef82f828 rdf:type skos:Concept;
  skos:scopeNote """Watercraft designed for use on canals generally long and narrow with bow and stern often nearly vertical for increased cargo capacity."""@en;
  skos:exactMatch aat:300212687;
  skos:prefLabel "narrow boat"@en;
  skos:prefLabel "kanaalschip"@nl;
  skos:prefLabel "kanalboot"@de;
  skos:altLabel "canalboat"@en;
  skos:broader dccd:a7a1ba74-6b80-11e5-aa7a-7b1dc4c873b5;
  skos:inScheme dccd:objectElementType.
dccd:a7a1be98-6b80-11e5-aa7c-5f4916f3501e rdf:type skos:Concept;
  skos:scopeNote """Lidded baskets, flat on one side and bulging on the other, intended primarily for holding fish, lobster, tackle, or the like; used especially with reference to those worn on the back or suspended from the shoulder by anglers."""@en;
  skos:exactMatch aat:300194850;
  skos:prefLabel "visben"@nl;
  skos:prefLabel "creel"@en;
  skos:altLabel "viskaar"@nl;
  skos:prefLabel "panier de pêche"@fr;
  skos:altLabel "gatter"@de;
  skos:prefLabel "fischkasten"@de;
  skos:inScheme dccd:objectElementType.
dccd:a7a1c6ea-6b80-11e5-aa88-97f224bfdc83 rdf:type skos:Concept;
  skos:scopeNote """shipsterm """@en;
  skos:broadMatch aat:300212614;
  skos:prefLabel "kombüse"@de;
  skos:prefLabel "cook's galley"@en;
  skos:prefLabel "cuisine de bord"@fr;
  skos:prefLabel "kombuis"@nl;
  skos:inScheme dccd:objectElementType.
dccd:a7a1ce38-6b80-11e5-aa93-b361acdcca4a rdf:type skos:Concept;
  skos:scopeNote """Uppermost complete deck extending from bow to stern"""@en;
  skos:broadMatch aat:300212614;
  skos:prefLabel "großdeck"@de;
  skos:prefLabel "main deck"@en;
  skos:prefLabel "pont principal"@fr;
  skos:prefLabel "overloopdek"@nl;
  skos:inScheme dccd:objectElementType.
dccd:a7a1da90-6b80-11e5-aaa2-abbbc790ddd7 rdf:type skos:Concept;
  skos:scopeNote """Use for buildings equipped with machinery for grinding grain into flour """@en;
  skos:exactMatch aat:300006286;
  skos:altLabel "corn mill"@en;
  skos:prefLabel "flour mill"@en;
  skos:altLabel "moulin à céréales"@fr;
  skos:prefLabel "kornmühle"@de;
  skos:prefLabel "moulin à farine"@fr;
  skos:prefLabel "korenmolen"@nl;
  skos:inScheme dccd:objectElementType.
dccd:a7a1de82-6b80-11e5-aaa8-03e18eb79e22 rdf:type skos:Concept;
  skos:scopeNote """Institutions that are staffed and equipped for the diagnosis of disease, for medical and surgical treatment of the sick and the injured, and for their housing during this process. The modern hospital also often serves as a center for investigation and for teaching."""@en;
  skos:exactMatch aat:300343473;
  skos:prefLabel "ziekenhuis"@nl;
  skos:prefLabel "hôpital"@fr;
  skos:prefLabel "hospital"@en;
  skos:prefLabel "krankenhaus"@de;
  skos:inScheme dccd:objectElementType.
dccd:a7a1e3b4-6b80-11e5-aab0-c76256113241 rdf:type skos:Concept;
  skos:scopeNote """Refers to the horizontal timbers laid across the principal rafters and supporting the common rafters in a roof."""@en;
  skos:exactMatch aat:300002399;
  skos:prefLabel "gording"@nl;
  skos:altLabel "worm"@nl;
  skos:altLabel "filière"@fr;
  skos:altLabel "filière"@fr;
  skos:prefLabel "pfette"@de;
  skos:prefLabel "purlin"@en;
  skos:altLabel "fliering"@nl;
  skos:prefLabel "panne"@fr;
  skos:inScheme dccd:objectElementType.
dccd:a7a1e508-6b80-11e5-aab2-ffd373add096 rdf:type skos:Concept;
  skos:scopeNote """ at the eastern side of the cloister """@en;
  skos:exactMatch aat:300007495;
  skos:prefLabel "abteikirche"@de;
  skos:prefLabel "abbey church"@en;
  skos:prefLabel "abbatiale"@fr;
  skos:prefLabel "abdijkerk"@nl;
  skos:inScheme dccd:objectElementType.
dccd:a7a1e85a-6b80-11e5-aab7-27a784c5bedf rdf:type skos:Concept;
  skos:scopeNote """Structures designed or used for the storage of commodities or merchandise """@en;
  skos:exactMatch aat:300007722;
  skos:altLabel "storehouse"@en;
  skos:altLabel "spijker"@nl;
  skos:prefLabel "warehouse"@en;
  skos:prefLabel "speicher"@de;
  skos:prefLabel "grenier"@fr;
  skos:prefLabel "spieker"@nl;
  skos:inScheme dccd:objectElementType.
dccd:a7a1e8fa-6b80-11e5-aab8-27091bd7ccec rdf:type skos:Concept;
  skos:scopeNote """Use for clearly articulated, often towerlike, building appendages containing only stairs """@en;
  skos:exactMatch aat:300130963;
  skos:altLabel "treppenturm"@de;
  skos:altLabel "stair tower"@en;
  skos:altLabel "staircase turret"@en;
  skos:altLabel "tourelle d'escalier"@fr;
  skos:altLabel "tour-escalier"@fr;
  skos:altLabel "traptoren"@nl;
  skos:inScheme dccd:objectElementType.
dccd:a7a1e9a4-6b80-11e5-aab9-f36d2e9158c6 rdf:type skos:Concept;
  skos:scopeNote """Pendulum-driven floor clocks having cases about 6 feet high or larger, developed in England in the mid-17th century """@en;
  skos:exactMatch aat:300041586;
  skos:altLabel "grandfather clock"@en;
  skos:prefLabel "staande klok"@nl;
  skos:prefLabel "horloge de parquet"@fr;
  skos:prefLabel "standuhr"@de;
  skos:prefLabel "long-case clock"@en;
  skos:inScheme dccd:objectElementType.
dccd:a7a1ea4e-6b80-11e5-aaba-f7315e356c04 rdf:type skos:Concept;
  skos:scopeNote """Use for structures of varying forms in gardens or parks designed to provide cool shady places of relaxation or retreats from summer heat """@en;
  skos:broadMatch aat:300006822;
  skos:altLabel "pavillion"@en;
  skos:altLabel "summerhouse"@en;
  skos:prefLabel "teepavillon"@de;
  skos:prefLabel "pavillon de thé"@fr;
  skos:prefLabel "theekoepel"@nl;
  skos:prefLabel "tea pavillion"@en;
  skos:inScheme dccd:objectElementType.
dccd:a7a1ec4c-6b80-11e5-aabd-77998b69834e rdf:type skos:Concept;
  skos:scopeNote """Refers to the ropes, wires, or chains on watercraft for securing or supporting masts, yards, and for hoisting, lowering, or trimming the sails."""@en;
  skos:exactMatch aat:300213053;
  skos:altLabel "rig"@en;
  skos:prefLabel "rigging"@en;
  skos:prefLabel "gréement"@fr;
  skos:prefLabel "tuig"@nl;
  skos:prefLabel "takelage"@de;
  skos:inScheme dccd:objectElementType.
dccd:a7a1ecf6-6b80-11e5-aabe-733b1edb25b6 rdf:type skos:Concept;
  skos:scopeNote """The strong outer works of a fortification, usually low enough to permit defensive fire"""@en;
  skos:exactMatch aat:300387515;
  skos:altLabel "bolwerk"@nl;
  skos:altLabel "bollwerk"@de;
  skos:prefLabel "verschansing"@nl;
  skos:prefLabel "pavois"@fr;
  skos:prefLabel "bulwark"@en;
  skos:prefLabel "schanzkleid"@de;
  skos:inScheme dccd:objectElementType.
dccd:a7a1eda0-6b80-11e5-aabf-4f74aad96181 rdf:type skos:Concept;
  skos:scopeNote """Openings in the wall of a building, serving to admit light, usually to permit vision, and often to admit air."""@en;
  skos:exactMatch aat:300002944;
  skos:prefLabel "venster"@nl;
  skos:prefLabel "fenêtre"@fr;
  skos:prefLabel "window"@en;
  skos:prefLabel "fenster"@de;
  skos:inScheme dccd:objectElementType.
dccd:a7a1ee4a-6b80-11e5-aac0-f39e6fcad391 rdf:type skos:Concept;
  skos:scopeNote """Use broadly for all sorts of walls constructed to resist attack."""@en;
  skos:exactMatch aat:300002485;
  skos:prefLabel "mauern"@de;
  skos:prefLabel "defensive wall"@en;
  skos:prefLabel "verdedigingsmuur"@nl;
  skos:prefLabel "mur défensif"@fr;
  skos:inScheme dccd:objectElementType.
dccd:a7a1f17e-6b80-11e5-aac5-03f16b00739e rdf:type skos:Concept;
  skos:closeMatch aat:300133704;
  skos:prefLabel "kamer"@nl;
  skos:prefLabel "zimmer"@de;
  skos:prefLabel "room"@en;
  skos:prefLabel "chambre"@fr;
  skos:altLabel "kammer"@de;
  skos:altLabel "raum"@de;
  skos:altLabel "chamber"@en;
  skos:altLabel "pièce"@fr;
  skos:altLabel "vertrek"@nl;
  skos:inScheme dccd:objectElementType.
dccd:a7a1f228-6b80-11e5-aac6-93686ee9d3e0 rdf:type skos:Concept;
  skos:scopeNote """Large, permanent, heavily fortified, defensive military positions, sometimes including a town. Larger and stronger than 'forts.'"""@en;
  skos:exactMatch aat:300006894;
  skos:prefLabel "vesting"@nl;
  skos:prefLabel "forteresse"@fr;
  skos:prefLabel "fortress"@en;
  skos:prefLabel "festung"@de;
  skos:inScheme dccd:objectElementType.
dccd:a7a1f6b0-6b80-11e5-aacd-2b888e92ae79 rdf:type skos:Concept;
  skos:scopeNote """Towers attached to churches"""@en;
  skos:exactMatch aat:300003625;
  skos:altLabel "steeple"@en;
  skos:altLabel "clocher"@fr;
  skos:prefLabel "kirchturm"@de;
  skos:prefLabel "churchtower"@en;
  skos:prefLabel "tour d'une église"@fr;
  skos:prefLabel "kerktoren"@nl;
  skos:inScheme dccd:objectElementType.
dccd:a7a1f75a-6b80-11e5-aace-73b5fb21de31 rdf:type skos:Concept;
  skos:scopeNote """Large boxes with hinged lids intended for the storage of textiles, clothing, and other articles """@en;
  skos:closeMatch aat:300038992;
  skos:altLabel "truhe"@de;
  skos:altLabel "box"@en;
  skos:prefLabel "kiste"@de;
  skos:prefLabel "chest"@en;
  skos:prefLabel "huche"@fr;
  skos:prefLabel "kist"@nl;
  skos:inScheme dccd:objectElementType.
dccd:a7a1f804-6b80-11e5-aacf-570f27e75fec rdf:type skos:Concept;
  skos:scopeNote """Use for the rooms or spaces in which bells are hung in a tower; for the entire tower structure, use 'bell towers.' """@en;
  skos:exactMatch aat:300137347;
  skos:prefLabel "beffroi"@fr;
  skos:prefLabel "belfry"@en;
  skos:prefLabel "glockenstuhl"@de;
  skos:prefLabel "klokkenstoel"@nl;
  skos:inScheme dccd:objectElementType.
dccd:a7a1f8a4-6b80-11e5-aad0-136968eb5e43 rdf:type skos:Concept;
  skos:broadMatch aat:300178758;
  skos:prefLabel "scheibenrad"@de;
  skos:prefLabel "disc wheel"@en;
  skos:prefLabel "roue à toile pleine"@fr;
  skos:prefLabel "schijfwiel"@nl;
  skos:inScheme dccd:objectElementType.
dccd:a7a1d9dc-6b80-11e5-aaa1-437e1e526a7a rdf:type skos:Concept;
  skos:scopeNote """A short horizontal pole projecting from a wall, on which the floorboards of scaffolding rest."""@en;
  skos:exactMatch aat:300263234;
  skos:prefLabel "boulin"@fr;
  skos:prefLabel "putlog"@en;
  skos:prefLabel "gerüstholz"@de;
  skos:prefLabel "korteling"@nl;
  skos:inScheme dccd:objectElementType.
dccd:a7a1f2d2-6b80-11e5-aac7-f7ab70dd5bd4 rdf:type skos:Concept;
  skos:scopeNote """ A framework of interwoven rods, poles, or branches; used with daub as a building material."""@en;
  skos:exactMatch aat:300011888;
  skos:altLabel "vitswerk"@nl;
  skos:prefLabel "wattle"@en;
  skos:prefLabel "vlechtwerk"@nl;
  skos:altLabel "geflecht"@de;
  skos:altLabel "traveau de tressage"@fr;
  skos:altLabel "traveau de nattage"@fr;
  skos:prefLabel "clayonnage"@fr;
  skos:prefLabel "flechtwerk"@de;
  skos:inScheme dccd:objectElementType.
dccd:a7a1dbe4-6b80-11e5-aaa4-7381f7bc04b0 rdf:type skos:Concept;
  skos:scopeNote """Vertical members connecting the apex of a triangular truss, as in a roof, with the base """@en;
  skos:broadMatch aat:300002382;
  skos:altLabel "kaiserstil"@de;
  skos:altLabel "poinçon de croupe"@fr;
  skos:altLabel "koningstijl"@nl;
  skos:altLabel "spitzsäule"@de;
  skos:altLabel "central vertical post"@en;
  skos:altLabel "spire mast"@en;
  skos:altLabel "poinçon"@fr;
  skos:prefLabel "king strut"@en;
  skos:prefLabel "makelaar"@nl;
  skos:prefLabel "spitzständer"@de;
  skos:prefLabel "poinçon (qui ne porte pas la faitière"@fr;
  skos:inScheme dccd:objectElementType.
dccd:a7a1dde2-6b80-11e5-aaa7-f386d8c44f3d rdf:type skos:Concept;
  skos:scopeNote """Hull planking"""@en;
  skos:broadMatch aat:300212614;
  skos:prefLabel "vlakplank"@nl;
  skos:prefLabel "bordage de la carène"@fr;
  skos:prefLabel "bottom plank"@en;
  skos:prefLabel "bodenplanke"@de;
  skos:altLabel "hull plank"@en;
  skos:inScheme dccd:objectElementType.
dccd:a7a1f96c-6b80-11e5-aad1-af8e72a87100 rdf:type skos:Concept;
  skos:scopeNote """Artificial navigable waterways."""@en;
  skos:exactMatch aat:300006075;
  skos:prefLabel "canal"@en;
  skos:prefLabel "canal"@fr;
  skos:prefLabel "kanal"@de;
  skos:prefLabel "kanaal"@nl;
  skos:altLabel "gracht"@nl;
  skos:inScheme dccd:objectElementType.
dccd:a7a206fa-6b80-11e5-aae2-03b9997c048d rdf:type skos:Concept;
  skos:closeMatch aat:300000824;
  skos:prefLabel "abfallgrube"@de;
  skos:prefLabel "waste pit"@en;
  skos:prefLabel "fosse à déchets"@fr;
  skos:prefLabel "afvalkuil"@nl;
  skos:inScheme dccd:objectElementType.
dccd:a7a207a4-6b80-11e5-aae3-c770eb3e56e5 rdf:type skos:Concept;
  skos:scopeNote """Use for constructions upon which religious sacrifice is offered. Includes both small, tablelike fixtures and larger, free-standing, outdoor structures. For the surface at which communion is celebrated in Protestant churches, use 'communion tables.' """@en;
  skos:exactMatch aat:300003725;
  skos:prefLabel "altar"@de;
  skos:prefLabel "altar"@en;
  skos:prefLabel "autel"@fr;
  skos:prefLabel "altaar"@nl;
  skos:inScheme dccd:objectElementType.
dccd:a7a2084e-6b80-11e5-aae4-97359a184c70 rdf:type skos:Concept;
  skos:scopeNote """Religious images on, above, or behind the altar of a Christian church """@en;
  skos:exactMatch aat:300075940;
  skos:prefLabel "altar"@de;
  skos:prefLabel "altarpiece"@en;
  skos:prefLabel "retable"@fr;
  skos:prefLabel "altaarstuk"@nl;
  skos:inScheme dccd:objectElementType.
dccd:a7a208f8-6b80-11e5-aae5-9709414dec40 rdf:type skos:Concept;
  skos:scopeNote """Stringed instrument.  Smallest in the violin family"""@en;
  skos:exactMatch aat:300042215;
  skos:prefLabel "violin"@en;
  skos:prefLabel "violon"@fr;
  skos:prefLabel "viool"@nl;
  skos:prefLabel "violine"@de;
  skos:inScheme dccd:objectElementType.
dccd:a7a209a2-6b80-11e5-aae6-87f34dd417e1 rdf:type skos:Concept;
  skos:exactMatch aat:300263195;
  skos:altLabel "rähm"@de;
  skos:altLabel "basting"@fr;
  skos:prefLabel "bohle"@de;
  skos:prefLabel "board"@en;
  skos:prefLabel "madrier"@fr;
  skos:prefLabel "badding"@nl;
  skos:inScheme dccd:objectElementType.
dccd:a7a20a4c-6b80-11e5-aae7-df8a7c01f739 rdf:type skos:Concept;
  skos:scopeNote """Parapets or low screens composed of balusters and carrying a rail or other horizontal member that is usually heavy in proportion to the balusters themselves """@en;
  skos:exactMatch aat:300001989;
  skos:prefLabel "geländer"@de;
  skos:prefLabel "balustrade"@en;
  skos:prefLabel "balustrade"@fr;
  skos:prefLabel "balustrade"@nl;
  skos:inScheme dccd:objectElementType.
dccd:a7a20af6-6b80-11e5-aae8-e759a16cd4db rdf:type skos:Concept;
  skos:scopeNote """Use for buildings or sets of buildings erected as common living quarters for groups of soldiers or workers"""@en;
  skos:exactMatch aat:300005665;
  skos:altLabel "barrack"@en;
  skos:altLabel "kaserne"@de;
  skos:altLabel "kazerne"@nl;
  skos:prefLabel "baracke"@de;
  skos:prefLabel "barak"@nl;
  skos:prefLabel "barracks"@en;
  skos:prefLabel "caserne"@fr;
  skos:inScheme dccd:objectElementType.
dccd:a7a20ba0-6b80-11e5-aae9-af39bcc68cdd rdf:type skos:Concept;
  skos:scopeNote """shipsterm """@en;
  skos:exactMatch aat:300233046;
  skos:altLabel "bark (ship)"@en;
  skos:prefLabel "kahn"@de;
  skos:prefLabel "barque"@en;
  skos:prefLabel "barque"@fr;
  skos:prefLabel "bark"@nl;
  skos:broader dccd:a7a1ba74-6b80-11e5-aa7a-7b1dc4c873b5;
  skos:inScheme dccd:objectElementType.
dccd:a7a20c4a-6b80-11e5-aaea-af22b1d087a7 rdf:type skos:Concept;
  skos:exactMatch aat:300042216;
  skos:prefLabel "bass"@de;
  skos:prefLabel "double bass"@en;
  skos:prefLabel "basse"@fr;
  skos:prefLabel "bas"@nl;
  skos:inScheme dccd:objectElementType.
dccd:a7a20cea-6b80-11e5-aaeb-3b48181d1012 rdf:type skos:Concept;
  skos:scopeNote """The projecting portions of the outer wall of a fortification """@en;
  skos:exactMatch aat:300002495;
  skos:altLabel "bastei"@de;
  skos:altLabel "bastion"@de;
  skos:altLabel "bulwark"@en;
  skos:altLabel "vallum"@en;
  skos:altLabel "bastion"@nl;
  skos:prefLabel "bollwerk"@de;
  skos:prefLabel "bastion"@en;
  skos:prefLabel "bastion"@fr;
  skos:prefLabel "bolwerk"@nl;
  skos:inScheme dccd:objectElementType.
dccd:a7a20d94-6b80-11e5-aaec-2f78bc5dd7b7 rdf:type skos:Concept;
  skos:scopeNote """Use for works of art in which images and forms are carried out primarily in three dimensions, especially those that retain the quality of being tangible objects or groups of objects. """@en;
  skos:exactMatch aat:300047090;
  skos:altLabel "beeld"@nl;
  skos:prefLabel "skulptur"@de;
  skos:prefLabel "sculpture"@en;
  skos:prefLabel "sculpture"@fr;
  skos:prefLabel "beeldhouwwerk"@nl;
  skos:inScheme dccd:objectElementType.
dccd:a7a20e48-6b80-11e5-aaed-3310364db131 rdf:type skos:Concept;
  skos:exactMatch aat:300052556;
  skos:prefLabel "senkgrube"@de;
  skos:prefLabel "cesspit"@en;
  skos:prefLabel "fosse d'aisances"@fr;
  skos:prefLabel "beerput"@nl;
  skos:inScheme dccd:objectElementType.
dccd:a7a20ee8-6b80-11e5-aaee-8b094e94944d rdf:type skos:Concept;
  skos:scopeNote """Areas used for burial or entombment """@en;
  skos:exactMatch aat:300266755;
  skos:prefLabel "friedhof"@de;
  skos:prefLabel "cemetery"@en;
  skos:prefLabel "cimetière"@fr;
  skos:prefLabel "begraafplaats"@nl;
  skos:inScheme dccd:objectElementType.
dccd:a7a20f92-6b80-11e5-aaef-afc8ef4162cd rdf:type skos:Concept;
  skos:scopeNote """shipsterm """@en;
  skos:exactMatch aat:300012825;
  skos:prefLabel "beplankung"@de;
  skos:prefLabel "planking"@en;
  skos:prefLabel "planchéiage"@fr;
  skos:prefLabel "bekleding"@nl;
  skos:inScheme dccd:objectElementType.
dccd:a7a2117c-6b80-11e5-aaf2-031aa7096b69 rdf:type skos:Concept;
  skos:scopeNote """Decorative or protective facings applied to the lower portion of an interior partition or wall, such as wood paneling; Wall coverings consisting of panels of wood or other material joined in a continuous surface """@en;
  skos:exactMatch aat:300014658;
  skos:altLabel "wainscoting"@en;
  skos:altLabel "lambris"@fr;
  skos:prefLabel "holzverkleidung"@de;
  skos:prefLabel "panelling"@en;
  skos:prefLabel "boiserie"@fr;
  skos:prefLabel "labrisering"@nl;
  skos:inScheme dccd:objectElementType.
dccd:a7a21226-6b80-11e5-aaf3-4ff4cf501724 rdf:type skos:Concept;
  skos:exactMatch aat:300001993;
  skos:altLabel "poller"@de;
  skos:altLabel "rolle"@de;
  skos:altLabel "bitt"@en;
  skos:altLabel "dolphin"@en;
  skos:altLabel "bitte"@fr;
  skos:altLabel "bitte (d'amarrage)"@fr;
  skos:altLabel "bitton"@fr;
  skos:altLabel "beting"@nl;
  skos:prefLabel "beting"@de;
  skos:prefLabel "bollard"@en;
  skos:prefLabel "bollard"@fr;
  skos:prefLabel "bolder"@nl;
  skos:inScheme dccd:objectElementType.
dccd:a7a212d0-6b80-11e5-aaf4-db19f7192b77 rdf:type skos:Concept;
  skos:scopeNote """Use for subsidiary supplementary structures, whether additions to a main building or separate from it, but usually visibly distinct and often with a separate entrance. """@en;
  skos:exactMatch aat:300077063;
  skos:altLabel "dépendance"@fr;
  skos:prefLabel "nebengebäude"@de;
  skos:prefLabel "annex"@en;
  skos:prefLabel "annexe"@fr;
  skos:prefLabel "bijgebouw"@nl;
  skos:inScheme dccd:objectElementType.
dccd:a7a2137a-6b80-11e5-aaf5-7bb1cc12186c rdf:type skos:Concept;
  skos:scopeNote """shipsterm """@en;
  skos:exactMatch aat:300262666;
  skos:altLabel "stringer"@de;
  skos:altLabel "inwale"@en;
  skos:altLabel "stringer"@en;
  skos:altLabel "serre"@fr;
  skos:prefLabel "dollbaum"@de;
  skos:prefLabel "inboard"@en;
  skos:prefLabel "préceinte interne"@fr;
  skos:prefLabel "binnenboord"@nl;
  skos:inScheme dccd:objectElementType.
dccd:a7a21424-6b80-11e5-aaf6-373c7762323d rdf:type skos:Concept;
  skos:scopeNote """shipsterm """@en;
  skos:exactMatch aat:300257611;
  skos:altLabel "block"@en;
  skos:altLabel "blok"@nl;
  skos:prefLabel "block"@de;
  skos:prefLabel "pulley"@en;
  skos:prefLabel "poulie"@fr;
  skos:prefLabel "katrol"@nl;
  skos:inScheme dccd:objectElementType.
dccd:a7a214ce-6b80-11e5-aaf7-bb6b5b679f12 rdf:type skos:Concept;
  skos:exactMatch aat:300005605;
  skos:prefLabel "blockbau"@de;
  skos:prefLabel "log building"@en;
  skos:prefLabel "construction en pièce sur pièce"@fr;
  skos:prefLabel "blokbouw"@nl;
  skos:inScheme dccd:objectElementType.
dccd:a7a21618-6b80-11e5-aaf9-473905d5169b rdf:type skos:Concept;
  skos:scopeNote """shipsterm """@en;
  skos:exactMatch aat:300184745;
  skos:prefLabel "galionsfigur"@de;
  skos:prefLabel "figurehead"@en;
  skos:prefLabel "figure de proue"@fr;
  skos:prefLabel "boegbeeld"@nl;
  skos:inScheme dccd:objectElementType.
dccd:a7a21762-6b80-11e5-aafb-43033fc42c9e rdf:type skos:Concept;
  skos:scopeNote """Complexes where plants or animals are raised for livelihood or commerce """@en;
  skos:exactMatch aat:300005574;
  skos:prefLabel "bauernhof"@de;
  skos:prefLabel "farmhouse"@en;
  skos:prefLabel "ferme"@fr;
  skos:prefLabel "boerderij"@nl;
  skos:inScheme dccd:objectElementType.
dccd:a7a218b6-6b80-11e5-aafd-231cef94b760 rdf:type skos:Concept;
  skos:exactMatch aat:300004790;
  skos:altLabel "édifice"@fr;
  skos:prefLabel "gebäude"@de;
  skos:prefLabel "building"@en;
  skos:prefLabel "bâtiment"@fr;
  skos:prefLabel "gebouw"@nl;
  skos:inScheme dccd:objectElementType.
dccd:a7a21956-6b80-11e5-aafe-671430d308ae rdf:type skos:Concept;
  skos:scopeNote """shipsterm """@en;
  skos:exactMatch aat:300007951;
  skos:altLabel "gemak"@nl;
  skos:prefLabel "latrine"@de;
  skos:prefLabel "latrine"@en;
  skos:prefLabel "latrine"@fr;
  skos:prefLabel "latrine"@nl;
  skos:inScheme dccd:objectElementType.
dccd:a7a1ff20-6b80-11e5-aad6-07f78bf76f67 rdf:type skos:Concept;
  skos:scopeNote """Beam integrated into a hanging or strutted frame, has to resist high tension forces"""@en;
  skos:exactMatch aat:300002419;
  skos:prefLabel "trekplaat"@nl;
  skos:prefLabel "tie beam"@en;
  skos:prefLabel "entrait"@fr;
  skos:prefLabel "spannbalken"@de;
  skos:altLabel "zugbalken"@de;
  skos:inScheme dccd:objectElementType.
dccd:a7a20268-6b80-11e5-aadb-b39c90c3cd65 rdf:type skos:Concept;
  skos:scopeNote """Paired timber below the roof plane, which is an element of a trasverse fram.  It supports purlines and the roof cladding."""@en;
  skos:exactMatch aat:300002440;
  skos:prefLabel "principal rafter"@en;
  skos:prefLabel "arbalétrier"@fr;
  skos:prefLabel "untersparren"@de;
  skos:prefLabel "spantbeen"@nl;
  skos:inScheme dccd:objectElementType.
dccd:a7a21032-6b80-11e5-aaf0-938dac5fca3a rdf:type skos:Concept;
  skos:scopeNote """Nonstructural, outer, exterior wall covering of buildings."""@en;
  skos:exactMatch aat:300014861;
  skos:prefLabel "dachschalung"@de;
  skos:prefLabel "boarded cladding"@en;
  skos:prefLabel "voligeage"@fr;
  skos:prefLabel "dakbeschot"@nl;
  skos:altLabel "siding (material)"@en;
  skos:inScheme dccd:objectElementType.
dccd:a7a2156e-6b80-11e5-aaf8-d72532287456 rdf:type skos:Concept;
  skos:broadMatch aat:300212614;
  skos:altLabel "boden"@de;
  skos:altLabel "fond"@fr;
  skos:altLabel "sole"@fr;
  skos:altLabel "bodem"@nl;
  skos:prefLabel "vlak"@nl;
  skos:prefLabel "schiffsboden"@de;
  skos:prefLabel "bottom (floor)"@en;
  skos:prefLabel "carène"@fr;
  skos:inScheme dccd:objectElementType.
dccd:a7a210dc-6b80-11e5-aaf1-c33401547327 rdf:type skos:Concept;
  skos:scopeNote """Walls that are constructed to resist lateral loads, such as walls that hold back banks of earth."""@en;
  skos:exactMatch aat:300005073;
  skos:prefLabel "paroi de soutènement"@fr;
  skos:prefLabel "wandbeschoeiing"@nl;
  skos:altLabel "revetment wall"@en;
  skos:prefLabel "retaining wall"@en;
  skos:altLabel "revêtement mural"@fr;
  skos:prefLabel "stützmauer"@de;
  skos:inScheme dccd:objectElementType.
dccd:a7a216b8-6b80-11e5-aafa-630e988a1afb rdf:type skos:Concept;
  skos:scopeNote """Top edge of the side of a boat"""@en;
  skos:exactMatch aat:300387515;
  skos:altLabel "wash strake"@en;
  skos:altLabel "coulisses"@fr;
  skos:altLabel "boeisel"@nl;
  skos:prefLabel "dollbord"@de;
  skos:altLabel "bulwark"@en;
  skos:altLabel "opboeisel"@nl;
  skos:prefLabel "dolboord"@nl;
  skos:prefLabel "gunwale"@en;
  skos:prefLabel "plat-bord"@fr;
  skos:inScheme dccd:objectElementType.
dccd:a7a21a00-6b80-11e5-aaff-5b6dd7cf9be2 rdf:type skos:Concept;
  skos:scopeNote """Use for simple watercraft constructed by hollowing out and carving a single log; found in cultures all over the world and developed at least during the Paleolithic era """@en;
  skos:exactMatch aat:300212722;
  skos:prefLabel "einbaum"@de;
  skos:prefLabel "dugout"@en;
  skos:prefLabel "boomstamkano"@nl;
  skos:prefLabel "piroque monoxyle"@fr;
  skos:inScheme dccd:objectElementType.
dccd:a7a21cda-6b80-11e5-ab00-0f0715311ad9 rdf:type skos:Concept;
  skos:scopeNote """Horizontal structural members that span an opening in a wall and that carry the superimposed weight of the wall """@en;
  skos:exactMatch aat:300003161;
  skos:prefLabel "sturz"@de;
  skos:prefLabel "lintel"@en;
  skos:prefLabel "linteau"@fr;
  skos:prefLabel "latei"@nl;
  skos:inScheme dccd:objectElementType.
dccd:a7a21dc0-6b80-11e5-ab01-e784143b85e4 rdf:type skos:Concept;
  skos:scopeNote """Structures spanning and providing passage over waterways, topographic depressions, transportation routes, or similar circulation barriers """@en;
  skos:exactMatch aat:300007836;
  skos:prefLabel "brücke"@de;
  skos:prefLabel "bridge"@en;
  skos:prefLabel "pont"@fr;
  skos:prefLabel "brug"@nl;
  skos:inScheme dccd:objectElementType.
dccd:a7a21e6a-6b80-11e5-ab02-4f85fec033c5 rdf:type skos:Concept;
  skos:scopeNote """shipsterm """@en;
  skos:broadMatch aat:300263189;
  skos:prefLabel "oberdeck"@de;
  skos:prefLabel "upper deck"@en;
  skos:prefLabel "pont supérieur"@fr;
  skos:prefLabel "bovendek"@nl;
  skos:inScheme dccd:objectElementType.
dccd:a7a21fc8-6b80-11e5-ab04-7316a38eb4c3 rdf:type skos:Concept;
  skos:closeMatch aat:300197197;
  skos:prefLabel "dose"@de;
  skos:prefLabel "box"@en;
  skos:prefLabel "boîte"@fr;
  skos:prefLabel "doos"@nl;
  skos:inScheme dccd:objectElementType.
dccd:a7a22112-6b80-11e5-ab06-8f4da5958741 rdf:type skos:Concept;
  skos:scopeNote """Generally, the rear portions of watercraft."""@en;
  skos:exactMatch aat:300262678;
  skos:altLabel "achtersteven"@de;
  skos:prefLabel "hintersteven"@de;
  skos:prefLabel "stern"@en;
  skos:prefLabel "étambot"@fr;
  skos:prefLabel "achtersteven"@nl;
  skos:inScheme dccd:objectElementType.
dccd:a7a22310-6b80-11e5-ab09-233eab22434f rdf:type skos:Concept;
  skos:exactMatch aat:300038697;
  skos:prefLabel "bett"@de;
  skos:prefLabel "bed"@en;
  skos:prefLabel "lit"@fr;
  skos:prefLabel "bed"@nl;
  skos:inScheme dccd:objectElementType.
dccd:a7a2245a-6b80-11e5-ab0b-13dcf3d23b15 rdf:type skos:Concept;
  skos:scopeNote """Foremost end of a beam or joist which is usually visible as poart of the façade and often decorated."""@en;
  skos:broadMatch aat:300001497;
  skos:altLabel "balkenende"@de;
  skos:prefLabel "balkenköpf"@de;
  skos:prefLabel "beam end"@en;
  skos:prefLabel "about"@fr;
  skos:prefLabel "balkkop"@nl;
  skos:inScheme dccd:objectElementType.
dccd:a7a22504-6b80-11e5-ab0c-73197baed170 rdf:type skos:Concept;
  skos:scopeNote """shipsterm. A structural crosspiece sometimes forming a seat for a rower"""@en;
  skos:broadMatch aat:300212614;
  skos:prefLabel "ruderbank"@de;
  skos:prefLabel "thwart"@en;
  skos:prefLabel "banc de nage"@fr;
  skos:prefLabel "roeibank"@nl;
  skos:inScheme dccd:objectElementType.
dccd:a7a225a4-6b80-11e5-ab0d-afd5893ffec6 rdf:type skos:Concept;
  skos:scopeNote """Short horizontal timber lying across a wall top which receives the end of a rafter"""@en;
  skos:broadMatch aat:300002382;
  skos:prefLabel "sattelbalken"@de;
  skos:prefLabel "sole piece"@en;
  skos:prefLabel "blochet"@fr;
  skos:prefLabel "blokkeel"@nl;
  skos:inScheme dccd:objectElementType.
dccd:a7a226f8-6b80-11e5-ab0f-338af312608a rdf:type skos:Concept;
  skos:scopeNote """Central woody stem of a tree"""@en;
  skos:broadMatch aat:300375171;
  skos:altLabel "stam"@nl;
  skos:prefLabel "stamm"@de;
  skos:prefLabel "(tree-)trunk"@en;
  skos:prefLabel "tronc"@fr;
  skos:prefLabel "boomstam"@nl;
  skos:inScheme dccd:objectElementType.
dccd:a7a228f6-6b80-11e5-ab12-ef3ddd8efce1 rdf:type skos:Concept;
  skos:scopeNote """Use for buildings or groups of buildings intended primarily to serve as a fortified residence of a prince or nobleman """@en;
  skos:exactMatch aat:300006891;
  skos:altLabel "burg"@de;
  skos:altLabel "burcht"@nl;
  skos:altLabel "château"@fr;
  skos:prefLabel "castle"@en;
  skos:prefLabel "château fort"@fr;
  skos:prefLabel "kasteel"@nl;
  skos:prefLabel "kastell"@de;
  skos:inScheme dccd:objectElementType.
dccd:a7a22996-6b80-11e5-ab13-bfb96fa50660 rdf:type skos:Concept;
  skos:scopeNote """Small, ancient Roman fortified towns or outposts """@en;
  skos:exactMatch aat:300008450;
  skos:prefLabel "castellum"@de;
  skos:prefLabel "castellum"@en;
  skos:prefLabel "castellum"@fr;
  skos:prefLabel "castellum"@nl;
  skos:inScheme dccd:objectElementType.
dccd:a7a22a40-6b80-11e5-ab14-3f630f3ccb52 rdf:type skos:Concept;
  skos:exactMatch aat:300209202;
  skos:prefLabel "cello"@de;
  skos:prefLabel "cello"@en;
  skos:prefLabel "violoncelle"@fr;
  skos:prefLabel "cello"@nl;
  skos:inScheme dccd:objectElementType.
dccd:a7a22b8a-6b80-11e5-ab16-47bca7020ecc rdf:type skos:Concept;
  skos:scopeNote """Largest and lowest-pitched instruments of the violin family, having four, or more rarely, five strings, and varying considerably in size and shape. """@en;
  skos:exactMatch aat:300042216;
  skos:prefLabel "kontrabass"@de;
  skos:prefLabel "double bass"@en;
  skos:prefLabel "contrebasse"@fr;
  skos:prefLabel "contrabas"@nl;
  skos:inScheme dccd:objectElementType.
dccd:a7a22c34-6b80-11e5-ab17-87ee6d5c0187 rdf:type skos:Concept;
  skos:scopeNote """Use for barriers to confine, control, or obstruct the flow of water """@en;
  skos:exactMatch aat:300006084;
  skos:prefLabel "damm"@de;
  skos:prefLabel "dam"@en;
  skos:prefLabel "digue"@fr;
  skos:prefLabel "dam"@nl;
  skos:inScheme dccd:objectElementType.
dccd:a7a22e28-6b80-11e5-ab1a-bf248ca1c87c rdf:type skos:Concept;
  skos:scopeNote """Barriers which swing, slide, tilt, or fold to close a doorway, usually of solid and finished construction and usually leading to or separating interior spaces. Use also for similar features that close a container or a piece of case furniture. For barriers of less solid or finished construction, and usually separating two exterior spaces, use 'gates.'"""@en;
  skos:exactMatch aat:300002803;
  skos:prefLabel "tür"@de;
  skos:prefLabel "door"@en;
  skos:prefLabel "porte"@fr;
  skos:prefLabel "deur"@nl;
  skos:inScheme dccd:objectElementType.
dccd:a7a22ed2-6b80-11e5-ab1b-6f3f7fe4f155 rdf:type skos:Concept;
  skos:scopeNote """Assemblies built into a wall, consisting of two upright members (doorjambs) and a horizontal member (doorhead) and providing support on which to hang the door """@en;
  skos:exactMatch aat:300002785;
  skos:altLabel "chambranle"@fr;
  skos:prefLabel "türstock"@de;
  skos:prefLabel "door frame"@en;
  skos:prefLabel "cadre de porte"@fr;
  skos:prefLabel "deurkozijn"@nl;
  skos:inScheme dccd:objectElementType.
dccd:a7a22f7c-6b80-11e5-ab1c-4bc325430632 rdf:type skos:Concept;
  skos:exactMatch aat:300069081;
  skos:altLabel "türpfosten"@de;
  skos:altLabel "door post"@en;
  skos:prefLabel "türständer"@de;
  skos:prefLabel "door jamb"@en;
  skos:prefLabel "piédroit d'une porte"@fr;
  skos:prefLabel "deurstijl"@nl;
  skos:inScheme dccd:objectElementType.
dccd:a7a23026-6b80-11e5-ab1d-6b5cd5ffbeca rdf:type skos:Concept;
  skos:scopeNote """Use for embankments built along a river or sea and set at some distance from it to control or retain flood waters. For embankments built only to prevent flooding of low-lying land use 'levees.' """@en;
  skos:exactMatch aat:300170882;
  skos:prefLabel "deich"@de;
  skos:prefLabel "dike"@en;
  skos:prefLabel "digue"@fr;
  skos:prefLabel "dijk"@nl;
  skos:inScheme dccd:objectElementType.
dccd:a7a23170-6b80-11e5-ab1f-739f81c2d49c rdf:type skos:Concept;
  skos:scopeNote """The strongest and securest parts of castles, often used as residences """@en;
  skos:exactMatch aat:300003694;
  skos:altLabel "turmburg"@de;
  skos:prefLabel "donjon"@de;
  skos:prefLabel "keep"@en;
  skos:prefLabel "donjon"@fr;
  skos:prefLabel "donjon"@nl;
  skos:inScheme dccd:objectElementType.
dccd:a7a23210-6b80-11e5-ab20-0b39385c7414 rdf:type skos:Concept;
  skos:exactMatch aat:300197585;
  skos:prefLabel "sarg"@de;
  skos:prefLabel "coffin"@en;
  skos:prefLabel "cercueil"@fr;
  skos:prefLabel "doodkist"@nl;
  skos:inScheme dccd:objectElementType.
dccd:a7a232ba-6b80-11e5-ab21-07bb844f9fc5 rdf:type skos:Concept;
  skos:scopeNote """Strips fastened to the floor beneath a door, usually required to cover the joint when two types of floor material meet; may provide weather protection on external doors; for the lower sides and bottom of doorways, use 'doorsills'"""@en;
  skos:exactMatch aat:300002800;
  skos:altLabel "schwell"@de;
  skos:altLabel "türschwelle"@de;
  skos:altLabel "doorstep"@en;
  skos:altLabel "sill"@en;
  skos:altLabel "seuil de porte"@fr;
  skos:altLabel "dorpel"@nl;
  skos:altLabel "onderdorpel"@nl;
  skos:altLabel "voetplaat"@nl;
  skos:prefLabel "schwelle"@de;
  skos:prefLabel "threshold"@en;
  skos:prefLabel "seuil"@fr;
  skos:prefLabel "drempel"@nl;
  skos:inScheme dccd:objectElementType.
dccd:a7a23364-6b80-11e5-ab22-eff9c2a3f34b rdf:type skos:Concept;
  skos:scopeNote """Use for drainage structures that extend across and beneath roadways, canals, embankments, or traveled ways other than bridges. """@en;
  skos:exactMatch aat:300006116;
  skos:prefLabel "düker"@de;
  skos:prefLabel "culvert"@en;
  skos:prefLabel "ponceau"@fr;
  skos:prefLabel "duiker"@nl;
  skos:inScheme dccd:objectElementType.
dccd:a7a2340e-6b80-11e5-ab23-cb99667f375d rdf:type skos:Concept;
  skos:exactMatch aat:300001525;
  skos:altLabel "quergurt"@de;
  skos:altLabel "querriegel"@de;
  skos:altLabel "quervergurtung"@de;
  skos:altLabel "transverse timber"@en;
  skos:altLabel "barrot"@fr;
  skos:altLabel "poutre transversale"@fr;
  skos:altLabel "dwarshout"@nl;
  skos:prefLabel "querbalken"@de;
  skos:prefLabel "sommier transversal"@fr;
  skos:prefLabel "cross beam"@en;
  skos:prefLabel "dwarsbalk"@nl;
  skos:inScheme dccd:objectElementType.
dccd:a7a234b8-6b80-11e5-ab24-e366a2f6f212 rdf:type skos:Concept;
  skos:scopeNote """Transverse arms of cruciform churches A series of steps or flights of steps connected by landings for passing from one level to another """@en;
  skos:exactMatch aat:300004645;
  skos:altLabel "querschiff"@de;
  skos:altLabel "dwarsschip"@nl;
  skos:prefLabel "kreuzschiff"@de;
  skos:prefLabel "transept"@en;
  skos:prefLabel "transept"@fr;
  skos:prefLabel "transept"@nl;
  skos:inScheme dccd:objectElementType.
dccd:a7a23562-6b80-11e5-ab25-0f4dcd1c05e8 rdf:type skos:Concept;
  skos:scopeNote """Use for those parts of structures, usually located below ground level, that transmit building loads to the soil or rock underneath; when specifically distinguishing the support systems and areas of structures below ground, including the foundation, from the above-ground portions, use 'substructures.'"""@en;
  skos:exactMatch aat:300000919;
  skos:prefLabel "fundament"@de;
  skos:prefLabel "foundation"@en;
  skos:prefLabel "fondation"@fr;
  skos:prefLabel "fundering"@nl;
  skos:inScheme dccd:objectElementType.
dccd:a7a23602-6b80-11e5-ab26-2719b631ebe1 rdf:type skos:Concept;
  skos:exactMatch aat:300000923;
  skos:prefLabel "gründungspfahl"@de;
  skos:prefLabel "foundation pile"@en;
  skos:prefLabel "pilot de fondation"@fr;
  skos:prefLabel "funderingspaal"@nl;
  skos:inScheme dccd:objectElementType.
dccd:a7a236ac-6b80-11e5-ab27-6f988d915f57 rdf:type skos:Concept;
  skos:scopeNote """Implements punishment for hanging criminals, consisting of two, three or four poles connected by a crossbar and equipped with nooses."""@en;
  skos:exactMatch aat:300266883;
  skos:prefLabel "galgen"@de;
  skos:prefLabel "gallow"@en;
  skos:prefLabel "potence"@fr;
  skos:prefLabel "galg"@nl;
  skos:inScheme dccd:objectElementType.
dccd:a7a2264e-6b80-11e5-ab0e-ff0eba6d3e67 rdf:type skos:Concept;
  skos:scopeNote """The fronts or forwardmost ends of watercraft"""@en;
  skos:exactMatch aat:300248152;
  skos:prefLabel "bug"@de;
  skos:prefLabel "proue"@fr;
  skos:prefLabel "boeg"@nl;
  skos:altLabel "prow"@en;
  skos:prefLabel "bow"@en;
  skos:inScheme dccd:objectElementType.
dccd:a7a221bc-6b80-11e5-ab07-030941e66f8c rdf:type skos:Concept;
  skos:scopeNote """The rear part of a ship"""@en;
  skos:broadMatch aat:300212614;
  skos:altLabel "heck"@de;
  skos:altLabel "quarter"@en;
  skos:prefLabel "hinterschiff"@de;
  skos:prefLabel "l'arrière du vaisseau"@fr;
  skos:prefLabel "achterschip"@nl;
  skos:prefLabel "aft"@en;
  skos:inScheme dccd:objectElementType.
dccd:a7a22d88-6b80-11e5-ab19-9f0c2a16a829 rdf:type skos:Concept;
  skos:scopeNote """Plank used to form the deck of a boat"""@en;
  skos:broadMatch aat:300212614;
  skos:prefLabel "decksplanke"@de;
  skos:prefLabel "deckplank"@en;
  skos:prefLabel "bordage de pont"@fr;
  skos:prefLabel "dekplank"@nl;
  skos:inScheme dccd:objectElementType.
dccd:a7a237f6-6b80-11e5-ab29-6308fe52a0ff rdf:type skos:Concept;
  skos:scopeNote """Use for passages affording entrance to the rooms of a building"""@en;
  skos:exactMatch aat:300004294;
  skos:altLabel "corridor"@en;
  skos:prefLabel "gang"@de;
  skos:prefLabel "hallway"@en;
  skos:prefLabel "couloir"@fr;
  skos:prefLabel "gang"@nl;
  skos:inScheme dccd:objectElementType.
dccd:a7a23c38-6b80-11e5-ab2c-03574548406f rdf:type skos:Concept;
  skos:scopeNote """Narrow boards used to build up a curved surface """@en;
  skos:exactMatch aat:300014680;
  skos:prefLabel "daube"@de;
  skos:prefLabel "stave"@en;
  skos:prefLabel "douelle"@fr;
  skos:prefLabel "duig"@nl;
  skos:inScheme dccd:objectElementType.
dccd:a7a23cec-6b80-11e5-ab2d-37c99bdad629 rdf:type skos:Concept;
  skos:scopeNote """The covering, usually wood boards, plywood, or wallboard, placed over the exterior studding or rafters of a building; provides a base for the application of wall or roof siding."""@en;
  skos:exactMatch aat:300014900;
  skos:altLabel "doublage"@fr;
  skos:altLabel "huidbeplating"@nl;
  skos:prefLabel "plankenbeslag"@de;
  skos:prefLabel "sheathing"@en;
  skos:prefLabel "revêtement"@fr;
  skos:prefLabel "dubbeling"@nl;
  skos:inScheme dccd:objectElementType.
dccd:a7a23eae-6b80-11e5-ab2e-4fcae47a03e2 rdf:type skos:Concept;
  skos:scopeNote """Remains of a tree when it has been cut down"""@en;
  skos:broadMatch aat:300375171;
  skos:prefLabel "baumstumpf"@de;
  skos:prefLabel "tree stump"@en;
  skos:prefLabel "souche"@fr;
  skos:prefLabel "boomstronk"@nl;
  skos:inScheme dccd:objectElementType.
dccd:a7a23f80-6b80-11e5-ab2f-cfb996b6cf65 rdf:type skos:Concept;
  skos:scopeNote """Use for those surfaces or portions of objects that face forward or are regarded as the most important or useful. For the adjective describing the location of something at or near the front of something, use 'front' from the Attributes and Properties hierarchy; Use for those exterior faces of a building which are substantially in one plane and seem to have been designed with special regard to their conspicuousness or association with entrance. Distinct from 'elevations (building divisions),' which may constitute any side or face of a building or large interior space"""@en;
  skos:exactMatch aat:300002526;
  skos:altLabel "gevel"@nl;
  skos:altLabel "pui"@nl;
  skos:prefLabel "giebel"@de;
  skos:prefLabel "façade"@en;
  skos:prefLabel "façade"@fr;
  skos:prefLabel "voorgevel"@nl;
  skos:inScheme dccd:objectElementType.
dccd:a7a24034-6b80-11e5-ab30-3bafcc09ae77 rdf:type skos:Concept;
  skos:exactMatch aat:300001324;
  skos:prefLabel "gewölbe"@de;
  skos:prefLabel "vault"@en;
  skos:prefLabel "voûte"@fr;
  skos:prefLabel "gewelf"@nl;
  skos:inScheme dccd:objectElementType.
dccd:a7a240de-6b80-11e5-ab31-3f3010557bc2 rdf:type skos:Concept;
  skos:exactMatch aat:300042025;
  skos:prefLabel "gitarre"@de;
  skos:prefLabel "guitar"@en;
  skos:prefLabel "guitare"@fr;
  skos:prefLabel "gitaar"@nl;
  skos:inScheme dccd:objectElementType.
dccd:a7a24188-6b80-11e5-ab32-e3504b08f149 rdf:type skos:Concept;
  skos:scopeNote """Storehouses or other repositories for grain, especially after it has been threshed or husked; sometimes also used to store corn """@en;
  skos:exactMatch aat:300004929;
  skos:prefLabel "getreidespeicher"@de;
  skos:prefLabel "granary"@en;
  skos:prefLabel "grange"@fr;
  skos:prefLabel "graanschuur"@nl;
  skos:inScheme dccd:objectElementType.
dccd:a7a24228-6b80-11e5-ab33-b35d8e4f08a0 rdf:type skos:Concept;
  skos:scopeNote """Excavations in the earth used for burial; for constructions raised over or around burial sites, use 'tombs.' """@en;
  skos:exactMatch aat:300005907;
  skos:prefLabel "grab"@de;
  skos:prefLabel "grave"@en;
  skos:prefLabel "sépulture"@fr;
  skos:prefLabel "graf"@nl;
  skos:inScheme dccd:objectElementType.
dccd:a7a242d2-6b80-11e5-ab34-bf914e9572a7 rdf:type skos:Concept;
  skos:exactMatch aat:300236072;
  skos:prefLabel "sattelholz"@de;
  skos:prefLabel "bolster"@en;
  skos:prefLabel "chapeau"@fr;
  skos:prefLabel "sleutelstuk"@nl;
  skos:inScheme dccd:objectElementType.
dccd:a7a2437c-6b80-11e5-ab35-1f9ef4aefe4f rdf:type skos:Concept;
  skos:scopeNote """Mansions belonging to, or used by, the lord of a manor"""@en;
  skos:exactMatch aat:300005579;
  skos:prefLabel "demeure"@fr;
  skos:prefLabel "herrenhaus"@de;
  skos:altLabel "versterkt huis"@nl;
  skos:prefLabel "manor house"@en;
  skos:prefLabel "buitenplaats"@nl;
  skos:altLabel "manor"@en;
  skos:inScheme dccd:objectElementType.
dccd:a7a244c6-6b80-11e5-ab37-db050af39099 rdf:type skos:Concept;
  skos:scopeNote """Rafters which are at right angles to the eaves of a roof and extend from the plate to the ridgeboard """@en;
  skos:closeMatch aat:300002424;
  skos:altLabel "dachsparren"@de;
  skos:altLabel "rafe"@de;
  skos:altLabel "rofe"@de;
  skos:altLabel "common rafter"@en;
  skos:altLabel "spar"@en;
  skos:altLabel "dakspoor"@nl;
  skos:altLabel "keper"@nl;
  skos:altLabel "spar"@nl;
  skos:prefLabel "sparren"@de;
  skos:prefLabel "rafter"@en;
  skos:prefLabel "chevron"@fr;
  skos:prefLabel "spoor"@nl;
  skos:inScheme dccd:objectElementType.
dccd:a7a24570-6b80-11e5-ab38-038b649415d6 rdf:type skos:Concept;
  skos:scopeNote """Beam running transversely across a building tying together two or more parts of a structure"""@en;
  skos:broadMatch aat:300001497;
  skos:altLabel "deckbalken"@de;
  skos:prefLabel "deckbinderbalken"@de;
  skos:prefLabel "superimposed tiebeam"@en;
  skos:prefLabel "solive"@fr;
  skos:prefLabel "dekbalk"@nl;
  skos:inScheme dccd:objectElementType.
dccd:a7a2461a-6b80-11e5-ab39-6349af355cf8 rdf:type skos:Concept;
  skos:broadMatch aat:300001497;
  skos:prefLabel "tragbalken"@de;
  skos:prefLabel "supporting beam"@en;
  skos:prefLabel "poutre"@fr;
  skos:prefLabel "draagbalk"@nl;
  skos:inScheme dccd:objectElementType.
dccd:a7a246ba-6b80-11e5-ab3a-3f1c0aa96493 rdf:type skos:Concept;
  skos:scopeNote """shipsterm """@en;
  skos:exactMatch aat:300002022;
  skos:prefLabel "handlauf"@de;
  skos:prefLabel "handrail"@en;
  skos:prefLabel "main courante"@fr;
  skos:prefLabel "handlijst"@nl;
  skos:inScheme dccd:objectElementType.
dccd:a7a24764-6b80-11e5-ab3b-d36a7e0aaa6b rdf:type skos:Concept;
  skos:scopeNote """Horizontal members which tie together and stiffen two opposite rafters, usually at a point about halfway up the rafters. """@en;
  skos:exactMatch aat:300078937;
  skos:altLabel "collar"@en;
  skos:prefLabel "kehlbalken"@de;
  skos:prefLabel "collar beam"@en;
  skos:prefLabel "petit-entrait"@fr;
  skos:prefLabel "hanenbalk"@nl;
  skos:inScheme dccd:objectElementType.
dccd:a7a24804-6b80-11e5-ab3c-e789163eed6c rdf:type skos:Concept;
  skos:exactMatch aat:300004575;
  skos:prefLabel "heiligtum"@de;
  skos:prefLabel "sanctuary"@en;
  skos:prefLabel "sanctuaire"@fr;
  skos:prefLabel "heiligdom"@nl;
  skos:inScheme dccd:objectElementType.
dccd:a7a248ae-6b80-11e5-ab3d-8f2c726266cc rdf:type skos:Concept;
  skos:scopeNote """Use for piles driven into position at the site """@en;
  skos:exactMatch aat:300000948;
  skos:prefLabel "rammpfahl"@de;
  skos:prefLabel "driven pile"@en;
  skos:prefLabel "pilot"@fr;
  skos:prefLabel "heipaal"@nl;
  skos:inScheme dccd:objectElementType.
dccd:a7a249ee-6b80-11e5-ab3f-cfe14f6349a7 rdf:type skos:Concept;
  skos:scopeNote """Designates ancient Roman storage buildings or warehouses, commonly used as granaries or for wine storage """@en;
  skos:exactMatch aat:300120504;
  skos:prefLabel "horreum"@de;
  skos:prefLabel "horreum"@en;
  skos:prefLabel "horreum"@fr;
  skos:prefLabel "horreum"@nl;
  skos:inScheme dccd:objectElementType.
dccd:a7a24c82-6b80-11e5-ab43-87d2a39ba864 rdf:type skos:Concept;
  skos:scopeNote """Images produced in the Eastern Rite churches, since the 6th century, according to prescribed formulas of subject (Christ, the Virgin, saints, and the great feasts) and composition, for devotional use in the church or home. Most commonly tempera on panel, but may be in any two-dimensional or relief medium, including fresco."""@en;
  skos:exactMatch aat:300033945;
  skos:prefLabel "ikone"@de;
  skos:prefLabel "icon"@en;
  skos:prefLabel "icône"@fr;
  skos:prefLabel "icoon"@nl;
  skos:inScheme dccd:objectElementType.
dccd:a7a24e76-6b80-11e5-ab46-bb78bbf94d92 rdf:type skos:Concept;
  skos:scopeNote """Shaped wooden bars resting on the shoulders of one or more animals to allow them to pull together, especially for drawing a plow or a load """@en;
  skos:exactMatch aat:300255560;
  skos:prefLabel "joch"@de;
  skos:prefLabel "yoke"@en;
  skos:prefLabel "joug"@fr;
  skos:prefLabel "juk"@nl;
  skos:inScheme dccd:objectElementType.
dccd:a7a24fc0-6b80-11e5-ab48-3b0d498a7626 rdf:type skos:Concept;
  skos:scopeNote """Case furniture consisting of a set of shelves, small drawers, or pigeonholes, fronted by one or more doors, and intended for the storage and sometimes the display of small objects. Also, similar built-in or fitted cases often designed for specific purposes, as in a kitchen or bathroom."""@en;
  skos:exactMatch aat:300038888;
  skos:prefLabel "kabinettschrank"@de;
  skos:prefLabel "cabinet"@en;
  skos:prefLabel "cabinet"@fr;
  skos:prefLabel "kabinet"@nl;
  skos:inScheme dccd:objectElementType.
dccd:a7a25060-6b80-11e5-ab49-bfcd805f1279 rdf:type skos:Concept;
  skos:scopeNote """Use for the outside, overhead enclosures of buildings or other structures, including the roofing and its structural framing """@en;
  skos:exactMatch aat:300002098;
  skos:prefLabel "roof"@en;
  skos:prefLabel "charpente"@fr;
  skos:prefLabel "kap"@nl;
  skos:prefLabel "dach"@de;
  skos:inScheme dccd:objectElementType.
dccd:a7a2510a-6b80-11e5-ab4a-7becef25d48f rdf:type skos:Concept;
  skos:scopeNote """Rooms or buildings that serve as sanctuaries or places of Christian worship. A chapel may be used for private worship in or attached to a church, palace, house, prison, monastery, or school, or it may be used for public worship of the established Church, subordinate to or dependent upon the parish church, the accommodation supplied by which it in some way supplements. The concept includes both freestanding chapels and rooms or recesses serving as chapels in churches or other buildings."""@en;
  skos:exactMatch aat:300004590;
  skos:prefLabel "kapelle"@de;
  skos:prefLabel "chapel"@en;
  skos:prefLabel "chapelle"@fr;
  skos:prefLabel "kapel"@nl;
  skos:inScheme dccd:objectElementType.
dccd:a7a251b4-6b80-11e5-ab4b-e3cc6d9519b7 rdf:type skos:Concept;
  skos:exactMatch aat:300004759;
  skos:prefLabel "keller"@de;
  skos:prefLabel "cellar"@en;
  skos:prefLabel "cellier"@fr;
  skos:prefLabel "kelder"@nl;
  skos:inScheme dccd:objectElementType.
dccd:a7a25254-6b80-11e5-ab4c-3f4a22eedb62 rdf:type skos:Concept;
  skos:exactMatch aat:300312247;
  skos:prefLabel "kirche"@de;
  skos:prefLabel "church"@en;
  skos:prefLabel "église"@fr;
  skos:prefLabel "kerk"@nl;
  skos:inScheme dccd:objectElementType.
dccd:a7a252f4-6b80-11e5-ab4d-5f76b1514f4d rdf:type skos:Concept;
  skos:scopeNote """Yards which belong to churches and are used as places for burial """@en;
  skos:exactMatch aat:300008170;
  skos:prefLabel "kirchhof"@de;
  skos:prefLabel "churchyard"@en;
  skos:prefLabel "cimetière"@fr;
  skos:prefLabel "kerkhof"@nl;
  skos:inScheme dccd:objectElementType.
dccd:a7a25394-6b80-11e5-ab4e-6701c4959f11 rdf:type skos:Concept;
  skos:scopeNote """Main structural members running for and aft along the bottom of a ship or boat, to which the frame of the vessel is attached shipsterm """@en;
  skos:exactMatch aat:300263190;
  skos:altLabel "scheepskiel"@nl;
  skos:prefLabel "kiel"@de;
  skos:prefLabel "keel"@en;
  skos:prefLabel "quille"@fr;
  skos:prefLabel "kiel"@nl;
  skos:inScheme dccd:objectElementType.
dccd:a7a24a98-6b80-11e5-ab40-2bc84ad14f9a rdf:type skos:Concept;
  skos:scopeNote """Outside of the body of a ship"""@en;
  skos:broadMatch aat:300212614;
  skos:altLabel "haut"@de;
  skos:altLabel "schale"@de;
  skos:altLabel "shell"@en;
  skos:altLabel "bordage"@fr;
  skos:altLabel "bordé"@fr;
  skos:prefLabel "außenhülle"@de;
  skos:prefLabel "outer hull"@en;
  skos:prefLabel "bordé extérieur"@fr;
  skos:prefLabel "huid"@nl;
  skos:inScheme dccd:objectElementType.
dccd:a7a24b38-6b80-11e5-ab41-d355b2ffeae7 rdf:type skos:Concept;
  skos:scopeNote """Part of the shell of the hull of a boat or ship which, in conjunction with the other strakes, keeps the sea out and the vessel afloat"""@en;
  skos:broadMatch aat:300212614;
  skos:altLabel "bordage"@fr;
  skos:altLabel "bordage"@fr;
  skos:prefLabel "hautplanke"@de;
  skos:prefLabel "huidplank"@nl;
  skos:prefLabel "hull plank"@en;
  skos:prefLabel "planche de bordage"@fr;
  skos:altLabel "huidgang"@nl;
  skos:altLabel "virure de bordage"@fr;
  skos:altLabel "hull strake"@en;
  skos:altLabel "hautgang"@de;
  skos:broader dccd:27171b0a-6c53-11e5-9a23-5739630d10e1;
  skos:inScheme dccd:objectElementType.
dccd:a7a24f16-6b80-11e5-ab47-4b13c7360c8b rdf:type skos:Concept;
  skos:scopeNote """Vertical-axled rotating machine developed for use on sailing ships to apply force to ropes, cables, and hawsers. The principle is similar to that of the windlass, which has a horizontal axle."""@en;
  skos:broadMatch aat:300212614;
  skos:prefLabel "schiffswinde"@de;
  skos:prefLabel "capstan"@en;
  skos:prefLabel "cabestan"@fr;
  skos:prefLabel "kaapstander"@nl;
  skos:inScheme dccd:objectElementType.
dccd:a7a2543e-6b80-11e5-ab4f-6f0be0003e5a rdf:type skos:Concept;
  skos:scopeNote """shipsterm """@en;
  skos:broadMatch aat:300212614;
  skos:prefLabel "kielbalken"@de;
  skos:prefLabel "keel beam"@en;
  skos:prefLabel "barrot de quille"@fr;
  skos:prefLabel "kielbalk"@nl;
  skos:inScheme dccd:objectElementType.
dccd:a7a25c22-6b80-11e5-ab57-eb22fc13837a rdf:type skos:Concept;
  skos:scopeNote """Parallel beams used to support floor and ceiling loads and supported in turn by larger beams, girders, bearing walls, or other members. """@en;
  skos:closeMatch aat:300001544;
  skos:altLabel "common joist"@en;
  skos:prefLabel "kindbalken"@de;
  skos:prefLabel "joist"@en;
  skos:prefLabel "solive"@fr;
  skos:prefLabel "kinderbalk"@nl;
  skos:inScheme dccd:objectElementType.
dccd:a7a25ccc-6b80-11e5-ab58-13cee7d43029 rdf:type skos:Concept;
  skos:scopeNote """Furniture that encloses a space and is generally boxlike in structure; intended for storage or display """@en;
  skos:exactMatch aat:300039240;
  skos:altLabel "schrein"@de;
  skos:altLabel "kästchen"@de;
  skos:altLabel "kisten"@de;
  skos:altLabel "case"@en;
  skos:altLabel "closet"@en;
  skos:altLabel "cupboard"@en;
  skos:altLabel "kast"@nl;
  skos:prefLabel "schrank"@de;
  skos:prefLabel "case furniture"@en;
  skos:prefLabel "armoire"@fr;
  skos:prefLabel "kastmeubilair"@nl;
  skos:inScheme dccd:objectElementType.
dccd:a7a25d8a-6b80-11e5-ab59-ab0cee14e514 rdf:type skos:Concept;
  skos:scopeNote """Use for instruments that measure and indicate the passage of time, especially by mechanical means producing a regularly recurring action and indicating, usually by hands or changing numbers, the hours and minutes; not designed to be worn or otherwise carried about on a person. For wearable timepieces, use 'watches.'"""@en;
  skos:exactMatch aat:300041575;
  skos:prefLabel "uhr"@de;
  skos:prefLabel "clock"@en;
  skos:prefLabel "horloge"@fr;
  skos:prefLabel "klok"@nl;
  skos:inScheme dccd:objectElementType.
dccd:a7a25e34-6b80-11e5-ab5a-e75d745e341b rdf:type skos:Concept;
  skos:scopeNote """Places of religious retirement or seclusion from the world for persons under religious vows """@en;
  skos:exactMatch aat:300000641;
  skos:altLabel "convent"@en;
  skos:altLabel "couvent"@fr;
  skos:prefLabel "kloster"@de;
  skos:prefLabel "monastery"@en;
  skos:prefLabel "monastère"@fr;
  skos:prefLabel "klooster"@nl;
  skos:inScheme dccd:objectElementType.
dccd:a7a25f88-6b80-11e5-ab5c-0bf38ec1ed1d rdf:type skos:Concept;
  skos:exactMatch aat:300203596;
  skos:altLabel "schale"@de;
  skos:prefLabel "schüssel"@de;
  skos:prefLabel "bowl"@en;
  skos:prefLabel "bol"@fr;
  skos:prefLabel "kom"@nl;
  skos:inScheme dccd:objectElementType.
dccd:a7a26028-6b80-11e5-ab5d-df35d48c16ab rdf:type skos:Concept;
  skos:scopeNote """Use for watercraft engaged in commercial transport on oceans or large inland bodies of water """@en;
  skos:exactMatch aat:300232781;
  skos:altLabel "kauffahrer"@de;
  skos:altLabel "kauffahrteischiff"@de;
  skos:altLabel "trader"@en;
  skos:altLabel "trading ship"@en;
  skos:altLabel "navire marchand"@fr;
  skos:prefLabel "handelsschiff"@de;
  skos:prefLabel "merchant vessel"@en;
  skos:prefLabel "navire de commerce"@fr;
  skos:prefLabel "koopvaardijschip"@nl;
  skos:inScheme dccd:objectElementType.
dccd:a7a260d2-6b80-11e5-ab5e-47fa35ea433e rdf:type skos:Concept;
  skos:scopeNote """Use for spaces in Christian churches containing the high altar and reserved for the use of the clergy. Includes the choir when present. Use 'choirs' for the spaces in Christian churches, generally between the altar area and the nave, reserved for choristers."""@en;
  skos:exactMatch aat:300001840;
  skos:prefLabel "chor"@de;
  skos:prefLabel "chancel"@en;
  skos:prefLabel "choeur"@fr;
  skos:prefLabel "koor"@nl;
  skos:inScheme dccd:objectElementType.
dccd:a7a2617c-6b80-11e5-ab5f-1fbeea9534ad rdf:type skos:Concept;
  skos:exactMatch aat:300076128;
  skos:prefLabel "chorstuhl"@de;
  skos:prefLabel "choir stall"@en;
  skos:prefLabel "stalle"@fr;
  skos:prefLabel "koorstoel"@nl;
  skos:inScheme dccd:objectElementType.
dccd:a7a26226-6b80-11e5-ab60-7f110d55838a rdf:type skos:Concept;
  skos:scopeNote """Bottom-based merchant ships of the 13th to the 15th century, clinker-built with rounded bow and stern, fore and after castles, and very broad in the beam; occasionaly used as warships"""@en;
  skos:exactMatch aat:300232923;
  skos:altLabel "cog ship"@en;
  skos:prefLabel "kogge"@de;
  skos:prefLabel "cog"@en;
  skos:prefLabel "cogue"@fr;
  skos:prefLabel "kogge"@nl;
  skos:broader dccd:a7a1ba74-6b80-11e5-aa7a-7b1dc4c873b5;
  skos:inScheme dccd:objectElementType.
dccd:a7a262d0-6b80-11e5-ab61-bf572e76a7e4 rdf:type skos:Concept;
  skos:scopeNote """Three-dimensional structure consisting of pendant posts, struts and straining beams."""@en;
  skos:broadMatch aat:300001497;
  skos:prefLabel "hängewerk"@de;
  skos:prefLabel "hanging truss"@en;
  skos:prefLabel "supports du premier faux-entrait"@fr;
  skos:prefLabel "hangwerk"@nl;
  skos:inScheme dccd:objectElementType.
dccd:a7a26370-6b80-11e5-ab62-6beeaf6283d3 rdf:type skos:Concept;
  skos:scopeNote """Upright post forming part of two distinct types of standing trusses.  Has two rows of posts or single axis row."""@en;
  skos:exactMatch aat:300002456;
  skos:prefLabel "queenpost"@en;
  skos:prefLabel "hangstijlstifl van een staande dakstoel"@nl;
  skos:prefLabel "poinçon"@fr;
  skos:altLabel "poteau"@fr;
  skos:altLabel "jukstijl"@nl;
  skos:prefLabel "stuflstander"@de;
  skos:altLabel "stuhlsaule"@de;
  skos:altLabel "mittelsaule"@de;
  skos:inScheme dccd:objectElementType.
dccd:a7a264c4-6b80-11e5-ab64-fb2cb060f063 rdf:type skos:Concept;
  skos:scopeNote """The projecting, uppermost features of classical entablatures; use also for similar features crowning a wall, in any style; corona: Overhanging vertical members of a cornice in classical architecture, supported by bed moldings and crowned by cymatia, usually with a drip to throw rainwater clear of the building."""@en;
  skos:exactMatch aat:300001788;
  skos:altLabel "corona"@en;
  skos:prefLabel "kranzgesims"@de;
  skos:prefLabel "cornice"@en;
  skos:prefLabel "corniche"@fr;
  skos:prefLabel "kroonlijst"@nl;
  skos:inScheme dccd:objectElementType.
dccd:a7a2656e-6b80-11e5-ab65-7f24dce16cb6 rdf:type skos:Concept;
  skos:exactMatch aat:300008027;
  skos:altLabel "loch"@de;
  skos:altLabel "mulde"@de;
  skos:altLabel "vertiefung"@de;
  skos:altLabel "hole"@en;
  skos:altLabel "fosse"@fr;
  skos:prefLabel "grube"@de;
  skos:prefLabel "pit"@en;
  skos:prefLabel "trou"@fr;
  skos:prefLabel "kuil"@nl;
  skos:inScheme dccd:objectElementType.
dccd:a7a26618-6b80-11e5-ab66-ab8d9e6fc590 rdf:type skos:Concept;
  skos:scopeNote """Large casks for holding liquids, especially wine, ale, or beer """@en;
  skos:exactMatch aat:300194514;
  skos:altLabel "fass"@de;
  skos:altLabel "kübel"@de;
  skos:altLabel "tub"@en;
  skos:altLabel "tun"@en;
  skos:altLabel "vat"@en;
  skos:altLabel "cuve"@fr;
  skos:altLabel "kuip"@nl;
  skos:altLabel "vat"@nl;
  skos:prefLabel "tonne"@de;
  skos:prefLabel "barrel"@en;
  skos:prefLabel "tonneau"@fr;
  skos:prefLabel "ton"@nl;
  skos:inScheme dccd:objectElementType.
dccd:a7a266c2-6b80-11e5-ab67-0b2994282775 rdf:type skos:Concept;
  skos:scopeNote """Frames, usually of wood or metal, consisting of two side pieces called stiles which are connected by crosspieces, usually round, called rungs; used as a means of climbing up or down. """@en;
  skos:exactMatch aat:300022376;
  skos:prefLabel "leiter"@de;
  skos:prefLabel "ladder"@en;
  skos:prefLabel "échelle"@fr;
  skos:prefLabel "ladder"@nl;
  skos:inScheme dccd:objectElementType.
dccd:a7a26762-6b80-11e5-ab68-6780e4cc4d70 rdf:type skos:Concept;
  skos:exactMatch aat:300040558;
  skos:prefLabel "schublade"@de;
  skos:prefLabel "drawer"@en;
  skos:prefLabel "tiroir"@fr;
  skos:prefLabel "lade"@nl;
  skos:inScheme dccd:objectElementType.
dccd:a7a2680c-6b80-11e5-ab69-cb98b6ec69b6 rdf:type skos:Concept;
  skos:closeMatch aat:300005567;
  skos:prefLabel "landgut"@de;
  skos:prefLabel "country estate"@en;
  skos:prefLabel "domaine"@fr;
  skos:prefLabel "landgoed"@nl;
  skos:inScheme dccd:objectElementType.
dccd:a7a268ac-6b80-11e5-ab6a-8bd9b38f7f29 rdf:type skos:Concept;
  skos:scopeNote """In contemporary military contexts, use for groups of huts, tents, or other shelters set up temporarily for troops; in historical contexts use for permanent or semipermanent places of encampment; use 'military bases' for contemporary permanent installations."""@en;
  skos:exactMatch aat:300000476;
  skos:prefLabel "militärlager"@de;
  skos:prefLabel "military camp"@en;
  skos:prefLabel "camp militaire"@fr;
  skos:prefLabel "legerplaats"@nl;
  skos:inScheme dccd:objectElementType.
dccd:a7a26956-6b80-11e5-ab6b-bb114e6ff487 rdf:type skos:Concept;
  skos:scopeNote """Parapets or balustrades of a lightweight, partly open, metal or wood construction; Use for railings that are intended to be grasped by the hand in order to serve as a support; may also refer to the top members of balustrades or railings """@en;
  skos:exactMatch aat:300002018;
  skos:prefLabel "geländer"@de;
  skos:prefLabel "railing"@en;
  skos:prefLabel "rampe"@fr;
  skos:prefLabel "leuning"@nl;
  skos:inScheme dccd:objectElementType.
dccd:a7a26a00-6b80-11e5-ab6c-0b87195c7120 rdf:type skos:Concept;
  skos:exactMatch aat:300001989;
  skos:prefLabel "balustrade"@de;
  skos:prefLabel "balustrade"@en;
  skos:prefLabel "balustrade"@fr;
  skos:prefLabel "balustrade"@nl;
  skos:inScheme dccd:objectElementType.
dccd:a7a26aaa-6b80-11e5-ab6d-3fafe99830a7 rdf:type skos:Concept;
  skos:scopeNote """shipsterm """@en;
  skos:exactMatch aat:300022367;
  skos:prefLabel "winde"@de;
  skos:prefLabel "winch"@en;
  skos:prefLabel "treuil"@fr;
  skos:prefLabel "windas"@nl;
  skos:inScheme dccd:objectElementType.
dccd:a7a26b4a-6b80-11e5-ab6e-2771c25a14f4 rdf:type skos:Concept;
  skos:scopeNote """Shallow piers or rectangular columns projecting only slightly from a wall and, in classical architecture, conforming with one of the orders. Shipsterm"""@en;
  skos:exactMatch aat:300002737;
  skos:prefLabel "pilaster"@de;
  skos:prefLabel "pilaster"@en;
  skos:prefLabel "pilastre"@fr;
  skos:prefLabel "pilaster"@nl;
  skos:inScheme dccd:objectElementType.
dccd:a7a26bf4-6b80-11e5-ab6f-3f4f98fb0e84 rdf:type skos:Concept;
  skos:exactMatch aat:300042101;
  skos:prefLabel "laute"@de;
  skos:prefLabel "lute"@en;
  skos:prefLabel "luth"@fr;
  skos:prefLabel "luit"@nl;
  skos:inScheme dccd:objectElementType.
dccd:a7a26fd2-6b80-11e5-ab75-eb16ea4df421 rdf:type skos:Concept;
  skos:exactMatch aat:300003092;
  skos:altLabel "montant"@fr;
  skos:altLabel "montant"@nl;
  skos:altLabel "post"@nl;
  skos:prefLabel "pfosten"@de;
  skos:prefLabel "mullion"@en;
  skos:prefLabel "meneau"@fr;
  skos:prefLabel "vensterstijl"@nl;
  skos:inScheme dccd:objectElementType.
dccd:a7a2707c-6b80-11e5-ab76-5fcac7fc7f5e rdf:type skos:Concept;
  skos:scopeNote """Steep mounds, a main feature of certain 11th- and 12th-century castles """@en;
  skos:exactMatch aat:300175482;
  skos:prefLabel "burghügel"@de;
  skos:prefLabel "motte"@en;
  skos:prefLabel "mound"@fr;
  skos:prefLabel "motte"@nl;
  skos:inScheme dccd:objectElementType.
dccd:a7a27126-6b80-11e5-ab77-a337a411c5f4 rdf:type skos:Concept;
  skos:exactMatch aat:300005768;
  skos:prefLabel "museum"@de;
  skos:prefLabel "museum"@en;
  skos:prefLabel "musée"@fr;
  skos:prefLabel "museum"@nl;
  skos:inScheme dccd:objectElementType.
dccd:a7a271c6-6b80-11e5-ab78-2b24443b781b rdf:type skos:Concept;
  skos:scopeNote """Vertical architectural members used to define and divide spaces """@en;
  skos:exactMatch aat:300002469;
  skos:altLabel "pan de mur"@fr;
  skos:altLabel "paroi"@fr;
  skos:prefLabel "wand"@de;
  skos:prefLabel "wall"@en;
  skos:prefLabel "mur"@fr;
  skos:prefLabel "wand"@nl;
  skos:inScheme dccd:objectElementType.
dccd:a7a2557e-6b80-11e5-ab51-4b797d54ff1c rdf:type skos:Concept;
  skos:scopeNote """shipsterm """@en;
  skos:broadMatch aat:300212614;
  skos:prefLabel "aufkimmung"@de;
  skos:prefLabel "bilge"@en;
  skos:prefLabel "bouchain"@fr;
  skos:prefLabel "kim"@nl;
  skos:inScheme dccd:objectElementType.
dccd:a7a258b2-6b80-11e5-ab52-33cf588653f2 rdf:type skos:Concept;
  skos:scopeNote """shipsterm """@en;
  skos:broadMatch aat:300212614;
  skos:prefLabel "kimmstück"@de;
  skos:prefLabel "chine block"@en;
  skos:prefLabel "pièce de bouchain"@fr;
  skos:prefLabel "kimstuk"@nl;
  skos:inScheme dccd:objectElementType.
dccd:a7a25984-6b80-11e5-ab53-272c5d4e5f62 rdf:type skos:Concept;
  skos:scopeNote """shipsterm """@en;
  skos:broadMatch aat:300212614;
  skos:prefLabel "kimmstringer"@de;
  skos:prefLabel "bilge stringer"@en;
  skos:prefLabel "bordage de bouchain"@fr;
  skos:prefLabel "kimweger"@nl;
  skos:inScheme dccd:objectElementType.
dccd:a7a2641a-6b80-11e5-ab63-036147e2b404 rdf:type skos:Concept;
  skos:broadMatch aat:300212614;
  skos:altLabel "courbe"@fr;
  skos:prefLabel "krummer"@de;
  skos:prefLabel "crock"@en;
  skos:prefLabel "bois courbe"@fr;
  skos:prefLabel "krommer"@nl;
  skos:inScheme dccd:objectElementType.
dccd:a7a26c94-6b80-11e5-ab70-e341ea1c9c3b rdf:type skos:Concept;
  skos:broadMatch aat:300212614;
  skos:altLabel "banc d’étambrai, banc de mât"@fr;
  skos:altLabel "banc de mât"@fr;
  skos:prefLabel "mastducht"@de;
  skos:prefLabel "mast thwart"@en;
  skos:prefLabel "banc d’étambrai"@fr;
  skos:prefLabel "mastbank"@nl;
  skos:inScheme dccd:objectElementType.
dccd:a7a26d3e-6b80-11e5-ab71-e7724b8494c6 rdf:type skos:Concept;
  skos:broadMatch aat:300212614;
  skos:prefLabel "mastblock"@de;
  skos:prefLabel "mast step"@en;
  skos:prefLabel "carlingue de mât"@fr;
  skos:prefLabel "mastblok"@nl;
  skos:inScheme dccd:objectElementType.
dccd:a7a26f32-6b80-11e5-ab74-a36e7bc0633a rdf:type skos:Concept;
  skos:scopeNote """Use for large beams that span between the two walls or sides of a structure """@en;
  skos:broadMatch aat:300001497;
  skos:prefLabel "mutterbalken"@de;
  skos:prefLabel "binder"@en;
  skos:prefLabel "poutre maîtresse"@fr;
  skos:prefLabel "moerbalk"@nl;
  skos:inScheme dccd:objectElementType.
dccd:a7a27270-6b80-11e5-ab79-affe6c8be6a3 rdf:type skos:Concept;
  skos:scopeNote """Sound-producing apparatuses whose primary function is to play music """@en;
  skos:exactMatch aat:300041620;
  skos:prefLabel "musikinstrument"@de;
  skos:prefLabel "musical instrument"@en;
  skos:prefLabel "instrument de musique"@fr;
  skos:prefLabel "muziekinstrument"@nl;
  skos:inScheme dccd:objectElementType.
dccd:a7a27540-6b80-11e5-ab7a-6b825593ddbd rdf:type skos:Concept;
  skos:scopeNote """Designates places or areas occupied, modified, or planned to be inhabited by communities of human populations and that contain enough societal functions to be relatively self-sufficient. """@en;
  skos:exactMatch aat:300008347;
  skos:prefLabel "siedlung"@de;
  skos:prefLabel "settlement"@en;
  skos:prefLabel "établissement humain"@fr;
  skos:prefLabel "nederzetting"@nl;
  skos:inScheme dccd:objectElementType.
dccd:a7a27612-6b80-11e5-ab7b-7f0859f2568e rdf:type skos:Concept;
  skos:scopeNote """Use for chancel screens surmounted by a cross or crucifix; generally found in English church architecture;"""@en;
  skos:exactMatch aat:300265155;
  skos:altLabel "chorbühne"@de;
  skos:prefLabel "lettner"@de;
  skos:prefLabel "rood screen"@en;
  skos:prefLabel "jubé"@fr;
  skos:prefLabel "doksaal"@nl;
  skos:inScheme dccd:objectElementType.
dccd:a7a276bc-6b80-11e5-ab7c-0ba85b4da745 rdf:type skos:Concept;
  skos:scopeNote """Broad embankments or mounds of earth raised as a fortification """@en;
  skos:exactMatch aat:300002505;
  skos:prefLabel "schutzwall"@de;
  skos:prefLabel "rampart"@en;
  skos:prefLabel "rempart"@fr;
  skos:prefLabel "omwalling"@nl;
  skos:inScheme dccd:objectElementType.
dccd:a7a2795a-6b80-11e5-ab80-eba838a4233a rdf:type skos:Concept;
  skos:broadMatch aat:300001834;
  skos:altLabel "langschoor"@nl;
  skos:prefLabel "strebe"@de;
  skos:prefLabel "(long) brace"@en;
  skos:prefLabel "décharge"@fr;
  skos:prefLabel "schoor"@nl;
  skos:inScheme dccd:objectElementType.
dccd:a7a27b44-6b80-11e5-ab83-c3e6ee19986d rdf:type skos:Concept;
  skos:scopeNote """Intersections of the sloping sides of roofs."""@en;
  skos:exactMatch aat:300002352;
  skos:prefLabel "ridge"@en;
  skos:prefLabel "faîte"@fr;
  skos:prefLabel "nok"@nl;
  skos:altLabel "first"@de;
  skos:prefLabel "dachfirst"@de;
  skos:altLabel "firstlinie"@de;
  skos:inScheme dccd:objectElementType.
dccd:a7a27bee-6b80-11e5-ab84-9fa70eab82a4 rdf:type skos:Concept;
  skos:scopeNote """Non-earthfast post rising from the group up to the ridge and usually supports a ridge purlin."""@en;
  skos:broadMatch aat:300001609;
  skos:prefLabel "firstständer"@de;
  skos:prefLabel "ridge post"@en;
  skos:prefLabel "poteau de fond porteur de la faîtière"@fr;
  skos:prefLabel "nokstijl"@nl;
  skos:inScheme dccd:objectElementType.
dccd:a7a27d4c-6b80-11e5-ab86-471faf96367b rdf:type skos:Concept;
  skos:scopeNote """Cavities in the earth resulting from removal of soil and rock for purposes of building construction or archaeology."""@en;
  skos:exactMatch aat:300108265;
  skos:prefLabel "ausgrabung"@de;
  skos:prefLabel "excavation"@en;
  skos:prefLabel "excavation"@fr;
  skos:prefLabel "opgraving"@nl;
  skos:inScheme dccd:objectElementType.
dccd:a7a27f40-6b80-11e5-ab89-1347ece9c897 rdf:type skos:Concept;
  skos:scopeNote """Complex aerophones consisting of one or more rows of individual pipes which are made to sound by air under pressure directed from a wind-raising device and admitted to the pipes by means of valves operated from a keyboard or set of levers """@en;
  skos:exactMatch aat:300041686;
  skos:prefLabel "orgel"@de;
  skos:prefLabel "organ"@en;
  skos:prefLabel "orgue"@fr;
  skos:prefLabel "orgel"@nl;
  skos:inScheme dccd:objectElementType.
dccd:a7a2808a-6b80-11e5-ab8b-6bc286283761 rdf:type skos:Concept;
  skos:scopeNote """Use for official residences, frequently large and impressively appointed, of sovereigns or other high dignitaries; for other large stately dwellings but not official residences, use 'mansions.' """@en;
  skos:exactMatch aat:300005734;
  skos:prefLabel "palast"@de;
  skos:prefLabel "palace"@en;
  skos:prefLabel "palais"@fr;
  skos:prefLabel "paleis"@nl;
  skos:inScheme dccd:objectElementType.
dccd:a7a28134-6b80-11e5-ab8c-3f0457a8e4dd rdf:type skos:Concept;
  skos:scopeNote """Barriers composed of long stakes, usually with pointed tops, driven into the earth close together, sometimes connected by horizontal beams """@en;
  skos:exactMatch aat:300003717;
  skos:prefLabel "palisade"@de;
  skos:prefLabel "palisade"@en;
  skos:prefLabel "palissade"@fr;
  skos:prefLabel "palissade"@nl;
  skos:inScheme dccd:objectElementType.
dccd:a7a281de-6b80-11e5-ab8d-1b18cbbaafc5 rdf:type skos:Concept;
  skos:exactMatch aat:300212606;
  skos:prefLabel "kriegsschiff"@de;
  skos:prefLabel "warship"@en;
  skos:prefLabel "navire de querre"@fr;
  skos:prefLabel "oorlogsschip"@nl;
  skos:broader dccd:a7a1ba74-6b80-11e5-aa7a-7b1dc4c873b5;
  skos:inScheme dccd:objectElementType.
dccd:a7a28328-6b80-11e5-ab8f-bf21795005df rdf:type skos:Concept;
  skos:scopeNote """The residences provided for clergymen, usually parsons/vicars """@en;
  skos:exactMatch aat:300005650;
  skos:altLabel "presbytère"@fr;
  skos:prefLabel "pfarrhaus"@de;
  skos:prefLabel "vicarage"@en;
  skos:prefLabel "cure"@fr;
  skos:prefLabel "pastorie"@nl;
  skos:inScheme dccd:objectElementType.
dccd:a7a283d2-6b80-11e5-ab90-f712f9ff8d3d rdf:type skos:Concept;
  skos:scopeNote """shipsterm """@en;
  skos:exactMatch aat:300213080;
  skos:prefLabel "paddel"@de;
  skos:prefLabel "paddle"@en;
  skos:prefLabel "pagaie"@fr;
  skos:prefLabel "peddel"@nl;
  skos:inScheme dccd:objectElementType.
dccd:a7a28472-6b80-11e5-ab91-17072903c8e8 rdf:type skos:Concept;
  skos:exactMatch aat:300010262;
  skos:prefLabel "platte"@de;
  skos:prefLabel "plaque"@en;
  skos:prefLabel "plate"@fr;
  skos:prefLabel "plaat"@nl;
  skos:inScheme dccd:objectElementType.
dccd:a7a2851c-6b80-11e5-ab92-17a3c6e09055 rdf:type skos:Concept;
  skos:scopeNote """The overhead surfaces of interior spaces, sometimes constructed to mask building systems or structural elements """@en;
  skos:exactMatch aat:300002031;
  skos:prefLabel "decke"@de;
  skos:prefLabel "ceiling"@en;
  skos:prefLabel "plafond"@fr;
  skos:prefLabel "plafond"@nl;
  skos:inScheme dccd:objectElementType.
dccd:a7a285bc-6b80-11e5-ab93-97ea9bfe9e3c rdf:type skos:Concept;
  skos:scopeNote """Long, wide, square-sawn thick piece of wood; Thin, flat, rigid objects, of considerable length or breadth compared to thickness, most often of wood, paperboard, or composite fiber materials. shipsterm """@en;
  skos:exactMatch aat:300126969;
  skos:altLabel "board"@en;
  skos:prefLabel "brett"@de;
  skos:prefLabel "plank"@en;
  skos:prefLabel "planche"@fr;
  skos:prefLabel "plank"@nl;
  skos:inScheme dccd:objectElementType.
dccd:a7a28666-6b80-11e5-ab94-ef208231c551 rdf:type skos:Concept;
  skos:scopeNote """Passages through fences or walls separating two exterior spaces, or the structures or ornamental constructions enclosing such passages; (Portal) Use for impressive, monumental entrances, gateways, or doorways usually to buildings or courtyards, especially those emphasized by stately architectural treatment"""@en;
  skos:exactMatch aat:300069189;
  skos:prefLabel "tor"@de;
  skos:prefLabel "gateway"@en;
  skos:prefLabel "porte"@fr;
  skos:prefLabel "poort"@nl;
  skos:inScheme dccd:objectElementType.
dccd:a7a28710-6b80-11e5-ab95-57acef8170ff rdf:type skos:Concept;
  skos:scopeNote """Use for structures at, near, or over entrance gateways, usually containing a gatekeeper's dwelling. For subordinate buildings on the grounds of estates or parks used as the dwellings of employees, such as gatekeepers, but not located at entranceways, prefer 'lodges (caretakers' houses).'"""@en;
  skos:exactMatch aat:300005621;
  skos:prefLabel "torbau"@de;
  skos:prefLabel "gatehouse"@en;
  skos:prefLabel "guérite"@fr;
  skos:prefLabel "poortgebouw"@nl;
  skos:inScheme dccd:objectElementType.
dccd:a7a287ba-6b80-11e5-ab96-d3e8d3934350 rdf:type skos:Concept;
  skos:scopeNote """Use for miniature scale houses or sets of rooms designed to hold or display miniature furniture and furnishings and usually to be used in conjunction with like-sized dolls; known since the 16th century """@en;
  skos:exactMatch aat:300136025;
  skos:prefLabel "puppenhaus"@de;
  skos:prefLabel "dollhouse"@en;
  skos:prefLabel "maison de poupée"@fr;
  skos:prefLabel "poppenhuis"@nl;
  skos:inScheme dccd:objectElementType.
dccd:a7a28904-6b80-11e5-ab98-cbd964da20b9 rdf:type skos:Concept;
  skos:scopeNote """Stands for a speaker, especially the preacher of a sermon """@en;
  skos:exactMatch aat:300003790;
  skos:prefLabel "kanzel"@de;
  skos:prefLabel "pulpit"@en;
  skos:prefLabel "chaire à prêcher"@fr;
  skos:prefLabel "preekstoel"@nl;
  skos:inScheme dccd:objectElementType.
dccd:a7a28a4e-6b80-11e5-ab9a-9342a386dc36 rdf:type skos:Concept;
  skos:exactMatch aat:300024976;
  skos:altLabel "wagenrad"@de;
  skos:prefLabel "rad"@de;
  skos:prefLabel "wheel"@en;
  skos:prefLabel "roue"@fr;
  skos:prefLabel "wiel"@nl;
  skos:inScheme dccd:objectElementType.
dccd:a7a28ba2-6b80-11e5-ab9c-5f9eed2dbfb9 rdf:type skos:Concept;
  skos:scopeNote """Use for the dining halls of monasteries or other religious institutions """@en;
  skos:exactMatch aat:300004347;
  skos:prefLabel "refektorium"@de;
  skos:prefLabel "refectory"@en;
  skos:prefLabel "réfectoire"@fr;
  skos:prefLabel "refectorium"@nl;
  skos:inScheme dccd:objectElementType.
dccd:a7a28cec-6b80-11e5-ab9e-3f07ebd3a8c3 rdf:type skos:Concept;
  skos:scopeNote """Use for images, especially pictorial compositions, executed in relief """@en;
  skos:exactMatch aat:300047230;
  skos:prefLabel "relief"@de;
  skos:prefLabel "relief"@en;
  skos:prefLabel "relief"@fr;
  skos:prefLabel "reliëf"@nl;
  skos:inScheme dccd:objectElementType.
dccd:a7a28d8c-6b80-11e5-ab9f-335ee90cfd84 rdf:type skos:Concept;
  skos:scopeNote """Use for painted or sculpted panels attached at the back of a Christian altar's mensa. For the Mexican and Spanish American paintings of Christian saints and other holy figures from Roman Catholicism, use 'retablos.' """@en;
  skos:exactMatch aat:300075940;
  skos:prefLabel "altarbild"@de;
  skos:prefLabel "altar piece"@en;
  skos:prefLabel "retable"@fr;
  skos:prefLabel "retabel"@nl;
  skos:inScheme dccd:objectElementType.
dccd:a7a28e36-6b80-11e5-aba0-839ba2ddbd34 rdf:type skos:Concept;
  skos:exactMatch aat:300079019;
  skos:prefLabel "deckwerk"@de;
  skos:prefLabel "revetment"@en;
  skos:prefLabel "revêtement"@fr;
  skos:prefLabel "dijkbeslag"@nl;
  skos:inScheme dccd:objectElementType.
dccd:a7a28f76-6b80-11e5-aba2-4bd79c1a7610 rdf:type skos:Concept;
  skos:scopeNote """Use for long slender shafts, usually wood, shaped to a round handle or grip at one end and flat-tipped blade at the other; for rowing. For similar but shorter devices with round-tipped blades for propelling small boats, use 'paddles (watercraft equipment).'
shipsterm"""@en;
  skos:exactMatch aat:300213077;
  skos:altLabel "riemen"@de;
  skos:altLabel "aviron"@fr;
  skos:altLabel "riem"@nl;
  skos:altLabel "roeiriem"@nl;
  skos:prefLabel "ruder"@de;
  skos:prefLabel "oar"@en;
  skos:prefLabel "rame"@fr;
  skos:prefLabel "roeispaan"@nl;
  skos:inScheme dccd:objectElementType.
dccd:a7a29020-6b80-11e5-aba3-db1826e02d86 rdf:type skos:Concept;
  skos:scopeNote """shipsterm """@en;
  skos:exactMatch aat:300212841;
  skos:prefLabel "ruder"@de;
  skos:prefLabel "rudder"@en;
  skos:prefLabel "gouvernail"@fr;
  skos:prefLabel "roer"@nl;
  skos:inScheme dccd:objectElementType.
dccd:a7a27df6-6b80-11e5-ab87-cb7ac5c04904 rdf:type skos:Concept;
  skos:broadMatch aat:300212614;
  skos:prefLabel "auflänger"@de;
  skos:prefLabel "futtock"@en;
  skos:prefLabel "allonge"@fr;
  skos:prefLabel "oplanger"@nl;
  skos:inScheme dccd:objectElementType.
dccd:a7a2885a-6b80-11e5-ab97-f3d99f749f6b rdf:type skos:Concept;
  skos:broadMatch aat:300212614;
  skos:prefLabel "bretterverschalung"@de;
  skos:prefLabel "boarding"@en;
  skos:prefLabel "bardage"@fr;
  skos:prefLabel "potdekseling"@nl;
  skos:inScheme dccd:objectElementType.
dccd:a7a289a4-6b80-11e5-ab99-eb953b10d27e rdf:type skos:Concept;
  skos:scopeNote """Piece of wood attached transversely to a ship's mast to support and guide the sail."""@en;
  skos:broadMatch aat:300212614;
  skos:prefLabel "rah"@de;
  skos:prefLabel "yard"@en;
  skos:prefLabel "vergue"@fr;
  skos:prefLabel "ra"@nl;
  skos:inScheme dccd:objectElementType.
dccd:a7a28af8-6b80-11e5-ab9b-b7f9a9a18ba5 rdf:type skos:Concept;
  skos:broadMatch aat:300212614;
  skos:prefLabel "rahenklampe"@de;
  skos:prefLabel "yard cleat"@en;
  skos:prefLabel "taquet vergues"@fr;
  skos:prefLabel "raklamp"@nl;
  skos:inScheme dccd:objectElementType.
dccd:a7a27766-6b80-11e5-ab7d-f7977bee1c64 rdf:type skos:Concept;
  skos:scopeNote """Space for carrying cargo in a ship"""@en;
  skos:broadMatch aat:300212614;
  skos:altLabel "frachtraum"@de;
  skos:altLabel "laderaum"@de;
  skos:prefLabel "schiffsraum"@de;
  skos:prefLabel "hold"@en;
  skos:prefLabel "cale"@fr;
  skos:prefLabel "scheepsruim"@nl;
  skos:inScheme dccd:objectElementType.
dccd:a7a290ca-6b80-11e5-aba4-9b5bfadc261a rdf:type skos:Concept;
  skos:scopeNote """Designates Roman villas serving agricultural purposes """@en;
  skos:exactMatch aat:300005518;
  skos:prefLabel "Romische villa (rustica)"@de;
  skos:prefLabel "Roman villa (rustica)"@en;
  skos:prefLabel "villa Romaine (rustica)"@fr;
  skos:prefLabel "romeinse villa (rustica)"@nl;
  skos:inScheme dccd:objectElementType.
dccd:a7a2939a-6b80-11e5-aba5-67a9c77e0515 rdf:type skos:Concept;
  skos:scopeNote """shipsterm """@en;
  skos:exactMatch aat:300213040;
  skos:prefLabel "schiffsrumpf"@de;
  skos:prefLabel "hull"@en;
  skos:prefLabel "coque"@fr;
  skos:prefLabel "scheepsromp"@nl;
  skos:inScheme dccd:objectElementType.
dccd:a7a29462-6b80-11e5-aba6-479824864dcb rdf:type skos:Concept;
  skos:scopeNote """shipsterm """@en;
  skos:exactMatch aat:300012784;
  skos:prefLabel "rundholz"@de;
  skos:prefLabel "log"@en;
  skos:prefLabel "grume"@fr;
  skos:prefLabel "rondhout"@nl;
  skos:inScheme dccd:objectElementType.
dccd:a7a2950c-6b80-11e5-aba7-6305061c8f37 rdf:type skos:Concept;
  skos:exactMatch aat:300042973;
  skos:altLabel "schüssel"@de;
  skos:altLabel "coupe"@fr;
  skos:prefLabel "schale"@de;
  skos:prefLabel "dish"@en;
  skos:prefLabel "plat"@fr;
  skos:prefLabel "schaal"@nl;
  skos:inScheme dccd:objectElementType.
dccd:a7a295b6-6b80-11e5-aba8-af39f5fa29c5 rdf:type skos:Concept;
  skos:scopeNote """The structures inclined toward the water on which a ship may be built or lowered into the water; may also be used for the guides that support the ship's hull """@en;
  skos:exactMatch aat:300006433;
  skos:prefLabel "schiffwerft"@de;
  skos:prefLabel "slipway"@en;
  skos:prefLabel "cale de carénage"@fr;
  skos:prefLabel "scheepshelling"@nl;
  skos:inScheme dccd:objectElementType.
dccd:a7a2970a-6b80-11e5-abaa-3755b50cf3ef rdf:type skos:Concept;
  skos:scopeNote """Places or enclosures where boats or ships are built or repaired """@en;
  skos:exactMatch aat:300000403;
  skos:prefLabel "schiffswerft"@de;
  skos:prefLabel "shipyard"@en;
  skos:prefLabel "chantier naval"@fr;
  skos:prefLabel "scheepswerf"@nl;
  skos:inScheme dccd:objectElementType.
dccd:a7a297aa-6b80-11e5-abab-ef549e0d00c9 rdf:type skos:Concept;
  skos:scopeNote """Wood in the form of broad, thin, flat or sometimes curved pieces as, for example, in polyptychs, doors, and plywood construction"""@en;
  skos:exactMatch aat:300014657;
  skos:prefLabel "täfelung"@de;
  skos:prefLabel "panel"@en;
  skos:prefLabel "panneau"@fr;
  skos:prefLabel "paneel"@nl;
  skos:inScheme dccd:objectElementType.
dccd:a7a29854-6b80-11e5-abac-a3ffe44283cb rdf:type skos:Concept;
  skos:scopeNote """Use both for the parts of buildings that project outward from the rest, especially common as corner, central, or terminal features in French architecture, and for the detached or semidetached units into which a building (as a hospital) is sometimes divided"""@en;
  skos:exactMatch aat:300002660;
  skos:prefLabel "pavillon"@de;
  skos:prefLabel "pavillion"@en;
  skos:prefLabel "pavillon"@fr;
  skos:prefLabel "paviljoen"@nl;
  skos:inScheme dccd:objectElementType.
dccd:a7a298fe-6b80-11e5-abad-b3623830f445 rdf:type skos:Concept;
  skos:scopeNote """Arched rppf truss made of two or more overlapping layers of curved boards or planks.  The French Philivert de l'Orme can be considered to be its inventor."""@en;
  skos:broadMatch aat:300002098;
  skos:prefLabel "bohlenbinder"@de;
  skos:prefLabel "Philibert Delorme roof"@en;
  skos:prefLabel "charpente à la Philibert-Delorme"@fr;
  skos:prefLabel "philibertspant"@nl;
  skos:inScheme dccd:objectElementType.
dccd:a7a299a8-6b80-11e5-abae-0bbe844336cd rdf:type skos:Concept;
  skos:scopeNote """Flat surfaces, blocks, or floors, generally raised above the adjoining floor."""@en;
  skos:exactMatch aat:300132129;
  skos:prefLabel "plattform"@de;
  skos:prefLabel "platform"@en;
  skos:prefLabel "estrade"@fr;
  skos:prefLabel "platform"@nl;
  skos:inScheme dccd:objectElementType.
dccd:a7a29a52-6b80-11e5-abaf-937d30e962ce rdf:type skos:Concept;
  skos:scopeNote """Open structure with a movable roof for storing loose hay on a farm"""@en;
  skos:broadMatch aat:300004895;
  skos:prefLabel "rutenberg"@de;
  skos:prefLabel "hay barrack"@en;
  skos:prefLabel "hooiberg (bâtiment agricole des Pays-Bas utilisé pour le stockage du grain)"@fr;
  skos:prefLabel "hooiberg"@nl;
  skos:inScheme dccd:objectElementType.
dccd:a7a29af2-6b80-11e5-abb0-bb92e9e3115e rdf:type skos:Concept;
  skos:scopeNote """Flat-bottomed boat with a square-cut bow, designed for use in small rivers or other shallow water."""@en;
  skos:broadMatch aat:300232951;
  skos:prefLabel "pünte"@de;
  skos:prefLabel "punt"@en;
  skos:prefLabel "plate"@fr;
  skos:prefLabel "punter"@nl;
  skos:inScheme dccd:objectElementType.
dccd:a7a29c5a-6b80-11e5-abb2-4ff0ed7338ae rdf:type skos:Concept;
  skos:exactMatch aat:300036869;
  skos:altLabel "buckler"@en;
  skos:prefLabel "schild"@de;
  skos:prefLabel "shield"@en;
  skos:prefLabel "bouclier"@fr;
  skos:prefLabel "schild"@nl;
  skos:inScheme dccd:objectElementType.
dccd:a7a29d04-6b80-11e5-abb3-ab8e57f3d3bb rdf:type skos:Concept;
  skos:scopeNote """Use for unique works in which images are formed primarily by the direct application of pigments suspended in oil, water, egg yolk, molten wax, or other liquid, arranged in masses of color, onto a generally two-dimensional surface """@en;
  skos:exactMatch aat:300033618;
  skos:prefLabel "gemälde"@de;
  skos:prefLabel "painting"@en;
  skos:prefLabel "peinture"@fr;
  skos:prefLabel "schilderij"@nl;
  skos:inScheme dccd:objectElementType.
dccd:a7a29dae-6b80-11e5-abb4-174609336039 rdf:type skos:Concept;
  skos:scopeNote """Individual buildings or groups of buildings designed or used as places of instruction """@en;
  skos:exactMatch aat:300006495;
  skos:altLabel "school building"@en;
  skos:altLabel "école"@fr;
  skos:prefLabel "schulgebäude"@de;
  skos:prefLabel "schoolgebouw"@nl;
  skos:prefLabel "school"@en;
  skos:prefLabel "bâtiment scolaire"@fr;
  skos:inScheme dccd:objectElementType.
dccd:a7a29e58-6b80-11e5-abb5-5feae86e5bc9 rdf:type skos:Concept;
  skos:scopeNote """Agricultural buildings with large, usually sliding doors, prominent roofs, and predominantly open spaces on the interior, primarily used as storage buildings for hay, grains, and farm equipment and shelters for livestock; does not include those structures, often termed barns, used for the processing of food and other agricultural produce, such as hop barns and tobacco barns"""@en;
  skos:exactMatch aat:300004900;
  skos:altLabel "stadel"@de;
  skos:prefLabel "scheune"@de;
  skos:prefLabel "barn"@en;
  skos:prefLabel "grange"@fr;
  skos:prefLabel "schuur"@nl;
  skos:inScheme dccd:objectElementType.
dccd:a7a2a056-6b80-11e5-abb8-73d4c2a47abf rdf:type skos:Concept;
  skos:scopeNote """Artificial passages for water, fitted with a valve or gate for stopping or regulating the flow """@en;
  skos:exactMatch aat:300006082;
  skos:altLabel "lock"@en;
  skos:prefLabel "schleuse"@de;
  skos:prefLabel "sluice"@en;
  skos:prefLabel "écluse"@fr;
  skos:prefLabel "sluis"@nl;
  skos:inScheme dccd:objectElementType.
dccd:a7a2a0f6-6b80-11e5-abb9-4f73d1cc241c rdf:type skos:Concept;
  skos:exactMatch aat:300024300;
  skos:prefLabel "schaufel"@de;
  skos:prefLabel "shovel"@en;
  skos:prefLabel "pelle"@fr;
  skos:prefLabel "schop"@nl;
  skos:inScheme dccd:objectElementType.
dccd:a7a2a24a-6b80-11e5-abbb-c37499110f0f rdf:type skos:Concept;
  skos:exactMatch aat:300211037;
  skos:prefLabel "spielzeug"@de;
  skos:prefLabel "jouet"@fr;
  skos:prefLabel "speelgoed"@nl;
  skos:prefLabel "toy"@en;
  skos:inScheme dccd:objectElementType.
dccd:a7a2a2ea-6b80-11e5-abbc-b33c0bfe4663 rdf:type skos:Concept;
  skos:scopeNote """Stairs whose tapered treads wind around, and engage in, a solid, central newel; Staircases that are circular in plan, consisting entirely of winders or wedge-shaped steps """@en;
  skos:exactMatch aat:300003243;
  skos:altLabel "newel-post stair"@en;
  skos:altLabel "solid newel stair"@en;
  skos:altLabel "escalier à noyeau"@fr;
  skos:prefLabel "spindeltreppe"@de;
  skos:prefLabel "spiral staircase"@en;
  skos:prefLabel "escalier à vis"@fr;
  skos:prefLabel "spiltrap"@nl;
  skos:inScheme dccd:objectElementType.
dccd:a7a2a43e-6b80-11e5-abbe-33cf5627f9a6 rdf:type skos:Concept;
  skos:scopeNote """Distinctions among villages, towns, and cities are relative and vary according to their individual regional contexts. Generally, cities designate large or important communities with population, status, and internal complexity greater than most towns in the region."""@en;
  skos:exactMatch aat:300008375;
  skos:altLabel "city"@en;
  skos:prefLabel "stadt"@de;
  skos:prefLabel "town"@en;
  skos:prefLabel "ville"@fr;
  skos:prefLabel "stad"@nl;
  skos:inScheme dccd:objectElementType.
dccd:a7a2a4e8-6b80-11e5-abbf-3fad96516361 rdf:type skos:Concept;
  skos:scopeNote """Use for the principal public administration buildings of towns and villages housing offices for transaction of government business and places for public assembly """@en;
  skos:exactMatch aat:300006063;
  skos:altLabel "stadhaus"@de;
  skos:altLabel "city hall"@en;
  skos:prefLabel "rathaus"@de;
  skos:prefLabel "town hall"@en;
  skos:prefLabel "hötel de ville"@fr;
  skos:prefLabel "stadhuis"@nl;
  skos:inScheme dccd:objectElementType.
dccd:a7a2a592-6b80-11e5-abc0-2b73c7d752c7 rdf:type skos:Concept;
  skos:scopeNote """Fortification walls of cities """@en;
  skos:exactMatch aat:300005072;
  skos:prefLabel "stadtmauer"@de;
  skos:prefLabel "city wall"@en;
  skos:prefLabel "enceinte de ville"@fr;
  skos:prefLabel "stadsmuur"@nl;
  skos:inScheme dccd:objectElementType.
dccd:a7a2a664-6b80-11e5-abc1-8737c248c661 rdf:type skos:Concept;
  skos:scopeNote """Buildings or portions of buildings for the housing and feeding of horses, cattle, and other such domestic animals, and often also for storing riding equipment and vehicles, and which occasionally have living quarters for associated personnel. For barnlike structures used primarily for housing farmstock and feed, use, for example, 'horse barns' or 'cattle barns.'"""@en;
  skos:exactMatch aat:300005015;
  skos:prefLabel "stalle"@de;
  skos:prefLabel "stable"@en;
  skos:prefLabel "écurie"@fr;
  skos:prefLabel "stal"@nl;
  skos:inScheme dccd:objectElementType.
dccd:a7a2a70e-6b80-11e5-abc2-3fd4bc6d6f38 rdf:type skos:Concept;
  skos:exactMatch aat:300006155;
  skos:prefLabel "steg"@de;
  skos:prefLabel "jetty"@en;
  skos:prefLabel "appontement"@fr;
  skos:prefLabel "steiger"@nl;
  skos:inScheme dccd:objectElementType.
dccd:a7a2a7ae-6b80-11e5-abc3-17e8cf913e19 rdf:type skos:Concept;
  skos:scopeNote """Pierlike masonry elements built to strengthen or support walls or resist the lateral thrust of vaults """@en;
  skos:exactMatch aat:300000891;
  skos:prefLabel "mauerstrebe"@de;
  skos:prefLabel "buttress"@en;
  skos:prefLabel "contrefort"@fr;
  skos:prefLabel "steunbeer"@nl;
  skos:inScheme dccd:objectElementType.
dccd:a7a2aab0-6b80-11e5-abc7-53d5d4ab51f8 rdf:type skos:Concept;
  skos:scopeNote """Seats for one person with a back or a back and arms. Distinct from 'stools' which have no back. """@en;
  skos:exactMatch aat:300037772;
  skos:prefLabel "stuhl"@de;
  skos:prefLabel "chair"@en;
  skos:prefLabel "chaise"@fr;
  skos:prefLabel "stoel"@nl;
  skos:inScheme dccd:objectElementType.
dccd:a7a2abc8-6b80-11e5-abc8-a3f29716528e rdf:type skos:Concept;
  skos:scopeNote """Use for openings or recesses in chimneys or walls in which fires may be built, as for heating or cooking; may also refer to low fireproof structures erected outdoors for cooking over open flames """@en;
  skos:exactMatch aat:300052267;
  skos:altLabel "herd"@de;
  skos:altLabel "hearth"@en;
  skos:prefLabel "feuerstelle"@de;
  skos:prefLabel "fireplace"@en;
  skos:prefLabel "foyer"@fr;
  skos:prefLabel "stookplaats"@nl;
  skos:inScheme dccd:objectElementType.
dccd:a7a2ae02-6b80-11e5-abcb-376f41674327 rdf:type skos:Concept;
  skos:exactMatch aat:300007590;
  skos:prefLabel "synagoge"@de;
  skos:prefLabel "synagogue"@en;
  skos:prefLabel "synagogue"@fr;
  skos:prefLabel "synagoge"@nl;
  skos:inScheme dccd:objectElementType.
dccd:a7a2a1a0-6b80-11e5-abba-132b7af2a434 rdf:type skos:Concept;
  skos:broadMatch aat:300212614;
  skos:prefLabel "spant"@de;
  skos:prefLabel "frame"@en;
  skos:prefLabel "couple"@fr;
  skos:prefLabel "spant"@nl;
  skos:inScheme dccd:objectElementType.
dccd:a7a2a394-6b80-11e5-abbd-8b26b982493b rdf:type skos:Concept;
  skos:scopeNote """A particular type of spar that supports the sail"""@en;
  skos:broadMatch aat:300212614;
  skos:prefLabel "spriet"@de;
  skos:prefLabel "sprit"@en;
  skos:prefLabel "livarde"@fr;
  skos:prefLabel "spriet"@nl;
  skos:inScheme dccd:objectElementType.
dccd:a7a2a9ac-6b80-11e5-abc6-873528dfe3ec rdf:type skos:Concept;
  skos:broadMatch aat:300212614;
  skos:prefLabel "bugholz"@de;
  skos:prefLabel "prow block"@en;
  skos:prefLabel "épaulure"@fr;
  skos:prefLabel "stevenplaat"@nl;
  skos:inScheme dccd:objectElementType.
dccd:a7a2acb8-6b80-11e5-abc9-4734b7b45d4c rdf:type skos:Concept;
  skos:scopeNote """Equipment for steering a watercraft"""@en;
  skos:broadMatch aat:300212614;
  skos:prefLabel "ruderanlage"@de;
  skos:prefLabel "steering gear"@en;
  skos:prefLabel "appareillage à gouverner"@fr;
  skos:prefLabel "stuurinrichting"@nl;
  skos:inScheme dccd:objectElementType.
dccd:a7a2aeac-6b80-11e5-abcc-9f4a262ef628 rdf:type skos:Concept;
  skos:scopeNote """Articles of furniture consisting of a flat, slablike top supported on one or more legs or supports """@en;
  skos:exactMatch aat:300039548;
  skos:prefLabel "tisch"@de;
  skos:prefLabel "table"@en;
  skos:prefLabel "table"@fr;
  skos:prefLabel "tafel"@nl;
  skos:inScheme dccd:objectElementType.
dccd:a7a2b1b8-6b80-11e5-abcd-6bbbe3957081 rdf:type skos:Concept;
  skos:scopeNote """Refers to places devoted to the worship of a deity or deities. In the strictest sense, it refers to the dwelling place of a deity, and thus often houses a cult image. In modern usage a temple is generally a structure, but it was originally derived from the Latin 'templum' and historically has referred to an uncovered place affording a view of the surrounding region. For Christian or Islamic religious buildings the terms 'churches' or 'mosques' are generally used, but an exception is that 'temples' is used for Protestant, as opposed to Roman Catholic, places of worship in France and some French-speaking regions"""@en;
  skos:exactMatch aat:300007595;
  skos:prefLabel "tempel"@de;
  skos:prefLabel "temple"@en;
  skos:prefLabel "temple"@fr;
  skos:prefLabel "tempel"@nl;
  skos:inScheme dccd:objectElementType.
dccd:a7a2b28a-6b80-11e5-abce-63fa6a297629 rdf:type skos:Concept;
  skos:scopeNote """Roofs which rise to a peak or ridge by inclined planes on all, usually four, sides, therefore requiring hip rafters."""@en;
  skos:exactMatch aat:300002147;
  skos:prefLabel "walmdach"@de;
  skos:prefLabel "toit à croupes"@fr;
  skos:prefLabel "schilddak"@nl;
  skos:prefLabel "hip roof"@en;
  skos:altLabel "hipped roof"@en;
  skos:altLabel "walmdak"@nl;
  skos:altLabel "wolfdak"@nl;
  skos:inScheme dccd:objectElementType.
dccd:a7a2b334-6b80-11e5-abcf-1fad00f6e162 rdf:type skos:Concept;
  skos:broadMatch aat:300024617;
  skos:prefLabel "schaufelrad"@de;
  skos:prefLabel "paddle wheel"@en;
  skos:prefLabel "roue à aubes"@fr;
  skos:prefLabel "schoepenrad"@nl;
  skos:inScheme dccd:objectElementType.
dccd:a7a2b5dc-6b80-11e5-abd3-e3bae058fc38 rdf:type skos:Concept;
  skos:scopeNote """Roof structure whose load-bearing rafters are the most important elements.  Their side pressure can be absorbed in different ways."""@en;
  skos:broadMatch aat:300002098;
  skos:prefLabel "sparrendach"@de;
  skos:prefLabel "common rafter roof"@en;
  skos:prefLabel "charpente à chevrons"@fr;
  skos:prefLabel "sporenkap"@nl;
  skos:inScheme dccd:objectElementType.
dccd:a7a2b686-6b80-11e5-abd4-e3a107f963ff rdf:type skos:Concept;
  skos:scopeNote """Mill with a tower supported by struts"""@en;
  skos:broadMatch aat:300006273;
  skos:prefLabel "galerieholländer"@de;
  skos:prefLabel "tower mill"@en;
  skos:prefLabel "moulin à galerie"@fr;
  skos:prefLabel "stellingmolen"@nl;
  skos:inScheme dccd:objectElementType.
dccd:a7a2b730-6b80-11e5-abd5-230ca0274fb1 rdf:type skos:Concept;
  skos:scopeNote """Artificial passages of wood or masonry, a dam or embankment, used for impounding the water of river, stream, or canal, and fitted with a valve or gate for stopping or regulating the flow."""@en;
  skos:exactMatch aat:300006082;
  skos:altLabel "outlet sluice"@en;
  skos:prefLabel "siel"@de;
  skos:prefLabel "drainage sluice"@en;
  skos:prefLabel "spuisluis"@nl;
  skos:prefLabel "écluse"@fr;
  skos:inScheme dccd:objectElementType.
dccd:a7a2b884-6b80-11e5-abd7-5349e90beb55 rdf:type skos:Concept;
  skos:scopeNote """Short vertical member in a common rafter roof, rarely in trasverse frames of a purlin roof."""@en;
  skos:broadMatch aat:300002450;
  skos:prefLabel "sparrenknecht"@de;
  skos:prefLabel "ashlar piece"@en;
  skos:prefLabel "potelet"@fr;
  skos:prefLabel "standzoon"@nl;
  skos:altLabel "ashlar post"@en;
  skos:altLabel "voetschoor"@nl;
  skos:inScheme dccd:objectElementType.
dccd:a7a2ba78-6b80-11e5-abda-7f85f79c435a rdf:type skos:Concept;
  skos:scopeNote """Wheels used as the primary means of maneuvering vehicles."""@en;
  skos:exactMatch aat:300212892;
  skos:prefLabel "steuerrad"@de;
  skos:prefLabel "steering wheel"@en;
  skos:prefLabel "roue de gouvernail"@fr;
  skos:prefLabel "stuurwiel"@nl;
  skos:inScheme dccd:objectElementType.
dccd:a7a2bb22-6b80-11e5-abdb-57403151de1c rdf:type skos:Concept;
  skos:scopeNote """Leg of a table"""@en;
  skos:broadMatch aat:300039548;
  skos:prefLabel "tischbein"@de;
  skos:prefLabel "table leg"@en;
  skos:prefLabel "pied de table"@fr;
  skos:prefLabel "tafelpoot"@nl;
  skos:inScheme dccd:objectElementType.
dccd:a7a2bbd6-6b80-11e5-abdc-9b09981608e9 rdf:type skos:Concept;
  skos:scopeNote """Use for tall structures that are at least roughly pyramidal, polygonal, or conical and that rise from towers or roofs """@en;
  skos:exactMatch aat:300003615;
  skos:closeMatch aat:300004847;
  skos:prefLabel "turm"@de;
  skos:prefLabel "tower"@en;
  skos:prefLabel "tour"@fr;
  skos:prefLabel "toren"@nl;
  skos:inScheme dccd:objectElementType.
dccd:a7a2bc80-6b80-11e5-abdd-cb5d31bf2950 rdf:type skos:Concept;
  skos:exactMatch aat:300002360;
  skos:prefLabel "turmspitze"@de;
  skos:prefLabel "spire"@en;
  skos:prefLabel "flèche"@fr;
  skos:prefLabel "torenspits"@nl;
  skos:inScheme dccd:objectElementType.
dccd:a7a2bd2a-6b80-11e5-abde-dbc036c4f7fc rdf:type skos:Concept;
  skos:exactMatch aat:300003228;
  skos:altLabel "staircase"@en;
  skos:prefLabel "treppe"@de;
  skos:prefLabel "stairs"@en;
  skos:prefLabel "escaliers"@fr;
  skos:prefLabel "trap"@nl;
  skos:inScheme dccd:objectElementType.
dccd:a7a2bdd4-6b80-11e5-abdf-4b8727f4114f rdf:type skos:Concept;
  skos:scopeNote """Stair units that consist of one tread and one riser, or any similar element providing a horizontal surface on which to support the foot of a person descending or ascending; The horizontal parts of steps"""@en;
  skos:exactMatch aat:300003312;
  skos:altLabel "giron"@fr;
  skos:altLabel "stair"@en;
  skos:altLabel "tread"@en;
  skos:prefLabel "treppenstufe"@de;
  skos:prefLabel "step"@en;
  skos:prefLabel "marche d'escalier"@fr;
  skos:prefLabel "traptrede"@nl;
  skos:inScheme dccd:objectElementType.
dccd:a7a2be74-6b80-11e5-abe0-7793fcbf4177 rdf:type skos:Concept;
  skos:exactMatch aat:300178749;
  skos:prefLabel "boat"@en;
  skos:prefLabel "boot"@nl;
  skos:prefLabel "bateau"@fr;
  skos:prefLabel "boot"@de;
  skos:inScheme dccd:objectElementType.
dccd:a7a2bf1e-6b80-11e5-abe1-ef397b44811b rdf:type skos:Concept;
  skos:scopeNote """Stringed instrument of the violin family.  Tuned a 5th lower than a true violin"""@en;
  skos:exactMatch aat:300042225;
  skos:prefLabel "viola"@en;
  skos:prefLabel "altviool"@nl;
  skos:prefLabel "viola"@de;
  skos:prefLabel "alto"@fr;
  skos:inScheme dccd:objectElementType.
dccd:a7a2bfbe-6b80-11e5-abe2-cbd88e5cbc94 rdf:type skos:Concept;
  skos:scopeNote """Use for watercraft generally larger and more seaworthy than boats; usually propelled by sails or engines"""@en;
  skos:exactMatch aat:300082981;
  skos:prefLabel "schiff"@de;
  skos:prefLabel "ship"@en;
  skos:prefLabel "bateau"@fr;
  skos:prefLabel "schip"@nl;
  skos:broader dccd:a7a1ba74-6b80-11e5-aa7a-7b1dc4c873b5;
  skos:inScheme dccd:objectElementType.
dccd:a7a2c068-6b80-11e5-abe3-173c576ad20e rdf:type skos:Concept;
  skos:scopeNote """Refers broadly to devices or contrivances by which people, animals, or objects are conveyed or carried."""@en;
  skos:exactMatch aat:300219258;
  skos:prefLabel "vehicle"@en;
  skos:prefLabel "véhicule"@fr;
  skos:prefLabel "fahrzeug"@de;
  skos:prefLabel "voertuig"@nl;
  skos:inScheme dccd:objectElementType.
dccd:a7a2c112-6b80-11e5-abe4-e3f2fbd024f6 rdf:type skos:Concept;
  skos:scopeNote """The surfaces of rooms or spaces on which one walks"""@en;
  skos:exactMatch aat:300002060;
  skos:prefLabel "floor"@en;
  skos:prefLabel "vloer"@nl;
  skos:prefLabel "sol"@fr;
  skos:prefLabel "fußboden"@de;
  skos:inScheme dccd:objectElementType.
dccd:a7a2c25c-6b80-11e5-abe6-cf08b09f60f2 rdf:type skos:Concept;
  skos:scopeNote """Designates independent and canonically erected monasteries, ruled by an abbot if occupied by monks and by an abbess if occupied by nuns """@en;
  skos:exactMatch aat:300000642;
  skos:prefLabel "abtei"@de;
  skos:prefLabel "abbey"@en;
  skos:prefLabel "abbaye"@fr;
  skos:prefLabel "abdij"@nl;
  skos:inScheme dccd:objectElementType.
dccd:a7a2c306-6b80-11e5-abe7-7fea5db06107 rdf:type skos:Concept;
  skos:scopeNote """Use for watercraft designed primarily to transport cargo """@en;
  skos:exactMatch aat:300212694;
  skos:altLabel "freighter"@en;
  skos:prefLabel "vrachtschip"@nl;
  skos:altLabel "frachtschiff"@de;
  skos:altLabel "lastschiff"@de;
  skos:prefLabel "cargo vessel"@en;
  skos:prefLabel "frachter"@de;
  skos:prefLabel "cargo"@fr;
  skos:inScheme dccd:objectElementType.
dccd:a7a2c4fa-6b80-11e5-abea-0b5625eff428 rdf:type skos:Concept;
  skos:scopeNote """Passages or rooms just inside the entrance of a residence, but sometimes with a vestibule between it and the outdoors. Prefer 'lobbies' for such spaces in larger public buildings."""@en;
  skos:exactMatch aat:300004263;
  skos:prefLabel "entrance hall"@en;
  skos:prefLabel "flur"@de;
  skos:prefLabel "hall d'entrée"@fr;
  skos:prefLabel "entreehal"@nl;
  skos:inScheme dccd:objectElementType.
dccd:a7a2c5a4-6b80-11e5-abeb-5f2542d3673a rdf:type skos:Concept;
  skos:scopeNote """Rooms or closets in which food, groceries, and other provisions, or silverware, dishes, and other items are kept."""@en;
  skos:exactMatch aat:300004499;
  skos:prefLabel "provisiekamer"@nl;
  skos:altLabel "voorraadkamer"@nl;
  skos:prefLabel "pantry"@en;
  skos:prefLabel "garde-manger"@fr;
  skos:prefLabel "speisekammer"@de;
  skos:inScheme dccd:objectElementType.
dccd:a7a2c644-6b80-11e5-abec-33b88023131e rdf:type skos:Concept;
  skos:scopeNote """A pair of small oars used by a single rower"""@en;
  skos:broadMatch aat:300213077;
  skos:prefLabel "scull"@en;
  skos:prefLabel "skull"@de;
  skos:prefLabel "godille"@fr;
  skos:prefLabel "wrikriem"@nl;
  skos:inScheme dccd:objectElementType.
dccd:a7a2c6ee-6b80-11e5-abed-bb1ab0b1dad9 rdf:type skos:Concept;
  skos:scopeNote """General term referring to all long outdoor passages used by and generally created by humans, intended to allow people to pass between different places, usually one wide enough to admit of the passage of wheeled vehicles, horses, or travellers on foot."""@en;
  skos:exactMatch aat:300008217;
  skos:altLabel "way"@en;
  skos:altLabel "chemin"@fr;
  skos:prefLabel "road"@en;
  skos:prefLabel "weg"@nl;
  skos:prefLabel "route"@fr;
  skos:prefLabel "straße"@de;
  skos:altLabel "weg"@de;
  skos:inScheme dccd:objectElementType.
dccd:a7a2c798-6b80-11e5-abee-07164408d7de rdf:type skos:Concept;
  skos:scopeNote """Rigid sheaths made of wood, metal, or leather, used to enclose and carry edged weapons or tools, or hand weapons such as carbines and rifles."""@en;
  skos:exactMatch aat:300037139;
  skos:prefLabel "scabbard"@en;
  skos:prefLabel "fourreau"@fr;
  skos:prefLabel "schede"@nl;
  skos:prefLabel "schwertscheide"@de;
  skos:altLabel "sheath"@en;
  skos:inScheme dccd:objectElementType.
dccd:a7a2c842-6b80-11e5-abef-5f1fbac074f8 rdf:type skos:Concept;
  skos:scopeNote """Use generally for rooms large in proportion to rooms for domestic functions, circulation, or storage; use also for the principal rooms of a Medieval house and for large central rooms in certain 19th- and 20th-century English and American houses. """@en;
  skos:exactMatch aat:300004441;
  skos:prefLabel "parlour"@en;
  skos:altLabel "hall"@en;
  skos:altLabel "best room"@en;
  skos:prefLabel "sejour"@fr;
  skos:prefLabel "pronkkamer"@nl;
  skos:prefLabel "beste Stube"@de;
  skos:inScheme dccd:objectElementType.
dccd:a7a2ca36-6b80-11e5-abf2-9bda48c69379 rdf:type skos:Concept;
  skos:scopeNote """Material derived from or comprising roots, which are parts of a plant that develop, growing typically from the radicle and downward into the soil."""@en;
  skos:exactMatch aat:300081475;
  skos:prefLabel "wurzelwerk"@de;
  skos:prefLabel "racines"@fr;
  skos:prefLabel "wortelstelsel"@nl;
  skos:prefLabel "roots"@en;
  skos:inScheme dccd:objectElementType.
dccd:a7a2d580-6b80-11e5-abff-c7cea56e4e4a rdf:type skos:Concept;
  skos:scopeNote """Buildings that house facilities for the housing and care of orphans, who are children whose parents are either dead or otherwise unable to care for their child."""@en;
  skos:exactMatch aat:300006769;
  skos:prefLabel "weeshuis"@nl;
  skos:prefLabel "orphelinat"@fr;
  skos:prefLabel "waisenhaus"@de;
  skos:prefLabel "orphanage"@en;
  skos:inScheme dccd:objectElementType.
dccd:a7a2d968-6b80-11e5-ac05-cfc3cb9d6c6a rdf:type skos:Concept;
  skos:scopeNote """Bodies of water serving as ways or routes for travel or transportation """@en;
  skos:exactMatch aat:300263418;
  skos:altLabel "voie d'eau"@fr;
  skos:prefLabel "waterway"@en;
  skos:prefLabel "waterweg"@nl;
  skos:prefLabel "voie navigable"@fr;
  skos:prefLabel "wasserstraße"@de;
  skos:inScheme dccd:objectElementType.
dccd:a7a2db34-6b80-11e5-ac06-3b3e4859a6b1 rdf:type skos:Concept;
  skos:scopeNote """A castle or stately home whose site is entirely surrounded by water-filled moats (moated castles) or natural waterbodies such as island castles in a river or offshore."""@en;
  skos:broadMatch aat:300005656;
  skos:prefLabel "waterburcht"@nl;
  skos:prefLabel "château-fort à douves"@fr;
  skos:prefLabel "watercastle"@en;
  skos:prefLabel "wasserburg"@de;
  skos:inScheme dccd:objectElementType.
dccd:a7a2dbe8-6b80-11e5-ac07-3bd42eaae36b rdf:type skos:Concept;
  skos:scopeNote """Implements or mechanisms used for defense or attack in combat, hunting, or war."""@en;
  skos:exactMatch aat:300036926;
  skos:prefLabel "wapen"@nl;
  skos:prefLabel "arme"@fr;
  skos:prefLabel "weapon"@en;
  skos:prefLabel "waffe"@de;
  skos:inScheme dccd:objectElementType.
dccd:a7a2dfd0-6b80-11e5-ac0d-cf2fdfdfbc96 rdf:type skos:Concept;
  skos:scopeNote """Any built structure used as a lookout station that affords observation of a surrounding area."""@en;
  skos:exactMatch aat:300134522;
  skos:altLabel "lookout tower"@en;
  skos:altLabel "wachttoren"@nl;
  skos:prefLabel "watchtower"@en;
  skos:prefLabel "tour de guet"@fr;
  skos:altLabel "wachtturm"@de;
  skos:prefLabel "wachturm"@de;
  skos:altLabel "uitkijktoren"@nl;
  skos:inScheme dccd:objectElementType.
dccd:a7a2e58e-6b80-11e5-ac16-e7b5b004826d rdf:type skos:Concept;
  skos:broadMatch aat:300045611;
  skos:altLabel "coffre"@fr;
  skos:altLabel "bac"@fr;
  skos:prefLabel "behälter"@de;
  skos:prefLabel "bak"@nl;
  skos:prefLabel "container"@en;
  skos:prefLabel "récipient"@fr;
  skos:inScheme dccd:objectElementType.
dccd:a7a2e638-6b80-11e5-ac17-6f09e2d2ba87 rdf:type skos:Concept;
  skos:scopeNote """Use for rafters placed at the juncture of the inclined planes forming hip roofs """@en;
  skos:exactMatch aat:300002431;
  skos:prefLabel "gratsparren"@de;
  skos:prefLabel "hip rafter"@en;
  skos:prefLabel "chevron d'arêtier"@fr;
  skos:prefLabel "hoekkeper"@nl;
  skos:inScheme dccd:objectElementType.
dccd:a7a2e6e2-6b80-11e5-ac18-bf94913bb2da rdf:type skos:Concept;
  skos:scopeNote """Use for rafters that do not extend from the roof plates to the ridgeboards; employed in hip roofs to reach from roof plates to hip rafters. For rafters spanning between valley rafters and ridgeboards, use 'valley jacks """@en;
  skos:exactMatch aat:300002434;
  skos:prefLabel "jack rafter"@en;
  skos:prefLabel "schifter"@de;
  skos:altLabel "schiftsparren"@de;
  skos:altLabel "karbeel"@nl;
  skos:prefLabel "verkorte spoor die tot aan de hoekkeper loopt"@nl;
  skos:altLabel "moise"@fr;
  skos:prefLabel "empanon"@fr;
  skos:inScheme dccd:objectElementType.
dccd:a7a2e782-6b80-11e5-ac19-6f5c5e97030d rdf:type skos:Concept;
  skos:scopeNote """Use for the main central part of an interior divided into a high center with lower side portions divided by columns or piers, usually but not always in a church. Use also for the main part of a church without aisles but with a distinct chancel"""@en;
  skos:exactMatch aat:300004627;
  skos:prefLabel "kerkruimte"@nl;
  skos:prefLabel "kirchenschiff"@de;
  skos:prefLabel "nave"@en;
  skos:prefLabel "nef"@fr;
  skos:inScheme dccd:objectElementType.
dccd:a7a2e82c-6b80-11e5-ac1a-ef7a55429a6a rdf:type skos:Concept;
  skos:scopeNote """Upward brace at the upper end of a frame running for example from a post to a wall plate"""@en;
  skos:broadMatch aat:300001834;
  skos:altLabel "curved brace"@en;
  skos:prefLabel "kopfband"@de;
  skos:prefLabel "guette"@fr;
  skos:altLabel "arch brace"@en;
  skos:altLabel "korbeel"@nl;
  skos:prefLabel "upward brace"@en;
  skos:altLabel "ascending bracae"@en;
  skos:prefLabel "schoor"@nl;
  skos:inScheme dccd:objectElementType.
dccd:a7a2e8d6-6b80-11e5-ac1b-af89ca1bff4a rdf:type skos:Concept;
  skos:scopeNote """Inclined timber rising from a beam to a rafter or principal rafter in roof constructions with knee walls."""@en;
  skos:broadMatch aat:300001834;
  skos:prefLabel "schubverteiler"@de;
  skos:prefLabel "sling brace"@en;
  skos:prefLabel "jambe de force"@fr;
  skos:prefLabel "kreupele stijl"@nl;
  skos:altLabel "post"@en;
  skos:altLabel "knee brace"@en;
  skos:inScheme dccd:objectElementType.
dccd:a7a2e980-6b80-11e5-ac1c-a324938ec043 rdf:type skos:Concept;
  skos:scopeNote """Long brace which crosses one or more vertical timbers"""@en;
  skos:broadMatch aat:300001834;
  skos:prefLabel "langstrebe"@de;
  skos:prefLabel "passing brace"@en;
  skos:prefLabel "écharpe"@fr;
  skos:prefLabel "kruisschoor"@nl;
  skos:inScheme dccd:objectElementType.
dccd:a7a2ea2a-6b80-11e5-ac1d-7feff7a3f669 rdf:type skos:Concept;
  skos:scopeNote """Horizontal members placed along the tops of walls or a series of studs to support joists or rafters """@en;
  skos:exactMatch aat:300001868;
  skos:prefLabel "mauerlatte"@de;
  skos:prefLabel "wall plate"@en;
  skos:prefLabel "sablière"@fr;
  skos:prefLabel "muurplaat"@nl;
  skos:inScheme dccd:objectElementType.
dccd:a7a2eaca-6b80-11e5-ac1e-6b2d55b7e84a rdf:type skos:Concept;
  skos:scopeNote """Series of vertical structural members which act as the supporting elements in a wall or partition."""@en;
  skos:exactMatch aat:300001882;
  skos:prefLabel "wandstijl"@nl;
  skos:prefLabel "wandständer"@de;
  skos:prefLabel "stud"@en;
  skos:prefLabel "poteau intermédiaire"@fr;
  skos:altLabel "muurstijl"@nl;
  skos:inScheme dccd:objectElementType.
dccd:a7a2eb74-6b80-11e5-ac1f-c775f5e8323d rdf:type skos:Concept;
  skos:broadMatch aat:300002424;
  skos:prefLabel "auflanger"@de;
  skos:prefLabel "aisle rafter"@en;
  skos:prefLabel "chevron de bas-côté"@fr;
  skos:prefLabel "oplanger"@nl;
  skos:inScheme dccd:objectElementType.
dccd:a7a2e1ba-6b80-11e5-ac10-6f527066854b rdf:type skos:Concept;
  skos:scopeNote """Use for the intersections of the sloping sides of roofs Use for the horizontal timbers laid across the principal rafters and supporting the common rafters in a roof """@en;
  skos:broadMatch aat:300002399;
  skos:prefLabel "firstpfette"@de;
  skos:altLabel "ridgepiece"@en;
  skos:prefLabel "ridge purlin"@en;
  skos:prefLabel "nokgording"@nl;
  skos:altLabel "piece faitière"@fr;
  skos:altLabel "faîtage"@fr;
  skos:altLabel "faîte"@fr;
  skos:altLabel "firstbalken"@de;
  skos:altLabel "nokbalk"@nl;
  skos:altLabel "ridge-beam"@en;
  skos:altLabel "ridge (pole/beam/piece)"@en;
  skos:altLabel "vorstbalk"@nl;
  skos:altLabel "vorst"@nl;
  skos:prefLabel "panne faitière"@fr;
  skos:altLabel "apex purlin"@en;
  skos:inScheme dccd:objectElementType.
dccd:a7a2cfae-6b80-11e5-abf6-fb6ac9d81235 rdf:type skos:Concept;
  skos:scopeNote """The strake immediately adjacent to the keel. There are two, one on each side of the keel."""@en;
  skos:broadMatch aat:300212614;
  skos:prefLabel "kielgang"@de;
  skos:prefLabel "zandstrook"@nl;
  skos:prefLabel "galbord"@fr;
  skos:prefLabel "garboard strake"@en;
  skos:inScheme dccd:objectElementType.
dccd:a7a2d0f8-6b80-11e5-abf8-ff3312346775 rdf:type skos:Concept;
  skos:scopeNote """V-shaped timber at the bow or the stern of a boat."""@en;
  skos:broadMatch aat:300212614;
  skos:prefLabel "wrange"@de;
  skos:prefLabel "wrang"@nl;
  skos:prefLabel "varangue"@fr;
  skos:prefLabel "floor timber (v-shaped)"@en;
  skos:inScheme dccd:objectElementType.
dccd:a7a2d436-6b80-11e5-abfd-f7a77e90a7b8 rdf:type skos:Concept;
  skos:scopeNote """Use broadly for all sorts of walls constructed to resist attack."""@en;
  skos:exactMatch aat:300002485;
  skos:prefLabel "mur de défense"@fr;
  skos:prefLabel "defensive wall"@en;
  skos:prefLabel "wehrmauer"@de;
  skos:prefLabel "weermuur"@nl;
  skos:inScheme dccd:objectElementType.
dccd:a7a2cf04-6b80-11e5-abf5-33866e83aa74 rdf:type skos:Concept;
  skos:scopeNote """Heavy transverse beam in which the mast is attached."""@en;
  skos:broadMatch aat:300212614;
  skos:prefLabel "mast beam"@en;
  skos:prefLabel "zeilbalk"@nl;
  skos:prefLabel "barrot de mât"@fr;
  skos:prefLabel "mastbalken"@de;
  skos:inScheme dccd:objectElementType.
dccd:a7a2df26-6b80-11e5-ac0c-6f0b8e77283e rdf:type skos:Concept;
  skos:scopeNote """Huts or boxes to shelter a sentry at his post."""@en;
  skos:exactMatch aat:6#http://vocab.getty.edu/aat/300048816;
  skos:altLabel "poste de guet"@fr;
  skos:prefLabel "poste de garde"@fr;
  skos:prefLabel "wachtpost"@nl;
  skos:prefLabel "wachtposten"@de;
  skos:prefLabel "sentry box"@en;
  skos:altLabel "guard post"@en;
  skos:inScheme dccd:objectElementType.
dccd:a7a2d38c-6b80-11e5-abfc-5b71ee2d176a rdf:type skos:Concept;
  skos:broadMatch aat:300212614;
  skos:altLabel "wegerplanke"@de;
  skos:prefLabel "ceiling plank"@en;
  skos:prefLabel "weger"@de;
  skos:prefLabel "vaigre"@fr;
  skos:prefLabel "weger"@nl;
  skos:altLabel "wegeringplank"@nl;
  skos:altLabel "bodenwegerung"@de;
  skos:inScheme dccd:objectElementType.
dccd:a7a2ecc8-6b80-11e5-ac21-8fac672b5a7b rdf:type skos:Concept;
  skos:scopeNote """A ram was a weapon carried by varied types of ships, dating back to antiquity. The weapon comprised an underwater prolongation of the bow of the ship to form an armoured beak, usually between six and 12 feet (2–4 m) in length. This would be driven into the hull of an enemy ship in order to puncture the hull and sink, or at least disable, that ship."""@en;
  skos:broadMatch aat:300203726;
  skos:prefLabel "rammbock"@de;
  skos:prefLabel "ram"@en;
  skos:prefLabel "bélier"@fr;
  skos:prefLabel "stormram"@nl;
  skos:inScheme dccd:objectElementType.
dccd:a7a2efde-6b80-11e5-ac22-a7ca8d1e7b86 rdf:type skos:Concept;
  skos:scopeNote """A type of manor house specific to Utrecht in Holland owner by one of the knighthood"""@en;
  skos:broadMatch aat:300005579;
  skos:prefLabel "ridderhofstad"@nl;
  skos:inScheme dccd:objectElementType.
dccd:a7a2f0b0-6b80-11e5-ac23-c7c7d44f97b3 rdf:type skos:Concept;
  skos:scopeNote """Small, usually isolated, fortification works of any form, commonly square or polygonal in plan, used to defend a prominent point"""@en;
  skos:broadMatch aat:300006888;
  skos:prefLabel "schanze"@de;
  skos:prefLabel "entrenchment"@en;
  skos:prefLabel "retranchement"@fr;
  skos:prefLabel "schans"@nl;
  skos:inScheme dccd:objectElementType.
dccd:a7a2f15a-6b80-11e5-ac24-8f9cdaba8bb1 rdf:type skos:Concept;
  skos:scopeNote """Wide plate of wood at the bottom of a posthold which prevents the post from sinking into the ground."""@en;
  skos:broadMatch aat:300078047;
  skos:prefLabel "pfostenschuh"@de;
  skos:prefLabel "post-pad"@en;
  skos:prefLabel "sabot"@fr;
  skos:prefLabel "paalschoen"@nl;
  skos:altLabel "patin (de bois)"@fr;
  skos:inScheme dccd:objectElementType.
dccd:a7a2f204-6b80-11e5-ac25-afb7ba91f44c rdf:type skos:Concept;
  skos:scopeNote """Blade in context of a water wheel"""@en;
  skos:broadMatch aat:300024617;
  skos:prefLabel "schaufel"@de;
  skos:prefLabel "blade"@en;
  skos:prefLabel "aube"@fr;
  skos:prefLabel "schoep"@nl;
  skos:inScheme dccd:objectElementType.
dccd:a7a2f2b8-6b80-11e5-ac26-23537fe2b26d rdf:type skos:Concept;
  skos:scopeNote """Inclined timber in the roof plane of a common rafter roof which crosses several rafters to provide lengthwise stability."""@en;
  skos:broadMatch aat:300001834;
  skos:altLabel "schwertlatte"@de;
  skos:altLabel "sturmlatte"@de;
  skos:altLabel "windlatte"@de;
  skos:altLabel "schrankhout"@nl;
  skos:prefLabel "windrispe"@de;
  skos:prefLabel "rafter brace"@en;
  skos:prefLabel "écharpe de contreventement"@fr;
  skos:prefLabel "windlat"@nl;
  skos:altLabel "sporenschrankhout"@nl;
  skos:inScheme dccd:objectElementType.
dccd:a7a2f362-6b80-11e5-ac27-db6fe564e933 rdf:type skos:Concept;
  skos:scopeNote """Types of construction in which walls, partitions, floors, and roof are wholly or partly made of wood; Use for constructions of any kind artificially fabricated of parts joined together in some definite manner and which may or may not provide enclosure or shelter??"""@en;
  skos:exactMatch aat:300111619;
  skos:prefLabel "gerüstbau"@de;
  skos:prefLabel "timber-framed construction"@en;
  skos:prefLabel "construction sur ossature"@fr;
  skos:prefLabel "houtskelebouw"@nl;
  skos:inScheme dccd:objectElementType.
dccd:a7a2f40c-6b80-11e5-ac28-cf95323d0a29 rdf:type skos:Concept;
  skos:scopeNote """Refers to the members that form the base of the roof truss and prevent the rafters from spreading."""@en;
  skos:exactMatch aat:300002419;
  skos:prefLabel "stuhlbalken"@de;
  skos:prefLabel "tie beam"@en;
  skos:prefLabel "faux-entrait de portique"@fr;
  skos:prefLabel "spantbalk"@nl;
  skos:inScheme dccd:objectElementType.
dccd:a7a2f4b6-6b80-11e5-ac29-bfb54ffedfd1 rdf:type skos:Concept;
  skos:scopeNote """Earliest type of European windmill. The defining feature is that the whole body of the mill that houses the machinery is mounted on a single vertical post, around which it can be turned to bring the sails into the wind."""@en;
  skos:broadMatch aat:300006273;
  skos:prefLabel "bockwindmühle"@de;
  skos:prefLabel "post mill"@en;
  skos:prefLabel "moulin sur pivot"@fr;
  skos:prefLabel "standerdmolen"@nl;
  skos:inScheme dccd:objectElementType.
dccd:a7a2f560-6b80-11e5-ac2a-8355c120e5f3 rdf:type skos:Concept;
  skos:scopeNote """Horizontal timber often resting on wooden or stone brackets or projection running adjacent to a wall but not an integrated part of the wall frame."""@en;
  skos:broadMatch aat:300001497;
  skos:prefLabel "streichbalken"@de;
  skos:prefLabel "applied beam"@en;
  skos:prefLabel "solive de rive"@fr;
  skos:prefLabel "strijkbalk"@nl;
  skos:inScheme dccd:objectElementType.
dccd:a7a2f60a-6b80-11e5-ac2b-afd750abcfb1 rdf:type skos:Concept;
  skos:scopeNote """Structural members whose primary function is to carry transverse loads"""@en;
  skos:exactMatch aat:300001497;
  skos:prefLabel "beam"@en;
  skos:prefLabel "balk"@nl;
  skos:prefLabel "balken"@de;
  skos:prefLabel "poutre"@fr;
  skos:altLabel "juk"@nl;
  skos:inScheme dccd:objectElementType.
dccd:a7a2f6b4-6b80-11e5-ac2c-fb98219bacee rdf:type skos:Concept;
  skos:scopeNote """Small hills, small elevations in the earth's surface, or small mounds or heaps of earth or stones."""@en;
  skos:exactMatch aat:300008781;
  skos:altLabel "knoll"@en;
  skos:altLabel "butte"@fr;
  skos:altLabel "monticule"@fr;
  skos:prefLabel "wurte"@de;
  skos:prefLabel "tetre"@fr;
  skos:prefLabel "terp"@nl;
  skos:prefLabel "hillock"@en;
  skos:inScheme dccd:objectElementType.
dccd:a7a2f768-6b80-11e5-ac2d-0f3535f98c4b rdf:type skos:Concept;
  skos:scopeNote """Pieces of wood or metal tapering to a thin edge; used to adjust elevation or tighten formwork, or to split wood or rock."""@en;
  skos:exactMatch aat:300024101;
  skos:prefLabel "wig"@nl;
  skos:prefLabel "coin"@fr;
  skos:prefLabel "wedge"@en;
  skos:prefLabel "keil"@de;
  skos:inScheme dccd:objectElementType.
dccd:a7a2f808-6b80-11e5-ac2e-2bcc0d81be52 rdf:type skos:Concept;
  skos:scopeNote """Large artificial mound in the Netherlands used to provide refuge for during a seasonally flood"""@en;
  skos:broadMatch aat:300008024;
  skos:prefLabel "wierde"@nl;
  skos:prefLabel "tertre"@fr;
  skos:prefLabel "terp"@en;
  skos:prefLabel "warft"@de;
  skos:inScheme dccd:objectElementType.
dccd:a7a2f8c6-6b80-11e5-ac2f-9fe50a029482 rdf:type skos:Concept;
  skos:scopeNote """Artificial paved banks or solid landing places built parallel to and extending the shoreline to serve in the loading and unloading of vessels. For less fixed and solid structures built in similar locations and for similar purposes, use 'wharves'; use 'piers (marine landings)' when such lighter structures extend out over the water."""@en;
  skos:exactMatch aat:300120782;
  skos:prefLabel "kai"@de;
  skos:prefLabel "quay"@en;
  skos:prefLabel "quai"@fr;
  skos:prefLabel "kade"@nl;
  skos:inScheme dccd:objectElementType.
dccd:a7a2f970-6b80-11e5-ac30-67d32cb0131b rdf:type skos:Concept;
  skos:scopeNote """Structures, in post-Second World War contexts, built generally parallel to the shoreline so that vessels may moor alongside to receive or discharge cargo or passengers; prior to the mid-20th century, may refer broadly to any such landing places. For similar loading and unloading places built to extend from the shoreline out over water, use 'piers (marine landings)'; if such places are artificial solid banks or shoreline extensions built parallel to the shoreline, use 'quays.'"""@en;
  skos:exactMatch aat:300120786;
  skos:prefLabel "wharf"@en;
  skos:prefLabel "werf"@nl;
  skos:inScheme dccd:objectElementType.
dccd:a7a2fa1a-6b80-11e5-ac31-a3d029d44e0c rdf:type skos:Concept;
  skos:scopeNote """Use, in post-Second World War contexts, for structures built generally parallel to the shoreline so that vessels may moor alongside to receive or discharge cargo or passengers; prior to the mid-20th century, may refer broadly to any such landing places. For similar loading and unloading places built to extend from the shoreline out over water, use 'piers (marine landings)'; if such places are artificial solid banks or shoreline extensions built parallel to the shoreline, use 'quays.'
Use for any of various structures built for loading or unloading goods or embarking or disembarking passengers onto and off of watercraft.
Use for artificial paved banks or solid landing places built parallel to and extending the shoreline to serve in the loading and unloading of vessels. For less fixed and solid structures built in similar locations and for similar purposes, use 'wharves'; use 'piers (marine landings)' when such lighter structures extend out over the water"""@en;
  skos:exactMatch aat:300007928;
  skos:altLabel "anlege"@de;
  skos:altLabel "anlegeplatz"@de;
  skos:altLabel "anlegestelle"@de;
  skos:altLabel "bootssteg"@de;
  skos:altLabel "landungsbrücke"@de;
  skos:altLabel "landungsplatz"@de;
  skos:altLabel "landungsstelle"@de;
  skos:altLabel "steg"@de;
  skos:altLabel "landing stage"@en;
  skos:altLabel "débarcadère"@fr;
  skos:altLabel "embarcadère"@fr;
  skos:altLabel "ponton"@fr;
  skos:altLabel "aanlegplaats"@nl;
  skos:altLabel "aanlegsteiger"@nl;
  skos:prefLabel "landing place"@en;
  skos:prefLabel "landingsplaats"@nl;
  skos:prefLabel "landung"@de;
  skos:prefLabel "atterrissage"@fr;
  skos:inScheme dccd:objectElementType.
dccd:a7a2fae2-6b80-11e5-ac32-d3cdf7f09544 rdf:type skos:Concept;
  skos:scopeNote """Long narrow excavations, usually with sloping sides, dug in the earth for defense, drainage, or irrigation."""@en;
  skos:exactMatch aat:300006178;
  skos:prefLabel "graben"@de;
  skos:prefLabel "greppel"@nl;
  skos:prefLabel "fossé"@fr;
  skos:prefLabel "ditch"@en;
  skos:altLabel "sloot"@nl;
  skos:inScheme dccd:objectElementType.
dccd:a7a2fb8c-6b80-11e5-ac33-b7bbe7d0e283 rdf:type skos:Concept;
  skos:scopeNote """Beam carrying a floor which forms a ceiling covering of a room"""@en;
  skos:exactMatch aat:300375090;
  skos:altLabel "vloerbalk"@nl;
  skos:altLabel "flurträger"@de;
  skos:altLabel "solive"@fr;
  skos:altLabel "joisting"@en;
  skos:altLabel "floor frame"@en;
  skos:prefLabel "floor joist"@en;
  skos:prefLabel "sommier"@fr;
  skos:prefLabel "vloerbalk"@nl;
  skos:prefLabel "deckenbalken"@de;
  skos:altLabel "ceiling joist"@en;
  skos:inScheme dccd:objectElementType.
dccd:a7a2fc40-6b80-11e5-ac34-b388a286cdde rdf:type skos:Concept;
  skos:scopeNote """Refers to deep, wide defensive ditches surrounding towns, castles, or houses and usually filled with water."""@en;
  skos:exactMatch aat:300003716;
  skos:prefLabel "wassergraben"@de;
  skos:prefLabel "moat"@en;
  skos:altLabel "burggraben"@de;
  skos:inScheme dccd:objectElementType.
dccd:a7a2fd94-6b80-11e5-ac36-77cd38447a8c rdf:type skos:Concept;
  skos:scopeNote """Water distribution structures"""@en;
  skos:broadMatch aat:300006164;
  skos:prefLabel "canalisation d'eau"@fr;
  skos:prefLabel "waterleiding"@nl;
  skos:prefLabel "wasserleitung"@de;
  skos:prefLabel "water pipe"@en;
  skos:altLabel "water conduit"@en;
  skos:altLabel "conduite d'eau"@fr;
  skos:inScheme dccd:objectElementType.
dccd:a7a20506-6b80-11e5-aadf-fbad49e629f1 rdf:type skos:Concept;
  skos:scopeNote """Short joist or beam set at right angles to interrupted joists to carry their ends.  Allows an opening through a fllor, for example for a chimney or a stair."""@en;
  skos:exactMatch aat:300001848;
  skos:altLabel "wechsel"@de;
  skos:altLabel "gousset"@fr;
  skos:altLabel "linçoir"@fr;
  skos:prefLabel "trimmer"@en;
  skos:prefLabel "chevêtre"@fr;
  skos:prefLabel "raveelbalk"@nl;
  skos:prefLabel "wechselbalken"@de;
  skos:altLabel "header"@en;
  skos:altLabel "trimmer joist"@en;
  skos:altLabel "trimmer beam"@en;
  skos:inScheme dccd:objectElementType.
dccd:a7a1b920-6b80-11e5-aa78-0f19e75e5a25 rdf:type skos:Concept;
  skos:scopeNote """Devices or assemblies of devices designed to support artillery and heavy small arms such as machine guns. They range from simple tripods to complex supporting, pivoting, and elevating mechanisms on gun carriages."""@en;
  skos:closeMatch aat:300221835;
  skos:altLabel "rolpaard"@nl;
  skos:prefLabel "lafette"@de;
  skos:prefLabel "carriage"@en;
  skos:prefLabel "affût"@fr;
  skos:prefLabel "affuit"@nl;
  skos:inScheme dccd:objectElementType.
dccd:a7a2fcea-6b80-11e5-ac35-c7e2cc964ee6 rdf:type skos:Concept;
  skos:scopeNote """Long, narrow, usually steep-sided cuts into the earth, as to receive pipes, wires, or footings; may also be used for defensive cuts, especially when the excavated earth is heaped in front as a barrier. For defensive cuts in which the earth is not used as added protection, use 'fosses' or 'moats.'"""@en;
  skos:exactMatch aat:300008022;
  skos:prefLabel "loopgraaf"@nl;
  skos:prefLabel "graben"@de;
  skos:prefLabel "tranchée"@fr;
  skos:altLabel "channel"@en;
  skos:altLabel "cutting"@en;
  skos:prefLabel "trench"@en;
  skos:inScheme dccd:objectElementType.
dccd:a7a2d058-6b80-11e5-abf7-d3eb86763f85 rdf:type skos:Concept;
  skos:scopeNote """A member which, particularly in a wooden vessel, lies parallel with its keel but above the transverse members such as timbers, frames or in a larger vessel, floors. It is fastened to the keel partly to impart additional longitudinal stiffness to it but principally to bind the longitudinal members (keel and hog) to the transverse members (frames and floors)."""@en;
  skos:broadMatch aat:300212614;
  skos:prefLabel "zaathout"@nl;
  skos:prefLabel "kielschwein"@de;
  skos:prefLabel "keelson"@en;
  skos:prefLabel "carlingue"@fr;
  skos:altLabel "kelson"@en;
  skos:inScheme dccd:objectElementType.
dccd:a7a2d2ec-6b80-11e5-abfb-c315e4efe4f4 rdf:type skos:Concept;
  skos:scopeNote """The interior lining between ports and the overhead interior surface of the cabin"""@en;
  skos:broadMatch aat:300212614;
  skos:altLabel "innenplanke"@de;
  skos:altLabel "wegerung"@de;
  skos:altLabel "ceiling"@en;
  skos:altLabel "spirketting"@en;
  skos:altLabel "feuilles bretonnes"@fr;
  skos:altLabel "seuillet"@fr;
  skos:altLabel "vaigrage"@fr;
  skos:altLabel "wegering"@nl;
  skos:inScheme dccd:objectElementType.
dccd:a7a2006a-6b80-11e5-aad8-b3302592f31a rdf:type skos:Concept;
  skos:scopeNote """In architecture, upright posts supporting the handrail at the top and bottom of a stairway or at the turn on a landing; also, the main posts about which circular staircases wind."""@en;
  skos:exactMatch aat:300003296;
  skos:prefLabel "spindel"@de;
  skos:prefLabel "newel (post)"@en;
  skos:prefLabel "noyeau"@fr;
  skos:prefLabel "trapspil"@nl;
  skos:altLabel "spil van een wenteltrap"@nl;
  skos:inScheme dccd:objectElementType.
dccd:a7a1e076-6b80-11e5-aaab-cb07216f4fab rdf:type skos:Concept;
  skos:scopeNote """Timber framework of a roof supporting the covering"""@en;
  skos:closeMatch aat:300125741;
  skos:altLabel "truss"@en;
  skos:altLabel "binder"@de;
  skos:altLabel "roof framing"@en;
  skos:altLabel "dachstuhl"@de;
  skos:altLabel "dachgebinde"@de;
  skos:altLabel "roof truss(es)"@en;
  skos:prefLabel "dachwerk"@de;
  skos:altLabel "combles"@fr;
  skos:prefLabel "roof construction"@en;
  skos:prefLabel "charpente"@fr;
  skos:altLabel "charpente de toiture"@fr;
  skos:altLabel "charpente de comble"@fr;
  skos:prefLabel "kapconstructie"@nl;
  skos:altLabel "dachgerüst"@de;
  skos:altLabel "dachtragwerk"@de;
  skos:inScheme dccd:objectElementType.
dccd:a7a223b0-6b80-11e5-ab0a-0357a6a30177 rdf:type skos:Concept;
  skos:scopeNote """Traverse beam trying a pair of posts to each other so that their sideways movement is prevented."""@en;
  skos:broadMatch aat:300001497;
  skos:altLabel "tussenbalk"@nl;
  skos:altLabel "zwischenbalken"@de;
  skos:altLabel "faux-entrait"@fr;
  skos:prefLabel "ankerbalken"@de;
  skos:prefLabel "anchor beam"@en;
  skos:prefLabel "entrait de portique"@fr;
  skos:prefLabel "ankerbalk"@nl;
  skos:inScheme dccd:objectElementType.
dccd:a7a1db3a-6b80-11e5-aaa3-7f7a21d2bfdf rdf:type skos:Concept;
  skos:scopeNote """Buildings equipped with machinery for grinding grain into flour."""@en;
  skos:exactMatch aat:300006286;
  skos:prefLabel "mühle"@de;
  skos:altLabel "mill"@en;
  skos:altLabel "molen"@nl;
  skos:altLabel "moulin"@fr;
  skos:prefLabel "flour mill"@;
  skos:prefLabel "meelfabriek"@nl;
  skos:prefLabel "moulin à farine"@fr;
  skos:inScheme dccd:objectElementType.
dccd:27171b0a-6c53-11e5-9a23-5739630d10e1 rdf:type skos:Concept;
  skos:scopeNote """Part of the shell of the hull of a boat or ship which, in conjunction with the other strakes, keeps the sea out and the vessel afloat. It is a strip of planking in a wooden vessel or of plating in a metal one, running longitudinally along the vessel's side, bottom or the turn of the bilge, usually from one end of the vessel to the other. On a longboat, one strake will typically be made up of numerous planks running end to end."""@en;
  skos:broadMatch aat:300212614;
  skos:prefLabel "strake"@en;
  skos:prefLabel "gang"@nl;
  skos:prefLabel "gang"@de;
  skos:altLabel "plankengang"@de;
  skos:prefLabel "virure"@fr;
  skos:broader dccd:a7a1cba4-6b80-11e5-aa8f-7b893ed983e4;
  skos:broader dccd:a7a24b38-6b80-11e5-ab41-d355b2ffeae7;
  skos:broader dccd:a7a230c6-6b80-11e5-ab1e-2b12aed0d631;
  skos:broader dccd:a7a24d2c-6b80-11e5-ab44-c75a3a6c2748;
  skos:inScheme dccd:objectElementType.
dccd:a7a1fd22-6b80-11e5-aad3-1b41b1704c65 rdf:type skos:Concept;
  skos:scopeNote """Framed construction made of vertical borizonal and diagonal timbers.  The spaces may have infill e.g. of wattle and daub."""@en;
  skos:broadMatch aat:300004790;
  skos:altLabel "fachwerk"@de;
  skos:prefLabel "vakwerk"@nl;
  skos:prefLabel "pan de bois"@fr;
  skos:altLabel "charpente à treilis"@fr;
  skos:altLabel "charpente triangulée"@fr;
  skos:prefLabel "timber framing"@en;
  skos:altLabel "framed building"@en;
  skos:altLabel "half timber work"@en;
  skos:altLabel "structure de colombages"@fr;
  skos:altLabel "vakwerkbouw"@nl;
  skos:altLabel "fachwerkbau"@de;
  skos:inScheme dccd:objectElementType.
dccd:a7a1f426-6b80-11e5-aac9-dfac25af0b6e rdf:type skos:Concept;
  skos:scopeNote """An obstruction placed in tidal waters, or wholly or partially across a river, to direct the passage of fish."""@en;
  skos:broadMatch aat:300247419;
  skos:altLabel "fischwehr"@de;
  skos:altLabel "temps pour la pêche"@fr;
  skos:altLabel "visweer"@nl;
  skos:prefLabel "fishing weir"@en;
  skos:altLabel "kiddle"@en;
  skos:altLabel "fishgarth"@en;
  skos:inScheme dccd:objectElementType.
dccd:02e8846a-6c55-11e5-9a26-5b6cbc576023 rdf:type skos:Concept;
  skos:scopeNote """Section of a building, roofed at an angle to the (often broader and taller) main range."""@en;
  skos:exactMatch aat:300004188;
  skos:prefLabel "wing"@en;
  skos:prefLabel "seitenflügel"@de;
  skos:prefLabel "zijvleugel"@nl;
  skos:altLabel "vleugel"@nl;
  skos:prefLabel "aile"@fr;
  skos:inScheme dccd:objectElementType.
dccd:a7a2d242-6b80-11e5-abfa-ef7dcc407f8f rdf:type skos:Concept;
  skos:scopeNote """ Buildings or devices with sails or vanes that turn in the wind and generate power. The devices operate by means of a rotating shaft on which sails are mounted or placed at an angle so that the force of wind against them causes rotation, which in turn produced energy. Windmills were historically used chiefly in flat districts for operating a mill to grind grain or pump water; the older and most characteristic European form consists of a conical mill-house with a dome or cap supporting four sails. Modern devices tap the wind to produce electricity by using a disk of sails mounted on a framework."""@en;
  skos:exactMatch aat:300006273;
  skos:prefLabel "windmill"@en;
  skos:prefLabel "windmolen"@nl;
  skos:prefLabel "moulin à vent"@fr;
  skos:prefLabel "windmühle"@de;
  skos:inScheme dccd:objectElementType.
dccd:69e49f8e-6c58-11e5-9a27-db85dd163663 rdf:type skos:Concept;
  skos:scopeNote """Load-bearing upgrifht constructional timber which forms a part of a wall.  It is dug or rammed into the ground."""@en;
  skos:exactMatch aat:300000938;
  skos:prefLabel "poteau"@fr;
  skos:prefLabel "pile"@en;
  skos:prefLabel "pfahl"@de;
  skos:prefLabel "paal"@nl;
  skos:inScheme dccd:objectElementType.
dccd:a7a2e304-6b80-11e5-ac12-f73ce7356e81 rdf:type skos:Concept;
  skos:scopeNote """The stem is the most forward part of a boat or ship's bow [1] and is an extension of the keel itself. The stem is the curved edge stretching from the keel below, up to the gunwale of the boat. The stem is more often found on wooden boats or ships, but not exclusively."""@en;
  skos:broadMatch aat:300263190;
  skos:altLabel "vordersteven"@de;
  skos:altLabel "voorsteven"@nl;
  skos:altLabel "vorsteven"@de;
  skos:prefLabel "étrave"@fr;
  skos:prefLabel "steven"@nl;
  skos:prefLabel "stem"@en;
  skos:prefLabel "steven"@de;
  skos:inScheme dccd:objectElementType.
dccd:a7a1c032-6b80-11e5-aa7e-477bb4b790c9 rdf:type skos:Concept;
  skos:scopeNote """Tall spar, or arrangement of spars, erected more or less vertically on the centre-line of a ship or boat. Its purposes include carrying sail, spars, and derricks."""@en;
  skos:broadMatch aat:300212614;
  skos:prefLabel "mast"@de;
  skos:prefLabel "mast"@en;
  skos:prefLabel "mast"@nl;
  skos:prefLabel "mât"@fr;
  skos:altLabel "standerd"@nl;
  skos:inScheme dccd:objectElementType.
dccd:a7a2c45a-6b80-11e5-abe9-dfb51fd8aa9e rdf:type skos:Concept;
  skos:scopeNote """A public building at or within which goods, and the like, are weighed. Most of these buildings were built before 1800, prior to the establishment of international standards for weights"""@en;
  skos:exactMatch aat:300312276;
  skos:prefLabel "waaggebouw"@nl;
  skos:prefLabel "weighhouse"@en;
  skos:prefLabel "poids public"@fr;
  skos:prefLabel "wiegehaus"@de;
  skos:inScheme dccd:objectElementType.
dccd:5b54afde-6c5a-11e5-9a29-7f859992c690 rdf:type skos:Concept;
  skos:scopeNote """In architecture or other construction, refers to stiff, vertical, relatively isolated members of considerable length. Posts are typically round, square, or rectangular in cross-section and are used in building as supports for a superstructure or to provide a firm point of lateral attachment. They are characteristically relatively undecorated and made of a single timber, but may be made of stone, metal, another material, or composite materials. The term is particularly used for any main vertical support in a timber frame structure. For square uprights in classical style, and for square and rectangular masonry uprights, use 'piers (supporting elements)'; for most cylindrical uprights, and for all uprights in steel and concrete frames, use 'columns (architectural elements).'"""@en;
  skos:exactMatch aat:300001609;
  skos:prefLabel "ständer"@de;
  skos:prefLabel "staander"@nl;
  skos:prefLabel "pfosten"@de;
  skos:prefLabel "post"@en;
  skos:altLabel "post"@nl;
  skos:inScheme dccd:objectElementType.
dccd:a7a2de86-6b80-11e5-ac0b-a73dda05ae89 rdf:type skos:Concept;
  skos:scopeNote """Refers to panels of oak or other wood that is used to line the walls of a room. It often refers specifically to the decorative or protective facings applied to the lower portion of an interior partition or wall, whether of wood or another material. The term originally referred to a superior quality of oak from Russia, Germany, and Holland, that was used primarily for fine panel-work."""@en;
  skos:exactMatch aat:300002691;
  skos:prefLabel "wainscot"@en;
  skos:prefLabel "wagenschot"@nl;
  skos:prefLabel "täfelung"@de;
  skos:prefLabel "lambris"@fr;
  skos:inScheme dccd:objectElementType.
dccd:a7a2d62a-6b80-11e5-ac00-2fe78140a7ed rdf:type skos:Concept;
  skos:scopeNote """Refers to a device utilizing a water wheel or otherwise operated by water with the purpose of running a mill to grind grain or to produce or process a product. It may also typically refers to the building or structure housing or supporting the device."""@en;
  skos:exactMatch aat:300006270;
  skos:altLabel "moulin hydraulique"@fr;
  skos:altLabel "waterradmolen"@nl;
  skos:prefLabel "water mill"@en;
  skos:prefLabel "watermolen"@nl;
  skos:prefLabel "moulin à eau"@fr;
  skos:prefLabel "wassermühle"@de;
  skos:inScheme dccd:objectElementType.
dccd:a7a22cde-6b80-11e5-ab18-dfa391c59cfb rdf:type skos:Concept;
  skos:scopeNote """Stiffening deck member supported at its extremities by knee connections to frames or bulkheads"""@en;
  skos:broadMatch aat:300212614;
  skos:prefLabel "decksbalken"@de;
  skos:prefLabel "deckbeam"@en;
  skos:prefLabel "barrot (de pont)"@fr;
  skos:prefLabel "dekbalk"@nl;
  skos:inScheme dccd:objectElementType.
dccd:a7a23ac6-6b80-11e5-ab2a-93eab5e83229 rdf:type skos:Concept;
  skos:scopeNote """shipsterm """@en;
  skos:broadMatch aat:300212614;
  skos:altLabel "passerelle"@fr;
  skos:altLabel "passe-avant"@fr;
  skos:prefLabel "gangbord"@de;
  skos:prefLabel "gangway"@en;
  skos:prefLabel "passavant"@fr;
  skos:prefLabel "gangboord"@nl;
  skos:inScheme dccd:objectElementType.
dccd:a7a2494e-6b80-11e5-ab3e-83f74bfaa123 rdf:type skos:Concept;
  skos:scopeNote """Timber that is part of the transom, i.e. the surface the forms the stern of a boat"""@en;
  skos:broadMatch aat:300212614;
  skos:altLabel "wing transom"@en;
  skos:altLabel "barre d' hourdi"@fr;
  skos:prefLabel "heckbalken"@de;
  skos:prefLabel "transom timber"@en;
  skos:prefLabel "lisse d' hourdi"@fr;
  skos:prefLabel "hekbalk"@nl;
  skos:inScheme dccd:objectElementType.
dccd:a7a24d2c-6b80-11e5-ab44-c75a3a6c2748 rdf:type skos:Concept;
  skos:scopeNote """Short strake employed to reduce the width of plank required where the girth of the hull increases or is necessary due to a tuck in the shape. It is commonly employed in carvel and iron/steel shipbuilding"""@en;
  skos:broadMatch aat:300212614;
  skos:altLabel "totgang"@de;
  skos:prefLabel "splissgang"@de;
  skos:prefLabel "stealer"@en;
  skos:prefLabel "virure perdue"@fr;
  skos:prefLabel "insteker"@nl;
  skos:broader dccd:27171b0a-6c53-11e5-9a23-5739630d10e1;
  skos:inScheme dccd:objectElementType.
dccd:a7a24dcc-6b80-11e5-ab45-eb04951ef6b1 rdf:type skos:Concept;
  skos:scopeNote """A piece of wood let into a wooden hull to replace decayed wood"""@en;
  skos:broadMatch aat:300212614;
  skos:altLabel "spunt"@de;
  skos:altLabel "rombaillet"@fr;
  skos:prefLabel "spund"@de;
  skos:prefLabel "graving piece"@en;
  skos:prefLabel "romaillet"@fr;
  skos:prefLabel "inzetstuk"@nl;
  skos:inScheme dccd:objectElementType.
dccd:a7a254de-6b80-11e5-ab50-43ef22485048 rdf:type skos:Concept;
  skos:scopeNote """shipsterm """@en;
  skos:broadMatch aat:300212614;
  skos:prefLabel "kielplanke"@de;
  skos:prefLabel "keel plank"@en;
  skos:prefLabel "bordage de quille"@fr;
  skos:prefLabel "kielplank"@nl;
  skos:inScheme dccd:objectElementType.
dccd:a7a25ede-6b80-11e5-ab5b-9b6c10b3eec0 rdf:type skos:Concept;
  skos:scopeNote """shipsterm """@en;
  skos:broadMatch aat:300212614;
  skos:prefLabel "knie"@de;
  skos:prefLabel "knee"@en;
  skos:prefLabel "courbe"@fr;
  skos:prefLabel "knie"@nl;
  skos:inScheme dccd:objectElementType.
dccd:a7a26de8-6b80-11e5-ab72-1fef4843fbf5 rdf:type skos:Concept;
  skos:broadMatch aat:300212614;
  skos:altLabel "foundation hole"@en;
  skos:prefLabel "mastspur"@de;
  skos:prefLabel "mast step"@en;
  skos:prefLabel "emplanture de mât"@fr;
  skos:prefLabel "mastspoor"@nl;
  skos:inScheme dccd:objectElementType.
dccd:a7a26e88-6b80-11e5-ab73-3b0269fd93c5 rdf:type skos:Concept;
  skos:scopeNote """Movable or fixed objects or equipment, which may be either functional or ornamental, particularly objects for sitting, reclining, or storage, such as chairs, beds, tables, cabinets, etc., in a dwelling, business, or public space."""@en;
  skos:exactMatch aat:300037680;
  skos:prefLabel "möbel"@de;
  skos:prefLabel "furniture"@en;
  skos:prefLabel "meuble"@fr;
  skos:prefLabel "meubel"@nl;
  skos:inScheme dccd:objectElementType.
dccd:a7a25a2e-6b80-11e5-ab54-d79279af2a97 rdf:type skos:Concept;
  skos:scopeNote """Use for openings in horizontal positions, as between the decks of a ship, and for doors horizontally divided, the upper part being opened for ventilation or so that articles may be passed over the lower part """@en;
  skos:broadMatch aat:300212614;
  skos:prefLabel "untertür"@de;
  skos:prefLabel "hatch"@en;
  skos:prefLabel "puce"@fr;
  skos:prefLabel "onderdeur"@nl;
  skos:inScheme dccd:objectElementType.
dccd:a7a278b0-6b80-11e5-ab7f-3b511552498a rdf:type skos:Concept;
  skos:scopeNote """A beam in a double flooring system which provides intermediate support to a series of floor beams nad reduces their span.  Is alsways situated below the floow beams and of approximately equal thickness."""@en;
  skos:exactMatch aat:300001833;
  skos:altLabel "onderslag"@nl;
  skos:prefLabel "unterzug"@de;
  skos:prefLabel "binder"@en;
  skos:prefLabel "poutre"@fr;
  skos:prefLabel "onderslagbalk"@nl;
  skos:inScheme dccd:objectElementType.
dccd:a7a28ed6-6b80-11e5-aba1-4b3605e4f5b9 rdf:type skos:Concept;
  skos:broadMatch aat:300212614;
  skos:prefLabel "roof"@de;
  skos:prefLabel "deck house"@en;
  skos:prefLabel "rouf"@fr;
  skos:prefLabel "roef"@nl;
  skos:inScheme dccd:objectElementType.
dccd:a7a29bb0-6b80-11e5-abb1-5b2a5fe42f95 rdf:type skos:Concept;
  skos:scopeNote """Upright wall within the hull of a ship"""@en;
  skos:broadMatch aat:300212614;
  skos:altLabel "schot"@nl;
  skos:prefLabel "schott"@de;
  skos:prefLabel "bulkhead"@en;
  skos:prefLabel "cloison"@fr;
  skos:prefLabel "scheidingswand"@nl;
  skos:inScheme dccd:objectElementType.
dccd:a7a2a902-6b80-11e5-abc5-3bb7676ae3cd rdf:type skos:Concept;
  skos:scopeNote """Upright structural member or post at the stern of a (generally wooden) ship or a boat, to which are attached the transoms and the rearmost left corner part of the stern."""@en;
  skos:broadMatch aat:300212614;
  skos:prefLabel "stevenbalken"@de;
  skos:prefLabel "barrot de poupe (arrière)/proue (avant)"@fr;
  skos:prefLabel "stevenbalk"@nl;
  skos:altLabel "stem post"@en;
  skos:prefLabel "sternpost"@en;
  skos:inScheme dccd:objectElementType.
dccd:a7a2ad58-6b80-11e5-abca-ebfe3098e810 rdf:type skos:Concept;
  skos:scopeNote """Oversized oar or board to control the direction of a ship or other watercraft prior to the invention of the rudder."""@en;
  skos:broadMatch aat:300213077;
  skos:altLabel "gouvernail-rame"@fr;
  skos:prefLabel "steuerriemen"@de;
  skos:prefLabel "steering oar"@en;
  skos:prefLabel "aviron de queue"@fr;
  skos:prefLabel "stuurriem"@nl;
  skos:inScheme dccd:objectElementType.

##############################################################
Following entries are missing any sort of AAT match
##############################################################
dccd:a7a23756-6b80-11e5-ab28-47b8e3d19c0e rdf:type skos:Concept;
  skos:scopeNote """Field in which a gallows stands"""@en;
  skos:prefLabel "galgenacker"@de;
  skos:prefLabel "gallows field"@en;
  skos:prefLabel "galgenveld"@nl;
  skos:inScheme dccd:objectElementType.
dccd:a7a28c42-6b80-11e5-ab9d-8b53286b9c54 rdf:type skos:Concept;
  skos:prefLabel "refugium"@de;
  skos:prefLabel "refugium"@en;
  skos:prefLabel "refugium"@fr;
  skos:prefLabel "refugehuis"@nl;
  skos:inScheme dccd:objectElementType.
dccd:a7a27aa4-6b80-11e5-ab82-073e553fa8e5 rdf:type skos:Concept;
  skos:prefLabel "rahmen"@de;
  skos:prefLabel "frame"@en;
  skos:prefLabel "cadre"@fr;
  skos:prefLabel "lijst"@nl;
  skos:inScheme dccd:objectElementType.
dccd:a7a27ea0-6b80-11e5-ab88-0b3c1f6771af rdf:type skos:Concept;
  skos:prefLabel "flügelrute"@de;
  skos:prefLabel "whip"@en;
  skos:prefLabel "scion"@fr;
  skos:prefLabel "oplanger"@nl;
  skos:inScheme dccd:objectElementType.
dccd:0f56a390-6c59-11e5-9a28-d354e8d82baf rdf:type skos:Concept;
  skos:scopeNote """Vertical timber in a timber-framed wall which in contrast to a post, is hardly load-bearing."""@en;
  skos:prefLabel "stijl"@nl;
  skos:prefLabel "puncheon"@en;
  skos:prefLabel "stiel"@de;
  skos:altLabel "stud (short)"@en;
  skos:prefLabel "potelet"@fr;
  skos:inScheme dccd:objectElementType.

##############################################################
Following entries need further checking by content specialists
##############################################################
dccd:a7a1d022-6b80-11e5-aa96-d7590262ad57 rdf:type skos:Concept;
  skos:editorialNote: """Needs clarification.  Panneau and plaat used in DCCD."""@en;
  skos:altLabel "bohle"@de;
  skos:altLabel "rähm"@de;
  skos:altLabel "plate"@en;
  skos:altLabel "feuille"@fr;
  skos:altLabel "panneau"@fr;
  skos:altLabel "plaat"@nl;
  skos:inScheme dccd:objectElementType.
dccd:a7a1eaf8-6b80-11e5-aabb-9376e14a7ea3 rdf:type skos:Concept;
  skos:editorialNote: """What is this? Travee used in DCCD."""@en;
  skos:altLabel "joch"@de;
  skos:altLabel "bay"@en;
  skos:altLabel "travée"@fr;
  skos:altLabel "travee"@nl;
  skos:inScheme dccd:objectElementType.
dccd:a7a201be-6b80-11e5-aada-076472dd2f4b rdf:type skos:Concept;
  skos:editorialNote: """Needs checking with Dirk Jan de Vries. Tafelment used in DCCD."""@en;
  skos:altLabel "balkenlage worauf zimmerwerk ruht"@de;
  skos:altLabel "tabling"@en;
  skos:altLabel "chaise stercoraire"@fr;
  skos:altLabel "tafelment"@nl;
  skos:inScheme dccd:objectElementType.
dccd:a7a2284c-6b80-11e5-ab11-0ffd1cfc9fc3 rdf:type skos:Concept;
  skos:editorialNote: """Specific to Watercraft?!? Legger used in DCCD."""@en;
  skos:altLabel "legger"@nl;
  skos:prefLabel "bodenwrange"@de;
  skos:prefLabel "floor timber"@en;
  skos:prefLabel "varangue plate"@fr;
  skos:prefLabel "buikstuk"@nl;
  skos:inScheme dccd:objectElementType.
dccd:a7a22aea-6b80-11e5-ab15-c365bef70e8a rdf:type skos:Concept;
  skos:editorialNote: """Needs clarification"""@en;
  skos:prefLabel "konsole"@de;
  skos:prefLabel "bracket"@en;
  skos:prefLabel "console"@fr;
  skos:prefLabel "console"@nl;
  skos:inScheme dccd:objectElementType.
dccd:a7a2b7da-6b80-11e5-abd6-b3eafbd487f6 rdf:type skos:Concept;
  skos:editorialNote: """No idea what this is.  Standvink used in DCCD."""@en;
  skos:altLabel "standvink"@nl;
  skos:altLabel "pilier"@fr;
  skos:altLabel "freestanding post"@en;
  skos:altLabel "freistehender ständer"@de;
  skos:inScheme dccd:objectElementType.
dccd:a7a2d774-6b80-11e5-ac02-573ced692617 rdf:type skos:Concept;
  skos:scopeNote """Use for wells sunk to extract water from a zone of saturation """@en;
  skos:editorialNote: """Bohrloch@de needs confirming."""@en;
  skos:exactMatch aat:300152327;
  skos:altLabel "water well"@en;
  skos:altLabel "cisterne"@fr;
  skos:prefLabel "well"@en;
  skos:prefLabel "waterput"@nl;
  skos:prefLabel "puits"@fr;
  skos:prefLabel "Brunnen"@de;
  skos:altLabel "Bohrloch"@de;
  skos:inScheme dccd:objectElementType.
dccd:a7a23b8e-6b80-11e5-ab2b-b78839bafed9 rdf:type skos:Concept;
  skos:editorialNote: """What is this?  Buikdenning used in DCCD."""@en;
  skos:altLabel "vaigrage de cale"@fr;
  skos:prefLabel "bodenwegerung"@de;
  skos:prefLabel "floor ceiling"@en;
  skos:prefLabel "vaigrage de fond"@fr;
  skos:prefLabel "buikdenning"@nl;
  skos:inScheme dccd:objectElementType.
dccd:a7a2c3b0-6b80-11e5-abe8-872f0307e16a rdf:type skos:Concept;
  skos:scopeNote """In complex castles, the spaces between the outer and inner walls """@en;
  skos:editorialNote: """de,nl,fr terms need checking.  Voorburcht used in DCCD."""@en;
  skos:exactMatch aat:300003688;
  skos:prefLabel "bailey"@en;
  skos:altLabel "voorburcht"@nl;
  skos:altLabel "ouvrage avancé"@fr;
  skos:altLabel "château-bas"@fr;
  skos:altLabel "outer bailey"@en;
  skos:altLabel "vorburg"@de;
  skos:altLabel "niederburg"@de;
  skos:inScheme dccd:objectElementType.
dccd:a7a1e314-6b80-11e5-aaaf-bff7d75a954f rdf:type skos:Concept;
  skos:scopeNote """Curved timbers scarfed together to form the lower part of the compound rib of a ship"""@en;
  skos:editorialNote: """de, fr and nl terms need confirming.  Zitter used in DCCD."""@en;
  skos:broadMatch aat:300212614;
  skos:altLabel "genou de couple"@fr;
  skos:altLabel "sitzer"@de;
  skos:altLabel "sitter"@de;
  skos:prefLabel "first futtock"@en;
  skos:altLabel "zitter"@nl;
  skos:inScheme dccd:objectElementType.
